QCP_examples/humaneval/spec_logic_rewrite_c_files/C_118_goal.v
@@ -1,0 +1,2085 @@
+Require Import Coq.ZArith.ZArith.
+Require Import Coq.Bool.Bool.
+Require Import Coq.Strings.String.
+Require Import Coq.Strings.Ascii.
+Require Import Coq.Lists.List.
+Require Import Coq.Classes.RelationClasses.
+Require Import Coq.Classes.Morphisms.
+Require Import Coq.micromega.Psatz.
+Require Import Coq.Sorting.Permutation.
+From AUXLib Require Import int_auto Axioms Feq Idents ListLib VMap.
+Require Import SetsClass.SetsClass. Import SetsNotation.
+From SimpleC.SL Require Import Mem SeparationLogic.
+Require Import Logic.LogicGenerator.demo932.Interface.
+Local Open Scope Z_scope.
+Local Open Scope sets.
+Local Open Scope string_scope.
+Local Open Scope list.
+Import naive_C_Rules.
+Require Import SimpleC.StdLib.string_lib.
+Require Import coins_118.
+Local Open Scope sac.
+From SimpleC.EE.QCP_demos_LLM Require Import char_array_strategy_goal.
+From SimpleC.EE.QCP_demos_LLM Require Import char_array_strategy_proof.
+From SimpleC.StdLib Require Import string_strategy_goal.
+From SimpleC.StdLib Require Import string_strategy_proof.
+
+(*----- Function is_vowel_code_118 -----*)
+
+Definition is_vowel_code_118_safety_wit_1 := 
+forall (ch_pre: Z) (PreH1 : (0 <= ch_pre)) (PreH2 : (ch_pre <= 127)) ,
+  ((( &( "ch" ) )) # Int  |-> ch_pre)
+|--
+  “ (65 <= INT_MAX) ” 
+  &&  “ ((INT_MIN) <= 65) ”
+.
+
+Definition is_vowel_code_118_safety_wit_2 := 
+forall (ch_pre: Z) (PreH1 : (ch_pre = 65)) (PreH2 : (0 <= ch_pre)) (PreH3 : (ch_pre <= 127)) ,
+  ((( &( "ch" ) )) # Int  |-> ch_pre)
+|--
+  “ (1 <= INT_MAX) ” 
+  &&  “ ((INT_MIN) <= 1) ”
+.
+
+Definition is_vowel_code_118_safety_wit_3 := 
+forall (ch_pre: Z) (PreH1 : (ch_pre <> 65)) (PreH2 : (0 <= ch_pre)) (PreH3 : (ch_pre <= 127)) ,
+  ((( &( "ch" ) )) # Int  |-> ch_pre)
+|--
+  “ (69 <= INT_MAX) ” 
+  &&  “ ((INT_MIN) <= 69) ”
+.
+
+Definition is_vowel_code_118_safety_wit_4 := 
+forall (ch_pre: Z) (PreH1 : (ch_pre = 69)) (PreH2 : (ch_pre <> 65)) (PreH3 : (0 <= ch_pre)) (PreH4 : (ch_pre <= 127)) ,
+  ((( &( "ch" ) )) # Int  |-> ch_pre)
+|--
+  “ (1 <= INT_MAX) ” 
+  &&  “ ((INT_MIN) <= 1) ”
+.
+
+Definition is_vowel_code_118_safety_wit_5 := 
+forall (ch_pre: Z) (PreH1 : (ch_pre <> 69)) (PreH2 : (ch_pre <> 65)) (PreH3 : (0 <= ch_pre)) (PreH4 : (ch_pre <= 127)) ,
+  ((( &( "ch" ) )) # Int  |-> ch_pre)
+|--
+  “ (73 <= INT_MAX) ” 
+  &&  “ ((INT_MIN) <= 73) ”
+.
+
+Definition is_vowel_code_118_safety_wit_6 := 
+forall (ch_pre: Z) (PreH1 : (ch_pre = 73)) (PreH2 : (ch_pre <> 69)) (PreH3 : (ch_pre <> 65)) (PreH4 : (0 <= ch_pre)) (PreH5 : (ch_pre <= 127)) ,
+  ((( &( "ch" ) )) # Int  |-> ch_pre)
+|--
+  “ (1 <= INT_MAX) ” 
+  &&  “ ((INT_MIN) <= 1) ”
+.
+
+Definition is_vowel_code_118_safety_wit_7 := 
+forall (ch_pre: Z) (PreH1 : (ch_pre <> 73)) (PreH2 : (ch_pre <> 69)) (PreH3 : (ch_pre <> 65)) (PreH4 : (0 <= ch_pre)) (PreH5 : (ch_pre <= 127)) ,
+  ((( &( "ch" ) )) # Int  |-> ch_pre)
+|--
+  “ (79 <= INT_MAX) ” 
+  &&  “ ((INT_MIN) <= 79) ”
+.
+
+Definition is_vowel_code_118_safety_wit_8 := 
+forall (ch_pre: Z) (PreH1 : (ch_pre = 79)) (PreH2 : (ch_pre <> 73)) (PreH3 : (ch_pre <> 69)) (PreH4 : (ch_pre <> 65)) (PreH5 : (0 <= ch_pre)) (PreH6 : (ch_pre <= 127)) ,
+  ((( &( "ch" ) )) # Int  |-> ch_pre)
+|--
+  “ (1 <= INT_MAX) ” 
+  &&  “ ((INT_MIN) <= 1) ”
+.
+
+Definition is_vowel_code_118_safety_wit_9 := 
+forall (ch_pre: Z) (PreH1 : (ch_pre <> 79)) (PreH2 : (ch_pre <> 73)) (PreH3 : (ch_pre <> 69)) (PreH4 : (ch_pre <> 65)) (PreH5 : (0 <= ch_pre)) (PreH6 : (ch_pre <= 127)) ,
+  ((( &( "ch" ) )) # Int  |-> ch_pre)
+|--
+  “ (85 <= INT_MAX) ” 
+  &&  “ ((INT_MIN) <= 85) ”
+.
+
+Definition is_vowel_code_118_safety_wit_10 := 
+forall (ch_pre: Z) (PreH1 : (ch_pre = 85)) (PreH2 : (ch_pre <> 79)) (PreH3 : (ch_pre <> 73)) (PreH4 : (ch_pre <> 69)) (PreH5 : (ch_pre <> 65)) (PreH6 : (0 <= ch_pre)) (PreH7 : (ch_pre <= 127)) ,
+  ((( &( "ch" ) )) # Int  |-> ch_pre)
+|--
+  “ (1 <= INT_MAX) ” 
+  &&  “ ((INT_MIN) <= 1) ”
+.
+
+Definition is_vowel_code_118_safety_wit_11 := 
+forall (ch_pre: Z) (PreH1 : (ch_pre <> 85)) (PreH2 : (ch_pre <> 79)) (PreH3 : (ch_pre <> 73)) (PreH4 : (ch_pre <> 69)) (PreH5 : (ch_pre <> 65)) (PreH6 : (0 <= ch_pre)) (PreH7 : (ch_pre <= 127)) ,
+  ((( &( "ch" ) )) # Int  |-> ch_pre)
+|--
+  “ (97 <= INT_MAX) ” 
+  &&  “ ((INT_MIN) <= 97) ”
+.
+
+Definition is_vowel_code_118_safety_wit_12 := 
+forall (ch_pre: Z) (PreH1 : (ch_pre = 97)) (PreH2 : (ch_pre <> 85)) (PreH3 : (ch_pre <> 79)) (PreH4 : (ch_pre <> 73)) (PreH5 : (ch_pre <> 69)) (PreH6 : (ch_pre <> 65)) (PreH7 : (0 <= ch_pre)) (PreH8 : (ch_pre <= 127)) ,
+  ((( &( "ch" ) )) # Int  |-> ch_pre)
+|--
+  “ (1 <= INT_MAX) ” 
+  &&  “ ((INT_MIN) <= 1) ”
+.
+
+Definition is_vowel_code_118_safety_wit_13 := 
+forall (ch_pre: Z) (PreH1 : (ch_pre <> 97)) (PreH2 : (ch_pre <> 85)) (PreH3 : (ch_pre <> 79)) (PreH4 : (ch_pre <> 73)) (PreH5 : (ch_pre <> 69)) (PreH6 : (ch_pre <> 65)) (PreH7 : (0 <= ch_pre)) (PreH8 : (ch_pre <= 127)) ,
+  ((( &( "ch" ) )) # Int  |-> ch_pre)
+|--
+  “ (101 <= INT_MAX) ” 
+  &&  “ ((INT_MIN) <= 101) ”
+.
+
+Definition is_vowel_code_118_safety_wit_14 := 
+forall (ch_pre: Z) (PreH1 : (ch_pre = 101)) (PreH2 : (ch_pre <> 97)) (PreH3 : (ch_pre <> 85)) (PreH4 : (ch_pre <> 79)) (PreH5 : (ch_pre <> 73)) (PreH6 : (ch_pre <> 69)) (PreH7 : (ch_pre <> 65)) (PreH8 : (0 <= ch_pre)) (PreH9 : (ch_pre <= 127)) ,
+  ((( &( "ch" ) )) # Int  |-> ch_pre)
+|--
+  “ (1 <= INT_MAX) ” 
+  &&  “ ((INT_MIN) <= 1) ”
+.
+
+Definition is_vowel_code_118_safety_wit_15 := 
+forall (ch_pre: Z) (PreH1 : (ch_pre <> 101)) (PreH2 : (ch_pre <> 97)) (PreH3 : (ch_pre <> 85)) (PreH4 : (ch_pre <> 79)) (PreH5 : (ch_pre <> 73)) (PreH6 : (ch_pre <> 69)) (PreH7 : (ch_pre <> 65)) (PreH8 : (0 <= ch_pre)) (PreH9 : (ch_pre <= 127)) ,
+  ((( &( "ch" ) )) # Int  |-> ch_pre)
+|--
+  “ (105 <= INT_MAX) ” 
+  &&  “ ((INT_MIN) <= 105) ”
+.
+
+Definition is_vowel_code_118_safety_wit_16 := 
+forall (ch_pre: Z) (PreH1 : (ch_pre = 105)) (PreH2 : (ch_pre <> 101)) (PreH3 : (ch_pre <> 97)) (PreH4 : (ch_pre <> 85)) (PreH5 : (ch_pre <> 79)) (PreH6 : (ch_pre <> 73)) (PreH7 : (ch_pre <> 69)) (PreH8 : (ch_pre <> 65)) (PreH9 : (0 <= ch_pre)) (PreH10 : (ch_pre <= 127)) ,
+  ((( &( "ch" ) )) # Int  |-> ch_pre)
+|--
+  “ (1 <= INT_MAX) ” 
+  &&  “ ((INT_MIN) <= 1) ”
+.
+
+Definition is_vowel_code_118_safety_wit_17 := 
+forall (ch_pre: Z) (PreH1 : (ch_pre <> 105)) (PreH2 : (ch_pre <> 101)) (PreH3 : (ch_pre <> 97)) (PreH4 : (ch_pre <> 85)) (PreH5 : (ch_pre <> 79)) (PreH6 : (ch_pre <> 73)) (PreH7 : (ch_pre <> 69)) (PreH8 : (ch_pre <> 65)) (PreH9 : (0 <= ch_pre)) (PreH10 : (ch_pre <= 127)) ,
+  ((( &( "ch" ) )) # Int  |-> ch_pre)
+|--
+  “ (111 <= INT_MAX) ” 
+  &&  “ ((INT_MIN) <= 111) ”
+.
+
+Definition is_vowel_code_118_safety_wit_18 := 
+forall (ch_pre: Z) (PreH1 : (ch_pre = 111)) (PreH2 : (ch_pre <> 105)) (PreH3 : (ch_pre <> 101)) (PreH4 : (ch_pre <> 97)) (PreH5 : (ch_pre <> 85)) (PreH6 : (ch_pre <> 79)) (PreH7 : (ch_pre <> 73)) (PreH8 : (ch_pre <> 69)) (PreH9 : (ch_pre <> 65)) (PreH10 : (0 <= ch_pre)) (PreH11 : (ch_pre <= 127)) ,
+  ((( &( "ch" ) )) # Int  |-> ch_pre)
+|--
+  “ (1 <= INT_MAX) ” 
+  &&  “ ((INT_MIN) <= 1) ”
+.
+
+Definition is_vowel_code_118_safety_wit_19 := 
+forall (ch_pre: Z) (PreH1 : (ch_pre <> 111)) (PreH2 : (ch_pre <> 105)) (PreH3 : (ch_pre <> 101)) (PreH4 : (ch_pre <> 97)) (PreH5 : (ch_pre <> 85)) (PreH6 : (ch_pre <> 79)) (PreH7 : (ch_pre <> 73)) (PreH8 : (ch_pre <> 69)) (PreH9 : (ch_pre <> 65)) (PreH10 : (0 <= ch_pre)) (PreH11 : (ch_pre <= 127)) ,
+  ((( &( "ch" ) )) # Int  |-> ch_pre)
+|--
+  “ (117 <= INT_MAX) ” 
+  &&  “ ((INT_MIN) <= 117) ”
+.
+
+Definition is_vowel_code_118_safety_wit_20 := 
+forall (ch_pre: Z) (PreH1 : (ch_pre = 117)) (PreH2 : (ch_pre <> 111)) (PreH3 : (ch_pre <> 105)) (PreH4 : (ch_pre <> 101)) (PreH5 : (ch_pre <> 97)) (PreH6 : (ch_pre <> 85)) (PreH7 : (ch_pre <> 79)) (PreH8 : (ch_pre <> 73)) (PreH9 : (ch_pre <> 69)) (PreH10 : (ch_pre <> 65)) (PreH11 : (0 <= ch_pre)) (PreH12 : (ch_pre <= 127)) ,
+  ((( &( "ch" ) )) # Int  |-> ch_pre)
+|--
+  “ (1 <= INT_MAX) ” 
+  &&  “ ((INT_MIN) <= 1) ”
+.
+
+Definition is_vowel_code_118_safety_wit_21 := 
+forall (ch_pre: Z) (PreH1 : (ch_pre <> 117)) (PreH2 : (ch_pre <> 111)) (PreH3 : (ch_pre <> 105)) (PreH4 : (ch_pre <> 101)) (PreH5 : (ch_pre <> 97)) (PreH6 : (ch_pre <> 85)) (PreH7 : (ch_pre <> 79)) (PreH8 : (ch_pre <> 73)) (PreH9 : (ch_pre <> 69)) (PreH10 : (ch_pre <> 65)) (PreH11 : (0 <= ch_pre)) (PreH12 : (ch_pre <= 127)) ,
+  ((( &( "ch" ) )) # Int  |-> ch_pre)
+|--
+  “ (0 <= INT_MAX) ” 
+  &&  “ ((INT_MIN) <= 0) ”
+.
+
+Definition is_vowel_code_118_return_wit_1 := 
+forall (ch_pre: Z) (PreH1 : (ch_pre <> 117)) (PreH2 : (ch_pre <> 111)) (PreH3 : (ch_pre <> 105)) (PreH4 : (ch_pre <> 101)) (PreH5 : (ch_pre <> 97)) (PreH6 : (ch_pre <> 85)) (PreH7 : (ch_pre <> 79)) (PreH8 : (ch_pre <> 73)) (PreH9 : (ch_pre <> 69)) (PreH10 : (ch_pre <> 65)) (PreH11 : (0 <= ch_pre)) (PreH12 : (ch_pre <= 127)) ,
+  TT && emp 
+|--
+  (“ (0 = 0) ” 
+  &&  “ ~((is_vowel_z_118 ch_pre )) ”
+  &&  emp)
+  ||
+  (“ (0 = 1) ” 
+  &&  “ (is_vowel_z_118 ch_pre ) ”
+  &&  emp)
+.
+
+Definition is_vowel_code_118_return_wit_2 := 
+forall (ch_pre: Z) (PreH1 : (ch_pre = 117)) (PreH2 : (ch_pre <> 111)) (PreH3 : (ch_pre <> 105)) (PreH4 : (ch_pre <> 101)) (PreH5 : (ch_pre <> 97)) (PreH6 : (ch_pre <> 85)) (PreH7 : (ch_pre <> 79)) (PreH8 : (ch_pre <> 73)) (PreH9 : (ch_pre <> 69)) (PreH10 : (ch_pre <> 65)) (PreH11 : (0 <= ch_pre)) (PreH12 : (ch_pre <= 127)) ,
+  TT && emp 
+|--
+  (“ (1 = 0) ” 
+  &&  “ ~((is_vowel_z_118 ch_pre )) ”
+  &&  emp)
+  ||
+  (“ (1 = 1) ” 
+  &&  “ (is_vowel_z_118 ch_pre ) ”
+  &&  emp)
+.
+
+Definition is_vowel_code_118_return_wit_3 := 
+forall (ch_pre: Z) (PreH1 : (ch_pre = 111)) (PreH2 : (ch_pre <> 105)) (PreH3 : (ch_pre <> 101)) (PreH4 : (ch_pre <> 97)) (PreH5 : (ch_pre <> 85)) (PreH6 : (ch_pre <> 79)) (PreH7 : (ch_pre <> 73)) (PreH8 : (ch_pre <> 69)) (PreH9 : (ch_pre <> 65)) (PreH10 : (0 <= ch_pre)) (PreH11 : (ch_pre <= 127)) ,
+  TT && emp 
+|--
+  (“ (1 = 0) ” 
+  &&  “ ~((is_vowel_z_118 ch_pre )) ”
+  &&  emp)
+  ||
+  (“ (1 = 1) ” 
+  &&  “ (is_vowel_z_118 ch_pre ) ”
+  &&  emp)
+.
+
+Definition is_vowel_code_118_return_wit_4 := 
+forall (ch_pre: Z) (PreH1 : (ch_pre = 105)) (PreH2 : (ch_pre <> 101)) (PreH3 : (ch_pre <> 97)) (PreH4 : (ch_pre <> 85)) (PreH5 : (ch_pre <> 79)) (PreH6 : (ch_pre <> 73)) (PreH7 : (ch_pre <> 69)) (PreH8 : (ch_pre <> 65)) (PreH9 : (0 <= ch_pre)) (PreH10 : (ch_pre <= 127)) ,
+  TT && emp 
+|--
+  (“ (1 = 0) ” 
+  &&  “ ~((is_vowel_z_118 ch_pre )) ”
+  &&  emp)
+  ||
+  (“ (1 = 1) ” 
+  &&  “ (is_vowel_z_118 ch_pre ) ”
+  &&  emp)
+.
+
+Definition is_vowel_code_118_return_wit_5 := 
+forall (ch_pre: Z) (PreH1 : (ch_pre = 101)) (PreH2 : (ch_pre <> 97)) (PreH3 : (ch_pre <> 85)) (PreH4 : (ch_pre <> 79)) (PreH5 : (ch_pre <> 73)) (PreH6 : (ch_pre <> 69)) (PreH7 : (ch_pre <> 65)) (PreH8 : (0 <= ch_pre)) (PreH9 : (ch_pre <= 127)) ,
+  TT && emp 
+|--
+  (“ (1 = 0) ” 
+  &&  “ ~((is_vowel_z_118 ch_pre )) ”
+  &&  emp)
+  ||
+  (“ (1 = 1) ” 
+  &&  “ (is_vowel_z_118 ch_pre ) ”
+  &&  emp)
+.
+
+Definition is_vowel_code_118_return_wit_6 := 
+forall (ch_pre: Z) (PreH1 : (ch_pre = 97)) (PreH2 : (ch_pre <> 85)) (PreH3 : (ch_pre <> 79)) (PreH4 : (ch_pre <> 73)) (PreH5 : (ch_pre <> 69)) (PreH6 : (ch_pre <> 65)) (PreH7 : (0 <= ch_pre)) (PreH8 : (ch_pre <= 127)) ,
+  TT && emp 
+|--
+  (“ (1 = 0) ” 
+  &&  “ ~((is_vowel_z_118 ch_pre )) ”
+  &&  emp)
+  ||
+  (“ (1 = 1) ” 
+  &&  “ (is_vowel_z_118 ch_pre ) ”
+  &&  emp)
+.
+
+Definition is_vowel_code_118_return_wit_7 := 
+forall (ch_pre: Z) (PreH1 : (ch_pre = 85)) (PreH2 : (ch_pre <> 79)) (PreH3 : (ch_pre <> 73)) (PreH4 : (ch_pre <> 69)) (PreH5 : (ch_pre <> 65)) (PreH6 : (0 <= ch_pre)) (PreH7 : (ch_pre <= 127)) ,
+  TT && emp 
+|--
+  (“ (1 = 0) ” 
+  &&  “ ~((is_vowel_z_118 ch_pre )) ”
+  &&  emp)
+  ||
+  (“ (1 = 1) ” 
+  &&  “ (is_vowel_z_118 ch_pre ) ”
+  &&  emp)
+.
+
+Definition is_vowel_code_118_return_wit_8 := 
+forall (ch_pre: Z) (PreH1 : (ch_pre = 79)) (PreH2 : (ch_pre <> 73)) (PreH3 : (ch_pre <> 69)) (PreH4 : (ch_pre <> 65)) (PreH5 : (0 <= ch_pre)) (PreH6 : (ch_pre <= 127)) ,
+  TT && emp 
+|--
+  (“ (1 = 0) ” 
+  &&  “ ~((is_vowel_z_118 ch_pre )) ”
+  &&  emp)
+  ||
+  (“ (1 = 1) ” 
+  &&  “ (is_vowel_z_118 ch_pre ) ”
+  &&  emp)
+.
+
+Definition is_vowel_code_118_return_wit_9 := 
+forall (ch_pre: Z) (PreH1 : (ch_pre = 73)) (PreH2 : (ch_pre <> 69)) (PreH3 : (ch_pre <> 65)) (PreH4 : (0 <= ch_pre)) (PreH5 : (ch_pre <= 127)) ,
+  TT && emp 
+|--
+  (“ (1 = 0) ” 
+  &&  “ ~((is_vowel_z_118 ch_pre )) ”
+  &&  emp)
+  ||
+  (“ (1 = 1) ” 
+  &&  “ (is_vowel_z_118 ch_pre ) ”
+  &&  emp)
+.
+
+Definition is_vowel_code_118_return_wit_10 := 
+forall (ch_pre: Z) (PreH1 : (ch_pre = 69)) (PreH2 : (ch_pre <> 65)) (PreH3 : (0 <= ch_pre)) (PreH4 : (ch_pre <= 127)) ,
+  TT && emp 
+|--
+  (“ (1 = 0) ” 
+  &&  “ ~((is_vowel_z_118 ch_pre )) ”
+  &&  emp)
+  ||
+  (“ (1 = 1) ” 
+  &&  “ (is_vowel_z_118 ch_pre ) ”
+  &&  emp)
+.
+
+Definition is_vowel_code_118_return_wit_11 := 
+forall (ch_pre: Z) (PreH1 : (ch_pre = 65)) (PreH2 : (0 <= ch_pre)) (PreH3 : (ch_pre <= 127)) ,
+  TT && emp 
+|--
+  (“ (1 = 0) ” 
+  &&  “ ~((is_vowel_z_118 ch_pre )) ”
+  &&  emp)
+  ||
+  (“ (1 = 1) ” 
+  &&  “ (is_vowel_z_118 ch_pre ) ”
+  &&  emp)
+.
+
+(*----- Function get_closest_vowel -----*)
+
+Definition get_closest_vowel_safety_wit_1 := 
+forall (word_pre: Z) (input: (@list Z)) (retval: Z) (PreH1 : (retval = (string_length (input)))) (PreH2 : (0 <= ((string_length (input)) + 1 ))) (PreH3 : (valid_string input )) (PreH4 : (all_ascii input )) (PreH5 : (problem_118_pre_z input )) (PreH6 : (ascii_range_z input )) (PreH7 : ((string_length (input)) < INT_MAX)) ,
+  ((( &( "out" ) )) # Ptr  |->_)
+  **  (store_string word_pre input )
+  **  ((( &( "n" ) )) # Int  |-> retval)
+  **  ((( &( "word" ) )) # Ptr  |-> word_pre)
+|--
+  “ (0 <= INT_MAX) ” 
+  &&  “ ((INT_MIN) <= 0) ”
+.
+
+Definition get_closest_vowel_safety_wit_2 := 
+forall (word_pre: Z) (input: (@list Z)) (n: Z) (out: Z) (PreH1 : (n = (string_length (input)))) (PreH2 : (out = 0)) (PreH3 : (valid_string input )) (PreH4 : (all_ascii input )) (PreH5 : (problem_118_pre_z input )) (PreH6 : (ascii_range_z input )) (PreH7 : (alpha_codes_z_118 input )) (PreH8 : ((string_length (input)) < INT_MAX)) ,
+  ((( &( "word" ) )) # Ptr  |-> word_pre)
+  **  ((( &( "n" ) )) # Int  |-> n)
+  **  ((( &( "out" ) )) # Ptr  |-> out)
+  **  (store_string word_pre input )
+|--
+  “ (3 <= INT_MAX) ” 
+  &&  “ ((INT_MIN) <= 3) ”
+.
+
+Definition get_closest_vowel_safety_wit_3 := 
+forall (word_pre: Z) (input: (@list Z)) (n: Z) (out: Z) (PreH1 : (n < 3)) (PreH2 : (n = (string_length (input)))) (PreH3 : (out = 0)) (PreH4 : (valid_string input )) (PreH5 : (all_ascii input )) (PreH6 : (problem_118_pre_z input )) (PreH7 : (ascii_range_z input )) (PreH8 : (alpha_codes_z_118 input )) (PreH9 : ((string_length (input)) < INT_MAX)) ,
+  ((( &( "word" ) )) # Ptr  |-> word_pre)
+  **  ((( &( "n" ) )) # Int  |-> n)
+  **  ((( &( "out" ) )) # Ptr  |-> out)
+  **  (store_string word_pre input )
+|--
+  “ (1 <= INT_MAX) ” 
+  &&  “ ((INT_MIN) <= 1) ”
+.
+
+Definition get_closest_vowel_safety_wit_4 := 
+forall (word_pre: Z) (input: (@list Z)) (n: Z) (out: Z) (retval: Z) (PreH1 : (retval <> 0)) (PreH2 : (0 <= ((string_length (input)) + 1 ))) (PreH3 : (n < 3)) (PreH4 : (n = (string_length (input)))) (PreH5 : (out = 0)) (PreH6 : (valid_string input )) (PreH7 : (all_ascii input )) (PreH8 : (problem_118_pre_z input )) (PreH9 : (ascii_range_z input )) (PreH10 : (alpha_codes_z_118 input )) (PreH11 : ((string_length (input)) < INT_MAX)) ,
+  (CharArray.undef_full retval 1 )
+  **  (CharArray.full word_pre ((string_length (input)) + 1 ) (c_string (input)) )
+  **  ((( &( "word" ) )) # Ptr  |-> word_pre)
+  **  ((( &( "n" ) )) # Int  |-> n)
+  **  ((( &( "out" ) )) # Ptr  |-> retval)
+|--
+  “ (0 <= INT_MAX) ” 
+  &&  “ ((INT_MIN) <= 0) ”
+.
+
+Definition get_closest_vowel_safety_wit_5 := 
+forall (word_pre: Z) (input: (@list Z)) (n: Z) (out: Z) (retval: Z) (PreH1 : (retval = 0)) (PreH2 : (retval <> 0)) (PreH3 : (0 <= ((string_length (input)) + 1 ))) (PreH4 : (n < 3)) (PreH5 : (n = (string_length (input)))) (PreH6 : (out = 0)) (PreH7 : (valid_string input )) (PreH8 : (all_ascii input )) (PreH9 : (problem_118_pre_z input )) (PreH10 : (ascii_range_z input )) (PreH11 : (alpha_codes_z_118 input )) (PreH12 : ((string_length (input)) < INT_MAX)) ,
+  (CharArray.undef_full retval 1 )
+  **  (CharArray.full word_pre ((string_length (input)) + 1 ) (c_string (input)) )
+  **  ((( &( "word" ) )) # Ptr  |-> word_pre)
+  **  ((( &( "n" ) )) # Int  |-> n)
+  **  ((( &( "out" ) )) # Ptr  |-> retval)
+|--
+  “ False ”
+.
+
+Definition get_closest_vowel_safety_wit_6 := 
+forall (word_pre: Z) (input: (@list Z)) (n: Z) (out: Z) (retval: Z) (PreH1 : (retval <> 0)) (PreH2 : (retval <> 0)) (PreH3 : (0 <= ((string_length (input)) + 1 ))) (PreH4 : (n < 3)) (PreH5 : (n = (string_length (input)))) (PreH6 : (out = 0)) (PreH7 : (valid_string input )) (PreH8 : (all_ascii input )) (PreH9 : (problem_118_pre_z input )) (PreH10 : (ascii_range_z input )) (PreH11 : (alpha_codes_z_118 input )) (PreH12 : ((string_length (input)) < INT_MAX)) ,
+  (CharArray.undef_full retval 1 )
+  **  (CharArray.full word_pre ((string_length (input)) + 1 ) (c_string (input)) )
+  **  ((( &( "word" ) )) # Ptr  |-> word_pre)
+  **  ((( &( "n" ) )) # Int  |-> n)
+  **  ((( &( "out" ) )) # Ptr  |-> retval)
+|--
+  “ (0 <= INT_MAX) ” 
+  &&  “ ((INT_MIN) <= 0) ”
+.
+
+Definition get_closest_vowel_safety_wit_7 := 
+forall (word_pre: Z) (input: (@list Z)) (n: Z) (out: Z) (retval: Z) (PreH1 : (retval <> 0)) (PreH2 : (retval <> 0)) (PreH3 : (0 <= ((string_length (input)) + 1 ))) (PreH4 : (n < 3)) (PreH5 : (n = (string_length (input)))) (PreH6 : (out = 0)) (PreH7 : (valid_string input )) (PreH8 : (all_ascii input )) (PreH9 : (problem_118_pre_z input )) (PreH10 : (ascii_range_z input )) (PreH11 : (alpha_codes_z_118 input )) (PreH12 : ((string_length (input)) < INT_MAX)) ,
+  (CharArray.undef_full retval 1 )
+  **  (CharArray.full word_pre ((string_length (input)) + 1 ) (c_string (input)) )
+  **  ((( &( "word" ) )) # Ptr  |-> word_pre)
+  **  ((( &( "n" ) )) # Int  |-> n)
+  **  ((( &( "out" ) )) # Ptr  |-> retval)
+|--
+  “ (0 <= INT_MAX) ” 
+  &&  “ ((INT_MIN) <= 0) ”
+.
+
+Definition get_closest_vowel_safety_wit_8 := 
+forall (word_pre: Z) (input: (@list Z)) (n: Z) (out: Z) (PreH1 : (n >= 3)) (PreH2 : (n = (string_length (input)))) (PreH3 : (out = 0)) (PreH4 : (valid_string input )) (PreH5 : (all_ascii input )) (PreH6 : (problem_118_pre_z input )) (PreH7 : (ascii_range_z input )) (PreH8 : (alpha_codes_z_118 input )) (PreH9 : ((string_length (input)) < INT_MAX)) ,
+  ((( &( "cur" ) )) # Int  |->_)
+  **  ((( &( "i" ) )) # Int  |->_)
+  **  ((( &( "word" ) )) # Ptr  |-> word_pre)
+  **  ((( &( "n" ) )) # Int  |-> n)
+  **  ((( &( "out" ) )) # Ptr  |-> out)
+  **  (store_string word_pre input )
+|--
+  “ (0 <= INT_MAX) ” 
+  &&  “ ((INT_MIN) <= 0) ”
+.
+
+Definition get_closest_vowel_safety_wit_9 := 
+forall (word_pre: Z) (input: (@list Z)) (n: Z) (out: Z) (PreH1 : (n >= 3)) (PreH2 : (n = (string_length (input)))) (PreH3 : (out = 0)) (PreH4 : (valid_string input )) (PreH5 : (all_ascii input )) (PreH6 : (problem_118_pre_z input )) (PreH7 : (ascii_range_z input )) (PreH8 : (alpha_codes_z_118 input )) (PreH9 : ((string_length (input)) < INT_MAX)) ,
+  ((( &( "right" ) )) # Int  |->_)
+  **  ((( &( "cur" ) )) # Int  |-> 0)
+  **  ((( &( "i" ) )) # Int  |->_)
+  **  ((( &( "word" ) )) # Ptr  |-> word_pre)
+  **  ((( &( "n" ) )) # Int  |-> n)
+  **  ((( &( "out" ) )) # Ptr  |-> out)
+  **  (store_string word_pre input )
+|--
+  “ (0 <= INT_MAX) ” 
+  &&  “ ((INT_MIN) <= 0) ”
+.
+
+Definition get_closest_vowel_safety_wit_10 := 
+forall (word_pre: Z) (input: (@list Z)) (n: Z) (out: Z) (PreH1 : (n >= 3)) (PreH2 : (n = (string_length (input)))) (PreH3 : (out = 0)) (PreH4 : (valid_string input )) (PreH5 : (all_ascii input )) (PreH6 : (problem_118_pre_z input )) (PreH7 : (ascii_range_z input )) (PreH8 : (alpha_codes_z_118 input )) (PreH9 : ((string_length (input)) < INT_MAX)) ,
+  ((( &( "left" ) )) # Int  |->_)
+  **  ((( &( "right" ) )) # Int  |-> 0)
+  **  ((( &( "cur" ) )) # Int  |-> 0)
+  **  ((( &( "i" ) )) # Int  |->_)
+  **  ((( &( "word" ) )) # Ptr  |-> word_pre)
+  **  ((( &( "n" ) )) # Int  |-> n)
+  **  ((( &( "out" ) )) # Ptr  |-> out)
+  **  (store_string word_pre input )
+|--
+  “ (0 <= INT_MAX) ” 
+  &&  “ ((INT_MIN) <= 0) ”
+.
+
+Definition get_closest_vowel_safety_wit_11 := 
+forall (word_pre: Z) (input: (@list Z)) (n: Z) (out: Z) (PreH1 : (n >= 3)) (PreH2 : (n = (string_length (input)))) (PreH3 : (out = 0)) (PreH4 : (valid_string input )) (PreH5 : (all_ascii input )) (PreH6 : (problem_118_pre_z input )) (PreH7 : (ascii_range_z input )) (PreH8 : (alpha_codes_z_118 input )) (PreH9 : ((string_length (input)) < INT_MAX)) ,
+  ((( &( "cur_vowel" ) )) # Int  |->_)
+  **  ((( &( "left" ) )) # Int  |-> 0)
+  **  ((( &( "right" ) )) # Int  |-> 0)
+  **  ((( &( "cur" ) )) # Int  |-> 0)
+  **  ((( &( "i" ) )) # Int  |->_)
+  **  ((( &( "word" ) )) # Ptr  |-> word_pre)
+  **  ((( &( "n" ) )) # Int  |-> n)
+  **  ((( &( "out" ) )) # Ptr  |-> out)
+  **  (store_string word_pre input )
+|--
+  “ (0 <= INT_MAX) ” 
+  &&  “ ((INT_MIN) <= 0) ”
+.
+
+Definition get_closest_vowel_safety_wit_12 := 
+forall (word_pre: Z) (input: (@list Z)) (n: Z) (out: Z) (PreH1 : (n >= 3)) (PreH2 : (n = (string_length (input)))) (PreH3 : (out = 0)) (PreH4 : (valid_string input )) (PreH5 : (all_ascii input )) (PreH6 : (problem_118_pre_z input )) (PreH7 : (ascii_range_z input )) (PreH8 : (alpha_codes_z_118 input )) (PreH9 : ((string_length (input)) < INT_MAX)) ,
+  ((( &( "right_vowel" ) )) # Int  |->_)
+  **  ((( &( "cur_vowel" ) )) # Int  |-> 0)
+  **  ((( &( "left" ) )) # Int  |-> 0)
+  **  ((( &( "right" ) )) # Int  |-> 0)
+  **  ((( &( "cur" ) )) # Int  |-> 0)
+  **  ((( &( "i" ) )) # Int  |->_)
+  **  ((( &( "word" ) )) # Ptr  |-> word_pre)
+  **  ((( &( "n" ) )) # Int  |-> n)
+  **  ((( &( "out" ) )) # Ptr  |-> out)
+  **  (store_string word_pre input )
+|--
+  “ (0 <= INT_MAX) ” 
+  &&  “ ((INT_MIN) <= 0) ”
+.
+
+Definition get_closest_vowel_safety_wit_13 := 
+forall (word_pre: Z) (input: (@list Z)) (n: Z) (out: Z) (PreH1 : (n >= 3)) (PreH2 : (n = (string_length (input)))) (PreH3 : (out = 0)) (PreH4 : (valid_string input )) (PreH5 : (all_ascii input )) (PreH6 : (problem_118_pre_z input )) (PreH7 : (ascii_range_z input )) (PreH8 : (alpha_codes_z_118 input )) (PreH9 : ((string_length (input)) < INT_MAX)) ,
+  ((( &( "left_vowel" ) )) # Int  |->_)
+  **  ((( &( "right_vowel" ) )) # Int  |-> 0)
+  **  ((( &( "cur_vowel" ) )) # Int  |-> 0)
+  **  ((( &( "left" ) )) # Int  |-> 0)
+  **  ((( &( "right" ) )) # Int  |-> 0)
+  **  ((( &( "cur" ) )) # Int  |-> 0)
+  **  ((( &( "i" ) )) # Int  |->_)
+  **  ((( &( "word" ) )) # Ptr  |-> word_pre)
+  **  ((( &( "n" ) )) # Int  |-> n)
+  **  ((( &( "out" ) )) # Ptr  |-> out)
+  **  (store_string word_pre input )
+|--
+  “ (0 <= INT_MAX) ” 
+  &&  “ ((INT_MIN) <= 0) ”
+.
+
+Definition get_closest_vowel_safety_wit_14 := 
+forall (word_pre: Z) (input: (@list Z)) (n: Z) (out: Z) (PreH1 : (n >= 3)) (PreH2 : (n = (string_length (input)))) (PreH3 : (out = 0)) (PreH4 : (valid_string input )) (PreH5 : (all_ascii input )) (PreH6 : (problem_118_pre_z input )) (PreH7 : (ascii_range_z input )) (PreH8 : (alpha_codes_z_118 input )) (PreH9 : ((string_length (input)) < INT_MAX)) ,
+  ((( &( "left_vowel" ) )) # Int  |-> 0)
+  **  ((( &( "right_vowel" ) )) # Int  |-> 0)
+  **  ((( &( "cur_vowel" ) )) # Int  |-> 0)
+  **  ((( &( "left" ) )) # Int  |-> 0)
+  **  ((( &( "right" ) )) # Int  |-> 0)
+  **  ((( &( "cur" ) )) # Int  |-> 0)
+  **  ((( &( "i" ) )) # Int  |->_)
+  **  ((( &( "word" ) )) # Ptr  |-> word_pre)
+  **  ((( &( "n" ) )) # Int  |-> n)
+  **  ((( &( "out" ) )) # Ptr  |-> out)
+  **  (store_string word_pre input )
+|--
+  “ ((n - 2 ) <= INT_MAX) ” 
+  &&  “ ((INT_MIN) <= (n - 2 )) ”
+.
+
+Definition get_closest_vowel_safety_wit_15 := 
+forall (word_pre: Z) (input: (@list Z)) (n: Z) (out: Z) (PreH1 : (n >= 3)) (PreH2 : (n = (string_length (input)))) (PreH3 : (out = 0)) (PreH4 : (valid_string input )) (PreH5 : (all_ascii input )) (PreH6 : (problem_118_pre_z input )) (PreH7 : (ascii_range_z input )) (PreH8 : (alpha_codes_z_118 input )) (PreH9 : ((string_length (input)) < INT_MAX)) ,
+  ((( &( "left_vowel" ) )) # Int  |-> 0)
+  **  ((( &( "right_vowel" ) )) # Int  |-> 0)
+  **  ((( &( "cur_vowel" ) )) # Int  |-> 0)
+  **  ((( &( "left" ) )) # Int  |-> 0)
+  **  ((( &( "right" ) )) # Int  |-> 0)
+  **  ((( &( "cur" ) )) # Int  |-> 0)
+  **  ((( &( "i" ) )) # Int  |->_)
+  **  ((( &( "word" ) )) # Ptr  |-> word_pre)
+  **  ((( &( "n" ) )) # Int  |-> n)
+  **  ((( &( "out" ) )) # Ptr  |-> out)
+  **  (store_string word_pre input )
+|--
+  “ (2 <= INT_MAX) ” 
+  &&  “ ((INT_MIN) <= 2) ”
+.
+
+Definition get_closest_vowel_safety_wit_16 := 
+forall (word_pre: Z) (input: (@list Z)) (i: Z) (left_vowel: Z) (right_vowel: Z) (cur_vowel: Z) (left: Z) (right: Z) (cur: Z) (out: Z) (n: Z) (PreH1 : (n = (string_length (input)))) (PreH2 : (out = 0)) (PreH3 : (3 <= n)) (PreH4 : (n < INT_MAX)) (PreH5 : (0 <= i)) (PreH6 : (i <= (n - 2 ))) (PreH7 : (valid_string input )) (PreH8 : (all_ascii input )) (PreH9 : (problem_118_pre_z input )) (PreH10 : (ascii_range_z input )) (PreH11 : (alpha_codes_z_118 input )) (PreH12 : (no_candidate_after_z_118 input i )) ,
+  ((( &( "word" ) )) # Ptr  |-> word_pre)
+  **  ((( &( "n" ) )) # Int  |-> n)
+  **  ((( &( "out" ) )) # Ptr  |-> out)
+  **  ((( &( "cur" ) )) # Int  |-> cur)
+  **  ((( &( "right" ) )) # Int  |-> right)
+  **  ((( &( "left" ) )) # Int  |-> left)
+  **  ((( &( "cur_vowel" ) )) # Int  |-> cur_vowel)
+  **  ((( &( "right_vowel" ) )) # Int  |-> right_vowel)
+  **  ((( &( "left_vowel" ) )) # Int  |-> left_vowel)
+  **  ((( &( "i" ) )) # Int  |-> i)
+  **  (store_string word_pre input )
+|--
+  “ (1 <= INT_MAX) ” 
+  &&  “ ((INT_MIN) <= 1) ”
+.
+
+Definition get_closest_vowel_safety_wit_17 := 
+forall (word_pre: Z) (input: (@list Z)) (i: Z) (left_vowel: Z) (right_vowel: Z) (cur_vowel: Z) (left: Z) (right: Z) (out: Z) (n: Z) (PreH1 : (i >= 1)) (PreH2 : (n = (string_length (input)))) (PreH3 : (out = 0)) (PreH4 : (3 <= n)) (PreH5 : (n < INT_MAX)) (PreH6 : (0 <= i)) (PreH7 : (i <= (n - 2 ))) (PreH8 : (valid_string input )) (PreH9 : (all_ascii input )) (PreH10 : (problem_118_pre_z input )) (PreH11 : (ascii_range_z input )) (PreH12 : (alpha_codes_z_118 input )) (PreH13 : (no_candidate_after_z_118 input i )) ,
+  ((( &( "word" ) )) # Ptr  |-> word_pre)
+  **  ((( &( "n" ) )) # Int  |-> n)
+  **  ((( &( "out" ) )) # Ptr  |-> out)
+  **  ((( &( "cur" ) )) # Int  |-> (Znth i (c_string (input)) 0))
+  **  ((( &( "right" ) )) # Int  |-> right)
+  **  ((( &( "left" ) )) # Int  |-> left)
+  **  ((( &( "cur_vowel" ) )) # Int  |-> cur_vowel)
+  **  ((( &( "right_vowel" ) )) # Int  |-> right_vowel)
+  **  ((( &( "left_vowel" ) )) # Int  |-> left_vowel)
+  **  ((( &( "i" ) )) # Int  |-> i)
+  **  (store_string word_pre input )
+|--
+  “ ((i + 1 ) <= INT_MAX) ” 
+  &&  “ ((INT_MIN) <= (i + 1 )) ”
+.
+
+Definition get_closest_vowel_safety_wit_18 := 
+forall (word_pre: Z) (input: (@list Z)) (i: Z) (left_vowel: Z) (right_vowel: Z) (cur_vowel: Z) (left: Z) (right: Z) (out: Z) (n: Z) (PreH1 : (i >= 1)) (PreH2 : (n = (string_length (input)))) (PreH3 : (out = 0)) (PreH4 : (3 <= n)) (PreH5 : (n < INT_MAX)) (PreH6 : (0 <= i)) (PreH7 : (i <= (n - 2 ))) (PreH8 : (valid_string input )) (PreH9 : (all_ascii input )) (PreH10 : (problem_118_pre_z input )) (PreH11 : (ascii_range_z input )) (PreH12 : (alpha_codes_z_118 input )) (PreH13 : (no_candidate_after_z_118 input i )) ,
+  ((( &( "word" ) )) # Ptr  |-> word_pre)
+  **  ((( &( "n" ) )) # Int  |-> n)
+  **  ((( &( "out" ) )) # Ptr  |-> out)
+  **  ((( &( "cur" ) )) # Int  |-> (Znth i (c_string (input)) 0))
+  **  ((( &( "right" ) )) # Int  |-> right)
+  **  ((( &( "left" ) )) # Int  |-> left)
+  **  ((( &( "cur_vowel" ) )) # Int  |-> cur_vowel)
+  **  ((( &( "right_vowel" ) )) # Int  |-> right_vowel)
+  **  ((( &( "left_vowel" ) )) # Int  |-> left_vowel)
+  **  ((( &( "i" ) )) # Int  |-> i)
+  **  (store_string word_pre input )
+|--
+  “ (1 <= INT_MAX) ” 
+  &&  “ ((INT_MIN) <= 1) ”
+.
+
+Definition get_closest_vowel_safety_wit_19 := 
+forall (word_pre: Z) (input: (@list Z)) (i: Z) (left_vowel: Z) (right_vowel: Z) (cur_vowel: Z) (left: Z) (out: Z) (n: Z) (PreH1 : (i >= 1)) (PreH2 : (n = (string_length (input)))) (PreH3 : (out = 0)) (PreH4 : (3 <= n)) (PreH5 : (n < INT_MAX)) (PreH6 : (0 <= i)) (PreH7 : (i <= (n - 2 ))) (PreH8 : (valid_string input )) (PreH9 : (all_ascii input )) (PreH10 : (problem_118_pre_z input )) (PreH11 : (ascii_range_z input )) (PreH12 : (alpha_codes_z_118 input )) (PreH13 : (no_candidate_after_z_118 input i )) ,
+  ((( &( "word" ) )) # Ptr  |-> word_pre)
+  **  ((( &( "n" ) )) # Int  |-> n)
+  **  ((( &( "out" ) )) # Ptr  |-> out)
+  **  ((( &( "cur" ) )) # Int  |-> (Znth i (c_string (input)) 0))
+  **  ((( &( "right" ) )) # Int  |-> (Znth (i + 1 ) (c_string (input)) 0))
+  **  ((( &( "left" ) )) # Int  |-> left)
+  **  ((( &( "cur_vowel" ) )) # Int  |-> cur_vowel)
+  **  ((( &( "right_vowel" ) )) # Int  |-> right_vowel)
+  **  ((( &( "left_vowel" ) )) # Int  |-> left_vowel)
+  **  ((( &( "i" ) )) # Int  |-> i)
+  **  (store_string word_pre input )
+|--
+  “ ((i - 1 ) <= INT_MAX) ” 
+  &&  “ ((INT_MIN) <= (i - 1 )) ”
+.
+
+Definition get_closest_vowel_safety_wit_20 := 
+forall (word_pre: Z) (input: (@list Z)) (i: Z) (left_vowel: Z) (right_vowel: Z) (cur_vowel: Z) (left: Z) (out: Z) (n: Z) (PreH1 : (i >= 1)) (PreH2 : (n = (string_length (input)))) (PreH3 : (out = 0)) (PreH4 : (3 <= n)) (PreH5 : (n < INT_MAX)) (PreH6 : (0 <= i)) (PreH7 : (i <= (n - 2 ))) (PreH8 : (valid_string input )) (PreH9 : (all_ascii input )) (PreH10 : (problem_118_pre_z input )) (PreH11 : (ascii_range_z input )) (PreH12 : (alpha_codes_z_118 input )) (PreH13 : (no_candidate_after_z_118 input i )) ,
+  ((( &( "word" ) )) # Ptr  |-> word_pre)
+  **  ((( &( "n" ) )) # Int  |-> n)
+  **  ((( &( "out" ) )) # Ptr  |-> out)
+  **  ((( &( "cur" ) )) # Int  |-> (Znth i (c_string (input)) 0))
+  **  ((( &( "right" ) )) # Int  |-> (Znth (i + 1 ) (c_string (input)) 0))
+  **  ((( &( "left" ) )) # Int  |-> left)
+  **  ((( &( "cur_vowel" ) )) # Int  |-> cur_vowel)
+  **  ((( &( "right_vowel" ) )) # Int  |-> right_vowel)
+  **  ((( &( "left_vowel" ) )) # Int  |-> left_vowel)
+  **  ((( &( "i" ) )) # Int  |-> i)
+  **  (store_string word_pre input )
+|--
+  “ (1 <= INT_MAX) ” 
+  &&  “ ((INT_MIN) <= 1) ”
+.
+
+Definition get_closest_vowel_safety_wit_21 := 
+forall (word_pre: Z) (input: (@list Z)) (i: Z) (left_vowel: Z) (right_vowel: Z) (out: Z) (n: Z) (retval: Z) (PreH1 : (retval = 0)) (PreH2 : ~((is_vowel_z_118 (Znth i (c_string (input)) 0) ))) (PreH3 : (0 <= ((string_length (input)) + 1 ))) (PreH4 : (i >= 1)) (PreH5 : (n = (string_length (input)))) (PreH6 : (out = 0)) (PreH7 : (3 <= n)) (PreH8 : (n < INT_MAX)) (PreH9 : (0 <= i)) (PreH10 : (i <= (n - 2 ))) (PreH11 : (valid_string input )) (PreH12 : (all_ascii input )) (PreH13 : (problem_118_pre_z input )) (PreH14 : (ascii_range_z input )) (PreH15 : (alpha_codes_z_118 input )) (PreH16 : (no_candidate_after_z_118 input i )) ,
+  (CharArray.full word_pre ((string_length (input)) + 1 ) (c_string (input)) )
+  **  ((( &( "word" ) )) # Ptr  |-> word_pre)
+  **  ((( &( "n" ) )) # Int  |-> n)
+  **  ((( &( "out" ) )) # Ptr  |-> out)
+  **  ((( &( "cur" ) )) # Int  |-> (Znth i (c_string (input)) 0))
+  **  ((( &( "right" ) )) # Int  |-> (Znth (i + 1 ) (c_string (input)) 0))
+  **  ((( &( "left" ) )) # Int  |-> (Znth (i - 1 ) (c_string (input)) 0))
+  **  ((( &( "cur_vowel" ) )) # Int  |-> retval)
+  **  ((( &( "right_vowel" ) )) # Int  |-> right_vowel)
+  **  ((( &( "left_vowel" ) )) # Int  |-> left_vowel)
+  **  ((( &( "i" ) )) # Int  |-> i)
+|--
+  “ (1 <= INT_MAX) ” 
+  &&  “ ((INT_MIN) <= 1) ”
+.
+
+Definition get_closest_vowel_safety_wit_22 := 
+forall (word_pre: Z) (input: (@list Z)) (i: Z) (left_vowel: Z) (right_vowel: Z) (out: Z) (n: Z) (retval: Z) (PreH1 : (retval = 1)) (PreH2 : (is_vowel_z_118 (Znth i (c_string (input)) 0) )) (PreH3 : (0 <= ((string_length (input)) + 1 ))) (PreH4 : (i >= 1)) (PreH5 : (n = (string_length (input)))) (PreH6 : (out = 0)) (PreH7 : (3 <= n)) (PreH8 : (n < INT_MAX)) (PreH9 : (0 <= i)) (PreH10 : (i <= (n - 2 ))) (PreH11 : (valid_string input )) (PreH12 : (all_ascii input )) (PreH13 : (problem_118_pre_z input )) (PreH14 : (ascii_range_z input )) (PreH15 : (alpha_codes_z_118 input )) (PreH16 : (no_candidate_after_z_118 input i )) ,
+  (CharArray.full word_pre ((string_length (input)) + 1 ) (c_string (input)) )
+  **  ((( &( "word" ) )) # Ptr  |-> word_pre)
+  **  ((( &( "n" ) )) # Int  |-> n)
+  **  ((( &( "out" ) )) # Ptr  |-> out)
+  **  ((( &( "cur" ) )) # Int  |-> (Znth i (c_string (input)) 0))
+  **  ((( &( "right" ) )) # Int  |-> (Znth (i + 1 ) (c_string (input)) 0))
+  **  ((( &( "left" ) )) # Int  |-> (Znth (i - 1 ) (c_string (input)) 0))
+  **  ((( &( "cur_vowel" ) )) # Int  |-> retval)
+  **  ((( &( "right_vowel" ) )) # Int  |-> right_vowel)
+  **  ((( &( "left_vowel" ) )) # Int  |-> left_vowel)
+  **  ((( &( "i" ) )) # Int  |-> i)
+|--
+  “ (1 <= INT_MAX) ” 
+  &&  “ ((INT_MIN) <= 1) ”
+.
+
+Definition get_closest_vowel_safety_wit_23 := 
+forall (word_pre: Z) (input: (@list Z)) (i: Z) (left_vowel: Z) (right_vowel: Z) (out: Z) (n: Z) (retval: Z) (PreH1 : (retval = 1)) (PreH2 : (retval = 0)) (PreH3 : ~((is_vowel_z_118 (Znth i (c_string (input)) 0) ))) (PreH4 : (0 <= ((string_length (input)) + 1 ))) (PreH5 : (i >= 1)) (PreH6 : (n = (string_length (input)))) (PreH7 : (out = 0)) (PreH8 : (3 <= n)) (PreH9 : (n < INT_MAX)) (PreH10 : (0 <= i)) (PreH11 : (i <= (n - 2 ))) (PreH12 : (valid_string input )) (PreH13 : (all_ascii input )) (PreH14 : (problem_118_pre_z input )) (PreH15 : (ascii_range_z input )) (PreH16 : (alpha_codes_z_118 input )) (PreH17 : (no_candidate_after_z_118 input i )) ,
+  (CharArray.full word_pre ((string_length (input)) + 1 ) (c_string (input)) )
+  **  ((( &( "word" ) )) # Ptr  |-> word_pre)
+  **  ((( &( "n" ) )) # Int  |-> n)
+  **  ((( &( "out" ) )) # Ptr  |-> out)
+  **  ((( &( "cur" ) )) # Int  |-> (Znth i (c_string (input)) 0))
+  **  ((( &( "right" ) )) # Int  |-> (Znth (i + 1 ) (c_string (input)) 0))
+  **  ((( &( "left" ) )) # Int  |-> (Znth (i - 1 ) (c_string (input)) 0))
+  **  ((( &( "cur_vowel" ) )) # Int  |-> retval)
+  **  ((( &( "right_vowel" ) )) # Int  |-> right_vowel)
+  **  ((( &( "left_vowel" ) )) # Int  |-> left_vowel)
+  **  ((( &( "i" ) )) # Int  |-> i)
+|--
+  “ False ”
+.
+
+Definition get_closest_vowel_safety_wit_24 := 
+forall (word_pre: Z) (input: (@list Z)) (i: Z) (left_vowel: Z) (right_vowel: Z) (out: Z) (n: Z) (retval: Z) (PreH1 : (retval <> 1)) (PreH2 : (retval = 1)) (PreH3 : (is_vowel_z_118 (Znth i (c_string (input)) 0) )) (PreH4 : (0 <= ((string_length (input)) + 1 ))) (PreH5 : (i >= 1)) (PreH6 : (n = (string_length (input)))) (PreH7 : (out = 0)) (PreH8 : (3 <= n)) (PreH9 : (n < INT_MAX)) (PreH10 : (0 <= i)) (PreH11 : (i <= (n - 2 ))) (PreH12 : (valid_string input )) (PreH13 : (all_ascii input )) (PreH14 : (problem_118_pre_z input )) (PreH15 : (ascii_range_z input )) (PreH16 : (alpha_codes_z_118 input )) (PreH17 : (no_candidate_after_z_118 input i )) ,
+  (CharArray.full word_pre ((string_length (input)) + 1 ) (c_string (input)) )
+  **  ((( &( "word" ) )) # Ptr  |-> word_pre)
+  **  ((( &( "n" ) )) # Int  |-> n)
+  **  ((( &( "out" ) )) # Ptr  |-> out)
+  **  ((( &( "cur" ) )) # Int  |-> (Znth i (c_string (input)) 0))
+  **  ((( &( "right" ) )) # Int  |-> (Znth (i + 1 ) (c_string (input)) 0))
+  **  ((( &( "left" ) )) # Int  |-> (Znth (i - 1 ) (c_string (input)) 0))
+  **  ((( &( "cur_vowel" ) )) # Int  |-> retval)
+  **  ((( &( "right_vowel" ) )) # Int  |-> right_vowel)
+  **  ((( &( "left_vowel" ) )) # Int  |-> left_vowel)
+  **  ((( &( "i" ) )) # Int  |-> i)
+|--
+  “ False ”
+.
+
+Definition get_closest_vowel_safety_wit_25 := 
+forall (word_pre: Z) (input: (@list Z)) (i: Z) (left_vowel: Z) (out: Z) (n: Z) (retval: Z) (retval_2: Z) (PreH1 : (retval_2 = 0)) (PreH2 : ~((is_vowel_z_118 (Znth (i + 1 ) (c_string (input)) 0) ))) (PreH3 : (retval = 1)) (PreH4 : (retval = 1)) (PreH5 : (is_vowel_z_118 (Znth i (c_string (input)) 0) )) (PreH6 : (0 <= ((string_length (input)) + 1 ))) (PreH7 : (i >= 1)) (PreH8 : (n = (string_length (input)))) (PreH9 : (out = 0)) (PreH10 : (3 <= n)) (PreH11 : (n < INT_MAX)) (PreH12 : (0 <= i)) (PreH13 : (i <= (n - 2 ))) (PreH14 : (valid_string input )) (PreH15 : (all_ascii input )) (PreH16 : (problem_118_pre_z input )) (PreH17 : (ascii_range_z input )) (PreH18 : (alpha_codes_z_118 input )) (PreH19 : (no_candidate_after_z_118 input i )) ,
+  (CharArray.full word_pre ((string_length (input)) + 1 ) (c_string (input)) )
+  **  ((( &( "word" ) )) # Ptr  |-> word_pre)
+  **  ((( &( "n" ) )) # Int  |-> n)
+  **  ((( &( "out" ) )) # Ptr  |-> out)
+  **  ((( &( "cur" ) )) # Int  |-> (Znth i (c_string (input)) 0))
+  **  ((( &( "right" ) )) # Int  |-> (Znth (i + 1 ) (c_string (input)) 0))
+  **  ((( &( "left" ) )) # Int  |-> (Znth (i - 1 ) (c_string (input)) 0))
+  **  ((( &( "cur_vowel" ) )) # Int  |-> retval)
+  **  ((( &( "right_vowel" ) )) # Int  |-> retval_2)
+  **  ((( &( "left_vowel" ) )) # Int  |-> left_vowel)
+  **  ((( &( "i" ) )) # Int  |-> i)
+|--
+  “ (0 <= INT_MAX) ” 
+  &&  “ ((INT_MIN) <= 0) ”
+.
+
+Definition get_closest_vowel_safety_wit_26 := 
+forall (word_pre: Z) (input: (@list Z)) (i: Z) (left_vowel: Z) (out: Z) (n: Z) (retval: Z) (retval_2: Z) (PreH1 : (retval_2 = 1)) (PreH2 : (is_vowel_z_118 (Znth (i + 1 ) (c_string (input)) 0) )) (PreH3 : (retval = 1)) (PreH4 : (retval = 1)) (PreH5 : (is_vowel_z_118 (Znth i (c_string (input)) 0) )) (PreH6 : (0 <= ((string_length (input)) + 1 ))) (PreH7 : (i >= 1)) (PreH8 : (n = (string_length (input)))) (PreH9 : (out = 0)) (PreH10 : (3 <= n)) (PreH11 : (n < INT_MAX)) (PreH12 : (0 <= i)) (PreH13 : (i <= (n - 2 ))) (PreH14 : (valid_string input )) (PreH15 : (all_ascii input )) (PreH16 : (problem_118_pre_z input )) (PreH17 : (ascii_range_z input )) (PreH18 : (alpha_codes_z_118 input )) (PreH19 : (no_candidate_after_z_118 input i )) ,
+  (CharArray.full word_pre ((string_length (input)) + 1 ) (c_string (input)) )
+  **  ((( &( "word" ) )) # Ptr  |-> word_pre)
+  **  ((( &( "n" ) )) # Int  |-> n)
+  **  ((( &( "out" ) )) # Ptr  |-> out)
+  **  ((( &( "cur" ) )) # Int  |-> (Znth i (c_string (input)) 0))
+  **  ((( &( "right" ) )) # Int  |-> (Znth (i + 1 ) (c_string (input)) 0))
+  **  ((( &( "left" ) )) # Int  |-> (Znth (i - 1 ) (c_string (input)) 0))
+  **  ((( &( "cur_vowel" ) )) # Int  |-> retval)
+  **  ((( &( "right_vowel" ) )) # Int  |-> retval_2)
+  **  ((( &( "left_vowel" ) )) # Int  |-> left_vowel)
+  **  ((( &( "i" ) )) # Int  |-> i)
+|--
+  “ (0 <= INT_MAX) ” 
+  &&  “ ((INT_MIN) <= 0) ”
+.
+
+Definition get_closest_vowel_safety_wit_27 := 
+forall (word_pre: Z) (input: (@list Z)) (i: Z) (left_vowel: Z) (out: Z) (n: Z) (retval: Z) (retval_2: Z) (PreH1 : (retval_2 <> 0)) (PreH2 : (retval_2 = 0)) (PreH3 : ~((is_vowel_z_118 (Znth (i + 1 ) (c_string (input)) 0) ))) (PreH4 : (retval = 1)) (PreH5 : (retval = 1)) (PreH6 : (is_vowel_z_118 (Znth i (c_string (input)) 0) )) (PreH7 : (0 <= ((string_length (input)) + 1 ))) (PreH8 : (i >= 1)) (PreH9 : (n = (string_length (input)))) (PreH10 : (out = 0)) (PreH11 : (3 <= n)) (PreH12 : (n < INT_MAX)) (PreH13 : (0 <= i)) (PreH14 : (i <= (n - 2 ))) (PreH15 : (valid_string input )) (PreH16 : (all_ascii input )) (PreH17 : (problem_118_pre_z input )) (PreH18 : (ascii_range_z input )) (PreH19 : (alpha_codes_z_118 input )) (PreH20 : (no_candidate_after_z_118 input i )) ,
+  (CharArray.full word_pre ((string_length (input)) + 1 ) (c_string (input)) )
+  **  ((( &( "word" ) )) # Ptr  |-> word_pre)
+  **  ((( &( "n" ) )) # Int  |-> n)
+  **  ((( &( "out" ) )) # Ptr  |-> out)
+  **  ((( &( "cur" ) )) # Int  |-> (Znth i (c_string (input)) 0))
+  **  ((( &( "right" ) )) # Int  |-> (Znth (i + 1 ) (c_string (input)) 0))
+  **  ((( &( "left" ) )) # Int  |-> (Znth (i - 1 ) (c_string (input)) 0))
+  **  ((( &( "cur_vowel" ) )) # Int  |-> retval)
+  **  ((( &( "right_vowel" ) )) # Int  |-> retval_2)
+  **  ((( &( "left_vowel" ) )) # Int  |-> left_vowel)
+  **  ((( &( "i" ) )) # Int  |-> i)
+|--
+  “ False ”
+.
+
+Definition get_closest_vowel_safety_wit_28 := 
+forall (word_pre: Z) (input: (@list Z)) (i: Z) (left_vowel: Z) (out: Z) (n: Z) (retval: Z) (retval_2: Z) (PreH1 : (retval_2 = 0)) (PreH2 : (retval_2 = 1)) (PreH3 : (is_vowel_z_118 (Znth (i + 1 ) (c_string (input)) 0) )) (PreH4 : (retval = 1)) (PreH5 : (retval = 1)) (PreH6 : (is_vowel_z_118 (Znth i (c_string (input)) 0) )) (PreH7 : (0 <= ((string_length (input)) + 1 ))) (PreH8 : (i >= 1)) (PreH9 : (n = (string_length (input)))) (PreH10 : (out = 0)) (PreH11 : (3 <= n)) (PreH12 : (n < INT_MAX)) (PreH13 : (0 <= i)) (PreH14 : (i <= (n - 2 ))) (PreH15 : (valid_string input )) (PreH16 : (all_ascii input )) (PreH17 : (problem_118_pre_z input )) (PreH18 : (ascii_range_z input )) (PreH19 : (alpha_codes_z_118 input )) (PreH20 : (no_candidate_after_z_118 input i )) ,
+  (CharArray.full word_pre ((string_length (input)) + 1 ) (c_string (input)) )
+  **  ((( &( "word" ) )) # Ptr  |-> word_pre)
+  **  ((( &( "n" ) )) # Int  |-> n)
+  **  ((( &( "out" ) )) # Ptr  |-> out)
+  **  ((( &( "cur" ) )) # Int  |-> (Znth i (c_string (input)) 0))
+  **  ((( &( "right" ) )) # Int  |-> (Znth (i + 1 ) (c_string (input)) 0))
+  **  ((( &( "left" ) )) # Int  |-> (Znth (i - 1 ) (c_string (input)) 0))
+  **  ((( &( "cur_vowel" ) )) # Int  |-> retval)
+  **  ((( &( "right_vowel" ) )) # Int  |-> retval_2)
+  **  ((( &( "left_vowel" ) )) # Int  |-> left_vowel)
+  **  ((( &( "i" ) )) # Int  |-> i)
+|--
+  “ False ”
+.
+
+Definition get_closest_vowel_safety_wit_29 := 
+forall (word_pre: Z) (input: (@list Z)) (i: Z) (out: Z) (n: Z) (retval: Z) (retval_2: Z) (retval_3: Z) (PreH1 : (retval_3 = 0)) (PreH2 : ~((is_vowel_z_118 (Znth (i - 1 ) (c_string (input)) 0) ))) (PreH3 : (retval_2 = 0)) (PreH4 : (retval_2 = 0)) (PreH5 : ~((is_vowel_z_118 (Znth (i + 1 ) (c_string (input)) 0) ))) (PreH6 : (retval = 1)) (PreH7 : (retval = 1)) (PreH8 : (is_vowel_z_118 (Znth i (c_string (input)) 0) )) (PreH9 : (0 <= ((string_length (input)) + 1 ))) (PreH10 : (i >= 1)) (PreH11 : (n = (string_length (input)))) (PreH12 : (out = 0)) (PreH13 : (3 <= n)) (PreH14 : (n < INT_MAX)) (PreH15 : (0 <= i)) (PreH16 : (i <= (n - 2 ))) (PreH17 : (valid_string input )) (PreH18 : (all_ascii input )) (PreH19 : (problem_118_pre_z input )) (PreH20 : (ascii_range_z input )) (PreH21 : (alpha_codes_z_118 input )) (PreH22 : (no_candidate_after_z_118 input i )) ,
+  (CharArray.full word_pre ((string_length (input)) + 1 ) (c_string (input)) )
+  **  ((( &( "word" ) )) # Ptr  |-> word_pre)
+  **  ((( &( "n" ) )) # Int  |-> n)
+  **  ((( &( "out" ) )) # Ptr  |-> out)
+  **  ((( &( "cur" ) )) # Int  |-> (Znth i (c_string (input)) 0))
+  **  ((( &( "right" ) )) # Int  |-> (Znth (i + 1 ) (c_string (input)) 0))
+  **  ((( &( "left" ) )) # Int  |-> (Znth (i - 1 ) (c_string (input)) 0))
+  **  ((( &( "cur_vowel" ) )) # Int  |-> retval)
+  **  ((( &( "right_vowel" ) )) # Int  |-> retval_2)
+  **  ((( &( "left_vowel" ) )) # Int  |-> retval_3)
+  **  ((( &( "i" ) )) # Int  |-> i)
+|--
+  “ (0 <= INT_MAX) ” 
+  &&  “ ((INT_MIN) <= 0) ”
+.
+
+Definition get_closest_vowel_safety_wit_30 := 
+forall (word_pre: Z) (input: (@list Z)) (i: Z) (out: Z) (n: Z) (retval: Z) (retval_2: Z) (retval_3: Z) (PreH1 : (retval_3 = 1)) (PreH2 : (is_vowel_z_118 (Znth (i - 1 ) (c_string (input)) 0) )) (PreH3 : (retval_2 = 0)) (PreH4 : (retval_2 = 0)) (PreH5 : ~((is_vowel_z_118 (Znth (i + 1 ) (c_string (input)) 0) ))) (PreH6 : (retval = 1)) (PreH7 : (retval = 1)) (PreH8 : (is_vowel_z_118 (Znth i (c_string (input)) 0) )) (PreH9 : (0 <= ((string_length (input)) + 1 ))) (PreH10 : (i >= 1)) (PreH11 : (n = (string_length (input)))) (PreH12 : (out = 0)) (PreH13 : (3 <= n)) (PreH14 : (n < INT_MAX)) (PreH15 : (0 <= i)) (PreH16 : (i <= (n - 2 ))) (PreH17 : (valid_string input )) (PreH18 : (all_ascii input )) (PreH19 : (problem_118_pre_z input )) (PreH20 : (ascii_range_z input )) (PreH21 : (alpha_codes_z_118 input )) (PreH22 : (no_candidate_after_z_118 input i )) ,
+  (CharArray.full word_pre ((string_length (input)) + 1 ) (c_string (input)) )
+  **  ((( &( "word" ) )) # Ptr  |-> word_pre)
+  **  ((( &( "n" ) )) # Int  |-> n)
+  **  ((( &( "out" ) )) # Ptr  |-> out)
+  **  ((( &( "cur" ) )) # Int  |-> (Znth i (c_string (input)) 0))
+  **  ((( &( "right" ) )) # Int  |-> (Znth (i + 1 ) (c_string (input)) 0))
+  **  ((( &( "left" ) )) # Int  |-> (Znth (i - 1 ) (c_string (input)) 0))
+  **  ((( &( "cur_vowel" ) )) # Int  |-> retval)
+  **  ((( &( "right_vowel" ) )) # Int  |-> retval_2)
+  **  ((( &( "left_vowel" ) )) # Int  |-> retval_3)
+  **  ((( &( "i" ) )) # Int  |-> i)
+|--
+  “ (0 <= INT_MAX) ” 
+  &&  “ ((INT_MIN) <= 0) ”
+.
+
+Definition get_closest_vowel_safety_wit_31 := 
+forall (word_pre: Z) (input: (@list Z)) (i: Z) (out: Z) (n: Z) (retval: Z) (retval_2: Z) (retval_3: Z) (PreH1 : (retval_3 <> 0)) (PreH2 : (retval_3 = 0)) (PreH3 : ~((is_vowel_z_118 (Znth (i - 1 ) (c_string (input)) 0) ))) (PreH4 : (retval_2 = 0)) (PreH5 : (retval_2 = 0)) (PreH6 : ~((is_vowel_z_118 (Znth (i + 1 ) (c_string (input)) 0) ))) (PreH7 : (retval = 1)) (PreH8 : (retval = 1)) (PreH9 : (is_vowel_z_118 (Znth i (c_string (input)) 0) )) (PreH10 : (0 <= ((string_length (input)) + 1 ))) (PreH11 : (i >= 1)) (PreH12 : (n = (string_length (input)))) (PreH13 : (out = 0)) (PreH14 : (3 <= n)) (PreH15 : (n < INT_MAX)) (PreH16 : (0 <= i)) (PreH17 : (i <= (n - 2 ))) (PreH18 : (valid_string input )) (PreH19 : (all_ascii input )) (PreH20 : (problem_118_pre_z input )) (PreH21 : (ascii_range_z input )) (PreH22 : (alpha_codes_z_118 input )) (PreH23 : (no_candidate_after_z_118 input i )) ,
+  (CharArray.full word_pre ((string_length (input)) + 1 ) (c_string (input)) )
+  **  ((( &( "word" ) )) # Ptr  |-> word_pre)
+  **  ((( &( "n" ) )) # Int  |-> n)
+  **  ((( &( "out" ) )) # Ptr  |-> out)
+  **  ((( &( "cur" ) )) # Int  |-> (Znth i (c_string (input)) 0))
+  **  ((( &( "right" ) )) # Int  |-> (Znth (i + 1 ) (c_string (input)) 0))
+  **  ((( &( "left" ) )) # Int  |-> (Znth (i - 1 ) (c_string (input)) 0))
+  **  ((( &( "cur_vowel" ) )) # Int  |-> retval)
+  **  ((( &( "right_vowel" ) )) # Int  |-> retval_2)
+  **  ((( &( "left_vowel" ) )) # Int  |-> retval_3)
+  **  ((( &( "i" ) )) # Int  |-> i)
+|--
+  “ False ”
+.
+
+Definition get_closest_vowel_safety_wit_32 := 
+forall (word_pre: Z) (input: (@list Z)) (i: Z) (out: Z) (n: Z) (retval: Z) (retval_2: Z) (retval_3: Z) (PreH1 : (retval_3 = 0)) (PreH2 : (retval_3 = 1)) (PreH3 : (is_vowel_z_118 (Znth (i - 1 ) (c_string (input)) 0) )) (PreH4 : (retval_2 = 0)) (PreH5 : (retval_2 = 0)) (PreH6 : ~((is_vowel_z_118 (Znth (i + 1 ) (c_string (input)) 0) ))) (PreH7 : (retval = 1)) (PreH8 : (retval = 1)) (PreH9 : (is_vowel_z_118 (Znth i (c_string (input)) 0) )) (PreH10 : (0 <= ((string_length (input)) + 1 ))) (PreH11 : (i >= 1)) (PreH12 : (n = (string_length (input)))) (PreH13 : (out = 0)) (PreH14 : (3 <= n)) (PreH15 : (n < INT_MAX)) (PreH16 : (0 <= i)) (PreH17 : (i <= (n - 2 ))) (PreH18 : (valid_string input )) (PreH19 : (all_ascii input )) (PreH20 : (problem_118_pre_z input )) (PreH21 : (ascii_range_z input )) (PreH22 : (alpha_codes_z_118 input )) (PreH23 : (no_candidate_after_z_118 input i )) ,
+  (CharArray.full word_pre ((string_length (input)) + 1 ) (c_string (input)) )
+  **  ((( &( "word" ) )) # Ptr  |-> word_pre)
+  **  ((( &( "n" ) )) # Int  |-> n)
+  **  ((( &( "out" ) )) # Ptr  |-> out)
+  **  ((( &( "cur" ) )) # Int  |-> (Znth i (c_string (input)) 0))
+  **  ((( &( "right" ) )) # Int  |-> (Znth (i + 1 ) (c_string (input)) 0))
+  **  ((( &( "left" ) )) # Int  |-> (Znth (i - 1 ) (c_string (input)) 0))
+  **  ((( &( "cur_vowel" ) )) # Int  |-> retval)
+  **  ((( &( "right_vowel" ) )) # Int  |-> retval_2)
+  **  ((( &( "left_vowel" ) )) # Int  |-> retval_3)
+  **  ((( &( "i" ) )) # Int  |-> i)
+|--
+  “ False ”
+.
+
+Definition get_closest_vowel_safety_wit_33 := 
+forall (word_pre: Z) (input: (@list Z)) (n: Z) (out: Z) (cur: Z) (i: Z) (right: Z) (left: Z) (cur_vowel: Z) (right_vowel: Z) (left_vowel: Z) (PreH1 : (n = (string_length (input)))) (PreH2 : (out = 0)) (PreH3 : (cur = (Znth (i) (input) (0)))) (PreH4 : (3 <= n)) (PreH5 : (n < INT_MAX)) (PreH6 : (1 <= i)) (PreH7 : (i <= (n - 2 ))) (PreH8 : (valid_string input )) (PreH9 : (all_ascii input )) (PreH10 : (problem_118_pre_z input )) (PreH11 : (ascii_range_z input )) (PreH12 : (alpha_codes_z_118 input )) (PreH13 : (closest_vowel_candidate_z_118 input i )) (PreH14 : (no_candidate_after_z_118 input i )) ,
+  ((( &( "word" ) )) # Ptr  |-> word_pre)
+  **  ((( &( "n" ) )) # Int  |-> n)
+  **  ((( &( "out" ) )) # Ptr  |-> out)
+  **  ((( &( "cur" ) )) # Int  |-> cur)
+  **  ((( &( "i" ) )) # Int  |-> i)
+  **  ((( &( "right" ) )) # Int  |-> right)
+  **  ((( &( "left" ) )) # Int  |-> left)
+  **  ((( &( "cur_vowel" ) )) # Int  |-> cur_vowel)
+  **  ((( &( "right_vowel" ) )) # Int  |-> right_vowel)
+  **  ((( &( "left_vowel" ) )) # Int  |-> left_vowel)
+  **  (store_string word_pre input )
+|--
+  “ (2 <= INT_MAX) ” 
+  &&  “ ((INT_MIN) <= 2) ”
+.
+
+Definition get_closest_vowel_safety_wit_34 := 
+forall (word_pre: Z) (input: (@list Z)) (n: Z) (out: Z) (cur: Z) (i: Z) (right: Z) (left: Z) (cur_vowel: Z) (right_vowel: Z) (left_vowel: Z) (retval: Z) (PreH1 : (retval <> 0)) (PreH2 : (0 <= ((string_length (input)) + 1 ))) (PreH3 : (n = (string_length (input)))) (PreH4 : (out = 0)) (PreH5 : (cur = (Znth (i) (input) (0)))) (PreH6 : (3 <= n)) (PreH7 : (n < INT_MAX)) (PreH8 : (1 <= i)) (PreH9 : (i <= (n - 2 ))) (PreH10 : (valid_string input )) (PreH11 : (all_ascii input )) (PreH12 : (problem_118_pre_z input )) (PreH13 : (ascii_range_z input )) (PreH14 : (alpha_codes_z_118 input )) (PreH15 : (closest_vowel_candidate_z_118 input i )) (PreH16 : (no_candidate_after_z_118 input i )) ,
+  (CharArray.undef_full retval 2 )
+  **  (CharArray.full word_pre ((string_length (input)) + 1 ) (c_string (input)) )
+  **  ((( &( "word" ) )) # Ptr  |-> word_pre)
+  **  ((( &( "n" ) )) # Int  |-> n)
+  **  ((( &( "out" ) )) # Ptr  |-> retval)
+  **  ((( &( "cur" ) )) # Int  |-> cur)
+  **  ((( &( "i" ) )) # Int  |-> i)
+  **  ((( &( "right" ) )) # Int  |-> right)
+  **  ((( &( "left" ) )) # Int  |-> left)
+  **  ((( &( "cur_vowel" ) )) # Int  |-> cur_vowel)
+  **  ((( &( "right_vowel" ) )) # Int  |-> right_vowel)
+  **  ((( &( "left_vowel" ) )) # Int  |-> left_vowel)
+|--
+  “ (0 <= INT_MAX) ” 
+  &&  “ ((INT_MIN) <= 0) ”
+.
+
+Definition get_closest_vowel_safety_wit_35 := 
+forall (word_pre: Z) (input: (@list Z)) (n: Z) (out: Z) (cur: Z) (i: Z) (right: Z) (left: Z) (cur_vowel: Z) (right_vowel: Z) (left_vowel: Z) (retval: Z) (PreH1 : (retval = 0)) (PreH2 : (retval <> 0)) (PreH3 : (0 <= ((string_length (input)) + 1 ))) (PreH4 : (n = (string_length (input)))) (PreH5 : (out = 0)) (PreH6 : (cur = (Znth (i) (input) (0)))) (PreH7 : (3 <= n)) (PreH8 : (n < INT_MAX)) (PreH9 : (1 <= i)) (PreH10 : (i <= (n - 2 ))) (PreH11 : (valid_string input )) (PreH12 : (all_ascii input )) (PreH13 : (problem_118_pre_z input )) (PreH14 : (ascii_range_z input )) (PreH15 : (alpha_codes_z_118 input )) (PreH16 : (closest_vowel_candidate_z_118 input i )) (PreH17 : (no_candidate_after_z_118 input i )) ,
+  (CharArray.undef_full retval 2 )
+  **  (CharArray.full word_pre ((string_length (input)) + 1 ) (c_string (input)) )
+  **  ((( &( "word" ) )) # Ptr  |-> word_pre)
+  **  ((( &( "n" ) )) # Int  |-> n)
+  **  ((( &( "out" ) )) # Ptr  |-> retval)
+  **  ((( &( "cur" ) )) # Int  |-> cur)
+  **  ((( &( "i" ) )) # Int  |-> i)
+  **  ((( &( "right" ) )) # Int  |-> right)
+  **  ((( &( "left" ) )) # Int  |-> left)
+  **  ((( &( "cur_vowel" ) )) # Int  |-> cur_vowel)
+  **  ((( &( "right_vowel" ) )) # Int  |-> right_vowel)
+  **  ((( &( "left_vowel" ) )) # Int  |-> left_vowel)
+|--
+  “ False ”
+.
+
+Definition get_closest_vowel_safety_wit_36 := 
+forall (word_pre: Z) (input: (@list Z)) (n: Z) (out: Z) (cur: Z) (i: Z) (right: Z) (left: Z) (cur_vowel: Z) (right_vowel: Z) (left_vowel: Z) (retval: Z) (PreH1 : (retval <> 0)) (PreH2 : (retval <> 0)) (PreH3 : (0 <= ((string_length (input)) + 1 ))) (PreH4 : (n = (string_length (input)))) (PreH5 : (out = 0)) (PreH6 : (cur = (Znth (i) (input) (0)))) (PreH7 : (3 <= n)) (PreH8 : (n < INT_MAX)) (PreH9 : (1 <= i)) (PreH10 : (i <= (n - 2 ))) (PreH11 : (valid_string input )) (PreH12 : (all_ascii input )) (PreH13 : (problem_118_pre_z input )) (PreH14 : (ascii_range_z input )) (PreH15 : (alpha_codes_z_118 input )) (PreH16 : (closest_vowel_candidate_z_118 input i )) (PreH17 : (no_candidate_after_z_118 input i )) ,
+  (CharArray.undef_full retval 2 )
+  **  (CharArray.full word_pre ((string_length (input)) + 1 ) (c_string (input)) )
+  **  ((( &( "word" ) )) # Ptr  |-> word_pre)
+  **  ((( &( "n" ) )) # Int  |-> n)
+  **  ((( &( "out" ) )) # Ptr  |-> retval)
+  **  ((( &( "cur" ) )) # Int  |-> cur)
+  **  ((( &( "i" ) )) # Int  |-> i)
+  **  ((( &( "right" ) )) # Int  |-> right)
+  **  ((( &( "left" ) )) # Int  |-> left)
+  **  ((( &( "cur_vowel" ) )) # Int  |-> cur_vowel)
+  **  ((( &( "right_vowel" ) )) # Int  |-> right_vowel)
+  **  ((( &( "left_vowel" ) )) # Int  |-> left_vowel)
+|--
+  “ (0 <= INT_MAX) ” 
+  &&  “ ((INT_MIN) <= 0) ”
+.
+
+Definition get_closest_vowel_safety_wit_37 := 
+forall (word_pre: Z) (input: (@list Z)) (n: Z) (out: Z) (cur: Z) (i: Z) (right: Z) (left: Z) (cur_vowel: Z) (right_vowel: Z) (left_vowel: Z) (retval: Z) (PreH1 : (retval <> 0)) (PreH2 : (retval <> 0)) (PreH3 : (0 <= ((string_length (input)) + 1 ))) (PreH4 : (n = (string_length (input)))) (PreH5 : (out = 0)) (PreH6 : (cur = (Znth (i) (input) (0)))) (PreH7 : (3 <= n)) (PreH8 : (n < INT_MAX)) (PreH9 : (1 <= i)) (PreH10 : (i <= (n - 2 ))) (PreH11 : (valid_string input )) (PreH12 : (all_ascii input )) (PreH13 : (problem_118_pre_z input )) (PreH14 : (ascii_range_z input )) (PreH15 : (alpha_codes_z_118 input )) (PreH16 : (closest_vowel_candidate_z_118 input i )) (PreH17 : (no_candidate_after_z_118 input i )) ,
+  (CharArray.undef_seg retval (0 + 1 ) 2 )
+  **  (((retval + (0 * sizeof(CHAR) ) )) # Char  |-> (signed_last_nbits (cur) (8)))
+  **  (CharArray.full word_pre ((string_length (input)) + 1 ) (c_string (input)) )
+  **  ((( &( "word" ) )) # Ptr  |-> word_pre)
+  **  ((( &( "n" ) )) # Int  |-> n)
+  **  ((( &( "out" ) )) # Ptr  |-> retval)
+  **  ((( &( "cur" ) )) # Int  |-> cur)
+  **  ((( &( "i" ) )) # Int  |-> i)
+  **  ((( &( "right" ) )) # Int  |-> right)
+  **  ((( &( "left" ) )) # Int  |-> left)
+  **  ((( &( "cur_vowel" ) )) # Int  |-> cur_vowel)
+  **  ((( &( "right_vowel" ) )) # Int  |-> right_vowel)
+  **  ((( &( "left_vowel" ) )) # Int  |-> left_vowel)
+|--
+  “ (1 <= INT_MAX) ” 
+  &&  “ ((INT_MIN) <= 1) ”
+.
+
+Definition get_closest_vowel_safety_wit_38 := 
+forall (word_pre: Z) (input: (@list Z)) (n: Z) (out: Z) (cur: Z) (i: Z) (right: Z) (left: Z) (cur_vowel: Z) (right_vowel: Z) (left_vowel: Z) (retval: Z) (PreH1 : (retval <> 0)) (PreH2 : (retval <> 0)) (PreH3 : (0 <= ((string_length (input)) + 1 ))) (PreH4 : (n = (string_length (input)))) (PreH5 : (out = 0)) (PreH6 : (cur = (Znth (i) (input) (0)))) (PreH7 : (3 <= n)) (PreH8 : (n < INT_MAX)) (PreH9 : (1 <= i)) (PreH10 : (i <= (n - 2 ))) (PreH11 : (valid_string input )) (PreH12 : (all_ascii input )) (PreH13 : (problem_118_pre_z input )) (PreH14 : (ascii_range_z input )) (PreH15 : (alpha_codes_z_118 input )) (PreH16 : (closest_vowel_candidate_z_118 input i )) (PreH17 : (no_candidate_after_z_118 input i )) ,
+  (CharArray.undef_seg retval (0 + 1 ) 2 )
+  **  (((retval + (0 * sizeof(CHAR) ) )) # Char  |-> (signed_last_nbits (cur) (8)))
+  **  (CharArray.full word_pre ((string_length (input)) + 1 ) (c_string (input)) )
+  **  ((( &( "word" ) )) # Ptr  |-> word_pre)
+  **  ((( &( "n" ) )) # Int  |-> n)
+  **  ((( &( "out" ) )) # Ptr  |-> retval)
+  **  ((( &( "cur" ) )) # Int  |-> cur)
+  **  ((( &( "i" ) )) # Int  |-> i)
+  **  ((( &( "right" ) )) # Int  |-> right)
+  **  ((( &( "left" ) )) # Int  |-> left)
+  **  ((( &( "cur_vowel" ) )) # Int  |-> cur_vowel)
+  **  ((( &( "right_vowel" ) )) # Int  |-> right_vowel)
+  **  ((( &( "left_vowel" ) )) # Int  |-> left_vowel)
+|--
+  “ (0 <= INT_MAX) ” 
+  &&  “ ((INT_MIN) <= 0) ”
+.
+
+Definition get_closest_vowel_safety_wit_39 := 
+forall (word_pre: Z) (input: (@list Z)) (n: Z) (out: Z) (cur: Z) (right: Z) (left: Z) (cur_vowel: Z) (right_vowel: Z) (left_vowel: Z) (i: Z) (PreH1 : (n = (string_length (input)))) (PreH2 : (out = 0)) (PreH3 : (3 <= n)) (PreH4 : (n < INT_MAX)) (PreH5 : (1 <= i)) (PreH6 : (i <= (n - 2 ))) (PreH7 : (valid_string input )) (PreH8 : (all_ascii input )) (PreH9 : (problem_118_pre_z input )) (PreH10 : (ascii_range_z input )) (PreH11 : (alpha_codes_z_118 input )) (PreH12 : ~((closest_vowel_candidate_z_118 input i ))) (PreH13 : (no_candidate_after_z_118 input i )) ,
+  ((( &( "word" ) )) # Ptr  |-> word_pre)
+  **  ((( &( "n" ) )) # Int  |-> n)
+  **  ((( &( "out" ) )) # Ptr  |-> out)
+  **  ((( &( "cur" ) )) # Int  |-> cur)
+  **  ((( &( "right" ) )) # Int  |-> right)
+  **  ((( &( "left" ) )) # Int  |-> left)
+  **  ((( &( "cur_vowel" ) )) # Int  |-> cur_vowel)
+  **  ((( &( "right_vowel" ) )) # Int  |-> right_vowel)
+  **  ((( &( "left_vowel" ) )) # Int  |-> left_vowel)
+  **  ((( &( "i" ) )) # Int  |-> i)
+  **  (store_string word_pre input )
+|--
+  “ ((i - 1 ) <= INT_MAX) ” 
+  &&  “ ((INT_MIN) <= (i - 1 )) ”
+.
+
+Definition get_closest_vowel_safety_wit_40 := 
+forall (word_pre: Z) (input: (@list Z)) (n: Z) (out: Z) (cur: Z) (right: Z) (left: Z) (cur_vowel: Z) (right_vowel: Z) (left_vowel: Z) (i: Z) (PreH1 : (n = (string_length (input)))) (PreH2 : (out = 0)) (PreH3 : (3 <= n)) (PreH4 : (n < INT_MAX)) (PreH5 : (1 <= i)) (PreH6 : (i <= (n - 2 ))) (PreH7 : (valid_string input )) (PreH8 : (all_ascii input )) (PreH9 : (problem_118_pre_z input )) (PreH10 : (ascii_range_z input )) (PreH11 : (alpha_codes_z_118 input )) (PreH12 : ~((closest_vowel_candidate_z_118 input i ))) (PreH13 : (no_candidate_after_z_118 input i )) ,
+  ((( &( "word" ) )) # Ptr  |-> word_pre)
+  **  ((( &( "n" ) )) # Int  |-> n)
+  **  ((( &( "out" ) )) # Ptr  |-> out)
+  **  ((( &( "cur" ) )) # Int  |-> cur)
+  **  ((( &( "right" ) )) # Int  |-> right)
+  **  ((( &( "left" ) )) # Int  |-> left)
+  **  ((( &( "cur_vowel" ) )) # Int  |-> cur_vowel)
+  **  ((( &( "right_vowel" ) )) # Int  |-> right_vowel)
+  **  ((( &( "left_vowel" ) )) # Int  |-> left_vowel)
+  **  ((( &( "i" ) )) # Int  |-> i)
+  **  (store_string word_pre input )
+|--
+  “ (1 <= INT_MAX) ” 
+  &&  “ ((INT_MIN) <= 1) ”
+.
+
+Definition get_closest_vowel_safety_wit_41 := 
+forall (word_pre: Z) (input: (@list Z)) (n: Z) (out: Z) (cur: Z) (right: Z) (left: Z) (cur_vowel: Z) (right_vowel: Z) (left_vowel: Z) (i: Z) (PreH1 : (n = (string_length (input)))) (PreH2 : (out = 0)) (PreH3 : (i = 0)) (PreH4 : (valid_string input )) (PreH5 : (all_ascii input )) (PreH6 : (problem_118_pre_z input )) (PreH7 : (ascii_range_z input )) (PreH8 : (alpha_codes_z_118 input )) (PreH9 : (no_candidate_after_z_118 input 0 )) ,
+  ((( &( "word" ) )) # Ptr  |-> word_pre)
+  **  ((( &( "n" ) )) # Int  |-> n)
+  **  ((( &( "out" ) )) # Ptr  |-> out)
+  **  ((( &( "cur" ) )) # Int  |-> cur)
+  **  ((( &( "right" ) )) # Int  |-> right)
+  **  ((( &( "left" ) )) # Int  |-> left)
+  **  ((( &( "cur_vowel" ) )) # Int  |-> cur_vowel)
+  **  ((( &( "right_vowel" ) )) # Int  |-> right_vowel)
+  **  ((( &( "left_vowel" ) )) # Int  |-> left_vowel)
+  **  ((( &( "i" ) )) # Int  |-> i)
+  **  (store_string word_pre input )
+|--
+  “ (1 <= INT_MAX) ” 
+  &&  “ ((INT_MIN) <= 1) ”
+.
+
+Definition get_closest_vowel_safety_wit_42 := 
+forall (word_pre: Z) (input: (@list Z)) (n: Z) (out: Z) (cur: Z) (right: Z) (left: Z) (cur_vowel: Z) (right_vowel: Z) (left_vowel: Z) (i: Z) (retval: Z) (PreH1 : (retval <> 0)) (PreH2 : (0 <= ((string_length (input)) + 1 ))) (PreH3 : (n = (string_length (input)))) (PreH4 : (out = 0)) (PreH5 : (i = 0)) (PreH6 : (valid_string input )) (PreH7 : (all_ascii input )) (PreH8 : (problem_118_pre_z input )) (PreH9 : (ascii_range_z input )) (PreH10 : (alpha_codes_z_118 input )) (PreH11 : (no_candidate_after_z_118 input 0 )) ,
+  (CharArray.undef_full retval 1 )
+  **  (CharArray.full word_pre ((string_length (input)) + 1 ) (c_string (input)) )
+  **  ((( &( "word" ) )) # Ptr  |-> word_pre)
+  **  ((( &( "n" ) )) # Int  |-> n)
+  **  ((( &( "out" ) )) # Ptr  |-> retval)
+  **  ((( &( "cur" ) )) # Int  |-> cur)
+  **  ((( &( "right" ) )) # Int  |-> right)
+  **  ((( &( "left" ) )) # Int  |-> left)
+  **  ((( &( "cur_vowel" ) )) # Int  |-> cur_vowel)
+  **  ((( &( "right_vowel" ) )) # Int  |-> right_vowel)
+  **  ((( &( "left_vowel" ) )) # Int  |-> left_vowel)
+  **  ((( &( "i" ) )) # Int  |-> i)
+|--
+  “ (0 <= INT_MAX) ” 
+  &&  “ ((INT_MIN) <= 0) ”
+.
+
+Definition get_closest_vowel_safety_wit_43 := 
+forall (word_pre: Z) (input: (@list Z)) (n: Z) (out: Z) (cur: Z) (right: Z) (left: Z) (cur_vowel: Z) (right_vowel: Z) (left_vowel: Z) (i: Z) (retval: Z) (PreH1 : (retval = 0)) (PreH2 : (retval <> 0)) (PreH3 : (0 <= ((string_length (input)) + 1 ))) (PreH4 : (n = (string_length (input)))) (PreH5 : (out = 0)) (PreH6 : (i = 0)) (PreH7 : (valid_string input )) (PreH8 : (all_ascii input )) (PreH9 : (problem_118_pre_z input )) (PreH10 : (ascii_range_z input )) (PreH11 : (alpha_codes_z_118 input )) (PreH12 : (no_candidate_after_z_118 input 0 )) ,
+  (CharArray.undef_full retval 1 )
+  **  (CharArray.full word_pre ((string_length (input)) + 1 ) (c_string (input)) )
+  **  ((( &( "word" ) )) # Ptr  |-> word_pre)
+  **  ((( &( "n" ) )) # Int  |-> n)
+  **  ((( &( "out" ) )) # Ptr  |-> retval)
+  **  ((( &( "cur" ) )) # Int  |-> cur)
+  **  ((( &( "right" ) )) # Int  |-> right)
+  **  ((( &( "left" ) )) # Int  |-> left)
+  **  ((( &( "cur_vowel" ) )) # Int  |-> cur_vowel)
+  **  ((( &( "right_vowel" ) )) # Int  |-> right_vowel)
+  **  ((( &( "left_vowel" ) )) # Int  |-> left_vowel)
+  **  ((( &( "i" ) )) # Int  |-> i)
+|--
+  “ False ”
+.
+
+Definition get_closest_vowel_safety_wit_44 := 
+forall (word_pre: Z) (input: (@list Z)) (n: Z) (out: Z) (cur: Z) (right: Z) (left: Z) (cur_vowel: Z) (right_vowel: Z) (left_vowel: Z) (i: Z) (retval: Z) (PreH1 : (retval <> 0)) (PreH2 : (retval <> 0)) (PreH3 : (0 <= ((string_length (input)) + 1 ))) (PreH4 : (n = (string_length (input)))) (PreH5 : (out = 0)) (PreH6 : (i = 0)) (PreH7 : (valid_string input )) (PreH8 : (all_ascii input )) (PreH9 : (problem_118_pre_z input )) (PreH10 : (ascii_range_z input )) (PreH11 : (alpha_codes_z_118 input )) (PreH12 : (no_candidate_after_z_118 input 0 )) ,
+  (CharArray.undef_full retval 1 )
+  **  (CharArray.full word_pre ((string_length (input)) + 1 ) (c_string (input)) )
+  **  ((( &( "word" ) )) # Ptr  |-> word_pre)
+  **  ((( &( "n" ) )) # Int  |-> n)
+  **  ((( &( "out" ) )) # Ptr  |-> retval)
+  **  ((( &( "cur" ) )) # Int  |-> cur)
+  **  ((( &( "right" ) )) # Int  |-> right)
+  **  ((( &( "left" ) )) # Int  |-> left)
+  **  ((( &( "cur_vowel" ) )) # Int  |-> cur_vowel)
+  **  ((( &( "right_vowel" ) )) # Int  |-> right_vowel)
+  **  ((( &( "left_vowel" ) )) # Int  |-> left_vowel)
+  **  ((( &( "i" ) )) # Int  |-> i)
+|--
+  “ (0 <= INT_MAX) ” 
+  &&  “ ((INT_MIN) <= 0) ”
+.
+
+Definition get_closest_vowel_safety_wit_45 := 
+forall (word_pre: Z) (input: (@list Z)) (n: Z) (out: Z) (cur: Z) (right: Z) (left: Z) (cur_vowel: Z) (right_vowel: Z) (left_vowel: Z) (i: Z) (retval: Z) (PreH1 : (retval <> 0)) (PreH2 : (retval <> 0)) (PreH3 : (0 <= ((string_length (input)) + 1 ))) (PreH4 : (n = (string_length (input)))) (PreH5 : (out = 0)) (PreH6 : (i = 0)) (PreH7 : (valid_string input )) (PreH8 : (all_ascii input )) (PreH9 : (problem_118_pre_z input )) (PreH10 : (ascii_range_z input )) (PreH11 : (alpha_codes_z_118 input )) (PreH12 : (no_candidate_after_z_118 input 0 )) ,
+  (CharArray.undef_full retval 1 )
+  **  (CharArray.full word_pre ((string_length (input)) + 1 ) (c_string (input)) )
+  **  ((( &( "word" ) )) # Ptr  |-> word_pre)
+  **  ((( &( "n" ) )) # Int  |-> n)
+  **  ((( &( "out" ) )) # Ptr  |-> retval)
+  **  ((( &( "cur" ) )) # Int  |-> cur)
+  **  ((( &( "right" ) )) # Int  |-> right)
+  **  ((( &( "left" ) )) # Int  |-> left)
+  **  ((( &( "cur_vowel" ) )) # Int  |-> cur_vowel)
+  **  ((( &( "right_vowel" ) )) # Int  |-> right_vowel)
+  **  ((( &( "left_vowel" ) )) # Int  |-> left_vowel)
+  **  ((( &( "i" ) )) # Int  |-> i)
+|--
+  “ (0 <= INT_MAX) ” 
+  &&  “ ((INT_MIN) <= 0) ”
+.
+
+Definition get_closest_vowel_entail_wit_1 := 
+(
+forall (word_pre: Z) (input: (@list Z)) (retval: Z) (PreH1 : (retval = (string_length (input)))) (PreH2 : (0 <= ((string_length (input)) + 1 ))) (PreH3 : (valid_string input )) (PreH4 : (all_ascii input )) (PreH5 : (problem_118_pre_z input )) (PreH6 : (ascii_range_z input )) (PreH7 : ((string_length (input)) < INT_MAX)) ,
+  (store_string word_pre input )
+|--
+  “ (retval = (string_length (input))) ” 
+  &&  “ (0 = 0) ” 
+  &&  “ (valid_string input ) ” 
+  &&  “ (all_ascii input ) ” 
+  &&  “ (problem_118_pre_z input ) ” 
+  &&  “ (ascii_range_z input ) ” 
+  &&  “ (alpha_codes_z_118 input ) ” 
+  &&  “ ((string_length (input)) < INT_MAX) ”
+  &&  (store_string word_pre input )
+) \/
+(
+forall (input: (@list Z)) (retval: Z) (PreH1 : (retval = (string_length (input)))) (PreH2 : (0 <= ((string_length (input)) + 1 ))) (PreH3 : (valid_string input )) (PreH4 : (all_ascii input )) (PreH5 : (problem_118_pre_z input )) (PreH6 : (ascii_range_z input )) (PreH7 : ((string_length (input)) < INT_MAX)) ,
+  TT && emp 
+|--
+  “ (alpha_codes_z_118 input ) ”
+  &&  emp
+).
+
+Definition get_closest_vowel_entail_wit_1_split_goal_1 := 
+forall (input: (@list Z)) (retval: Z) (PreH1 : (retval = (string_length (input)))) (PreH2 : (0 <= ((string_length (input)) + 1 ))) (PreH3 : (valid_string input )) (PreH4 : (all_ascii input )) (PreH5 : (problem_118_pre_z input )) (PreH6 : (ascii_range_z input )) (PreH7 : ((string_length (input)) < INT_MAX)) ,
+  TT && emp 
+|--
+  “ (alpha_codes_z_118 input ) ”
+.
+
+Definition get_closest_vowel_entail_wit_2 := 
+(
+forall (word_pre: Z) (input: (@list Z)) (n: Z) (out: Z) (PreH1 : (n >= 3)) (PreH2 : (n = (string_length (input)))) (PreH3 : (out = 0)) (PreH4 : (valid_string input )) (PreH5 : (all_ascii input )) (PreH6 : (problem_118_pre_z input )) (PreH7 : (ascii_range_z input )) (PreH8 : (alpha_codes_z_118 input )) (PreH9 : ((string_length (input)) < INT_MAX)) ,
+  (store_string word_pre input )
+|--
+  “ (n = (string_length (input))) ” 
+  &&  “ (out = 0) ” 
+  &&  “ (3 <= n) ” 
+  &&  “ (n < INT_MAX) ” 
+  &&  “ (0 <= (n - 2 )) ” 
+  &&  “ ((n - 2 ) <= (n - 2 )) ” 
+  &&  “ (valid_string input ) ” 
+  &&  “ (all_ascii input ) ” 
+  &&  “ (problem_118_pre_z input ) ” 
+  &&  “ (ascii_range_z input ) ” 
+  &&  “ (alpha_codes_z_118 input ) ” 
+  &&  “ (no_candidate_after_z_118 input (n - 2 ) ) ”
+  &&  (store_string word_pre input )
+) \/
+(
+forall (input: (@list Z)) (n: Z) (out: Z) (PreH1 : (0 <= ((string_length (input)) + 1 ))) (PreH2 : (n >= 3)) (PreH3 : (n = (string_length (input)))) (PreH4 : (out = 0)) (PreH5 : (valid_string input )) (PreH6 : (all_ascii input )) (PreH7 : (problem_118_pre_z input )) (PreH8 : (ascii_range_z input )) (PreH9 : (alpha_codes_z_118 input )) (PreH10 : ((string_length (input)) < INT_MAX)) ,
+  TT && emp 
+|--
+  “ (no_candidate_after_z_118 input (n - 2 ) ) ”
+  &&  emp
+).
+
+Definition get_closest_vowel_entail_wit_2_split_goal_1 := 
+forall (input: (@list Z)) (n: Z) (out: Z) (PreH1 : (0 <= ((string_length (input)) + 1 ))) (PreH2 : (n >= 3)) (PreH3 : (n = (string_length (input)))) (PreH4 : (out = 0)) (PreH5 : (valid_string input )) (PreH6 : (all_ascii input )) (PreH7 : (problem_118_pre_z input )) (PreH8 : (ascii_range_z input )) (PreH9 : (alpha_codes_z_118 input )) (PreH10 : ((string_length (input)) < INT_MAX)) ,
+  TT && emp 
+|--
+  “ (no_candidate_after_z_118 input (n - 2 ) ) ”
+.
+
+Definition get_closest_vowel_entail_wit_3 := 
+(
+forall (word_pre: Z) (input: (@list Z)) (i: Z) (out: Z) (n: Z) (retval: Z) (retval_2: Z) (retval_3: Z) (PreH1 : (retval_3 = 0)) (PreH2 : (retval_3 = 0)) (PreH3 : ~((is_vowel_z_118 (Znth (i - 1 ) (c_string (input)) 0) ))) (PreH4 : (retval_2 = 0)) (PreH5 : (retval_2 = 0)) (PreH6 : ~((is_vowel_z_118 (Znth (i + 1 ) (c_string (input)) 0) ))) (PreH7 : (retval = 1)) (PreH8 : (retval = 1)) (PreH9 : (is_vowel_z_118 (Znth i (c_string (input)) 0) )) (PreH10 : (0 <= ((string_length (input)) + 1 ))) (PreH11 : (i >= 1)) (PreH12 : (n = (string_length (input)))) (PreH13 : (out = 0)) (PreH14 : (3 <= n)) (PreH15 : (n < INT_MAX)) (PreH16 : (0 <= i)) (PreH17 : (i <= (n - 2 ))) (PreH18 : (valid_string input )) (PreH19 : (all_ascii input )) (PreH20 : (problem_118_pre_z input )) (PreH21 : (ascii_range_z input )) (PreH22 : (alpha_codes_z_118 input )) (PreH23 : (no_candidate_after_z_118 input i )) ,
+  (CharArray.full word_pre ((string_length (input)) + 1 ) (c_string (input)) )
+|--
+  “ (n = (string_length (input))) ” 
+  &&  “ (out = 0) ” 
+  &&  “ ((Znth i (c_string (input)) 0) = (Znth (i) (input) (0))) ” 
+  &&  “ (3 <= n) ” 
+  &&  “ (n < INT_MAX) ” 
+  &&  “ (1 <= i) ” 
+  &&  “ (i <= (n - 2 )) ” 
+  &&  “ (valid_string input ) ” 
+  &&  “ (all_ascii input ) ” 
+  &&  “ (problem_118_pre_z input ) ” 
+  &&  “ (ascii_range_z input ) ” 
+  &&  “ (alpha_codes_z_118 input ) ” 
+  &&  “ (closest_vowel_candidate_z_118 input i ) ” 
+  &&  “ (no_candidate_after_z_118 input i ) ”
+  &&  (store_string word_pre input )
+) \/
+(
+forall (input: (@list Z)) (i: Z) (out: Z) (n: Z) (retval: Z) (retval_2: Z) (retval_3: Z) (PreH1 : (retval_3 = 0)) (PreH2 : (retval_3 = 0)) (PreH3 : ~((is_vowel_z_118 (Znth (i - 1 ) (c_string (input)) 0) ))) (PreH4 : (retval_2 = 0)) (PreH5 : (retval_2 = 0)) (PreH6 : ~((is_vowel_z_118 (Znth (i + 1 ) (c_string (input)) 0) ))) (PreH7 : (retval = 1)) (PreH8 : (retval = 1)) (PreH9 : (is_vowel_z_118 (Znth i (c_string (input)) 0) )) (PreH10 : (0 <= ((string_length (input)) + 1 ))) (PreH11 : (i >= 1)) (PreH12 : (n = (string_length (input)))) (PreH13 : (out = 0)) (PreH14 : (3 <= n)) (PreH15 : (n < INT_MAX)) (PreH16 : (0 <= i)) (PreH17 : (i <= (n - 2 ))) (PreH18 : (valid_string input )) (PreH19 : (all_ascii input )) (PreH20 : (problem_118_pre_z input )) (PreH21 : (ascii_range_z input )) (PreH22 : (alpha_codes_z_118 input )) (PreH23 : (no_candidate_after_z_118 input i )) ,
+  TT && emp 
+|--
+  “ (closest_vowel_candidate_z_118 input i ) ” 
+  &&  “ ((Znth i (c_string (input)) 0) = (Znth (i) (input) (0))) ”
+  &&  emp
+).
+
+Definition get_closest_vowel_entail_wit_3_split_goal_1 := 
+forall (input: (@list Z)) (i: Z) (out: Z) (n: Z) (retval: Z) (retval_2: Z) (retval_3: Z) (PreH1 : (retval_3 = 0)) (PreH2 : (retval_3 = 0)) (PreH3 : ~((is_vowel_z_118 (Znth (i - 1 ) (c_string (input)) 0) ))) (PreH4 : (retval_2 = 0)) (PreH5 : (retval_2 = 0)) (PreH6 : ~((is_vowel_z_118 (Znth (i + 1 ) (c_string (input)) 0) ))) (PreH7 : (retval = 1)) (PreH8 : (retval = 1)) (PreH9 : (is_vowel_z_118 (Znth i (c_string (input)) 0) )) (PreH10 : (0 <= ((string_length (input)) + 1 ))) (PreH11 : (i >= 1)) (PreH12 : (n = (string_length (input)))) (PreH13 : (out = 0)) (PreH14 : (3 <= n)) (PreH15 : (n < INT_MAX)) (PreH16 : (0 <= i)) (PreH17 : (i <= (n - 2 ))) (PreH18 : (valid_string input )) (PreH19 : (all_ascii input )) (PreH20 : (problem_118_pre_z input )) (PreH21 : (ascii_range_z input )) (PreH22 : (alpha_codes_z_118 input )) (PreH23 : (no_candidate_after_z_118 input i )) ,
+  TT && emp 
+|--
+  “ (closest_vowel_candidate_z_118 input i ) ”
+.
+
+Definition get_closest_vowel_entail_wit_3_split_goal_2 := 
+forall (input: (@list Z)) (i: Z) (out: Z) (n: Z) (retval: Z) (retval_2: Z) (retval_3: Z) (PreH1 : (retval_3 = 0)) (PreH2 : (retval_3 = 0)) (PreH3 : ~((is_vowel_z_118 (Znth (i - 1 ) (c_string (input)) 0) ))) (PreH4 : (retval_2 = 0)) (PreH5 : (retval_2 = 0)) (PreH6 : ~((is_vowel_z_118 (Znth (i + 1 ) (c_string (input)) 0) ))) (PreH7 : (retval = 1)) (PreH8 : (retval = 1)) (PreH9 : (is_vowel_z_118 (Znth i (c_string (input)) 0) )) (PreH10 : (0 <= ((string_length (input)) + 1 ))) (PreH11 : (i >= 1)) (PreH12 : (n = (string_length (input)))) (PreH13 : (out = 0)) (PreH14 : (3 <= n)) (PreH15 : (n < INT_MAX)) (PreH16 : (0 <= i)) (PreH17 : (i <= (n - 2 ))) (PreH18 : (valid_string input )) (PreH19 : (all_ascii input )) (PreH20 : (problem_118_pre_z input )) (PreH21 : (ascii_range_z input )) (PreH22 : (alpha_codes_z_118 input )) (PreH23 : (no_candidate_after_z_118 input i )) ,
+  TT && emp 
+|--
+  “ ((Znth i (c_string (input)) 0) = (Znth (i) (input) (0))) ”
+.
+
+Definition get_closest_vowel_entail_wit_4_1 := 
+(
+forall (word_pre: Z) (input: (@list Z)) (i: Z) (out: Z) (n: Z) (retval: Z) (PreH1 : (retval <> 1)) (PreH2 : (retval = 0)) (PreH3 : ~((is_vowel_z_118 (Znth i (c_string (input)) 0) ))) (PreH4 : (0 <= ((string_length (input)) + 1 ))) (PreH5 : (i >= 1)) (PreH6 : (n = (string_length (input)))) (PreH7 : (out = 0)) (PreH8 : (3 <= n)) (PreH9 : (n < INT_MAX)) (PreH10 : (0 <= i)) (PreH11 : (i <= (n - 2 ))) (PreH12 : (valid_string input )) (PreH13 : (all_ascii input )) (PreH14 : (problem_118_pre_z input )) (PreH15 : (ascii_range_z input )) (PreH16 : (alpha_codes_z_118 input )) (PreH17 : (no_candidate_after_z_118 input i )) ,
+  (CharArray.full word_pre ((string_length (input)) + 1 ) (c_string (input)) )
+|--
+  “ (n = (string_length (input))) ” 
+  &&  “ (out = 0) ” 
+  &&  “ (3 <= n) ” 
+  &&  “ (n < INT_MAX) ” 
+  &&  “ (1 <= i) ” 
+  &&  “ (i <= (n - 2 )) ” 
+  &&  “ (valid_string input ) ” 
+  &&  “ (all_ascii input ) ” 
+  &&  “ (problem_118_pre_z input ) ” 
+  &&  “ (ascii_range_z input ) ” 
+  &&  “ (alpha_codes_z_118 input ) ” 
+  &&  “ ~((closest_vowel_candidate_z_118 input i )) ” 
+  &&  “ (no_candidate_after_z_118 input i ) ”
+  &&  (store_string word_pre input )
+) \/
+(
+forall (input: (@list Z)) (i: Z) (out: Z) (n: Z) (retval: Z) (PreH1 : (retval <> 1)) (PreH2 : (retval = 0)) (PreH3 : ~((is_vowel_z_118 (Znth i (c_string (input)) 0) ))) (PreH4 : (0 <= ((string_length (input)) + 1 ))) (PreH5 : (i >= 1)) (PreH6 : (n = (string_length (input)))) (PreH7 : (out = 0)) (PreH8 : (3 <= n)) (PreH9 : (n < INT_MAX)) (PreH10 : (0 <= i)) (PreH11 : (i <= (n - 2 ))) (PreH12 : (valid_string input )) (PreH13 : (all_ascii input )) (PreH14 : (problem_118_pre_z input )) (PreH15 : (ascii_range_z input )) (PreH16 : (alpha_codes_z_118 input )) (PreH17 : (no_candidate_after_z_118 input i )) ,
+  TT && emp 
+|--
+  “ ~((closest_vowel_candidate_z_118 input i )) ”
+  &&  emp
+).
+
+Definition get_closest_vowel_entail_wit_4_1_split_goal_1 := 
+forall (input: (@list Z)) (i: Z) (out: Z) (n: Z) (retval: Z) (PreH1 : (retval <> 1)) (PreH2 : (retval = 0)) (PreH3 : ~((is_vowel_z_118 (Znth i (c_string (input)) 0) ))) (PreH4 : (0 <= ((string_length (input)) + 1 ))) (PreH5 : (i >= 1)) (PreH6 : (n = (string_length (input)))) (PreH7 : (out = 0)) (PreH8 : (3 <= n)) (PreH9 : (n < INT_MAX)) (PreH10 : (0 <= i)) (PreH11 : (i <= (n - 2 ))) (PreH12 : (valid_string input )) (PreH13 : (all_ascii input )) (PreH14 : (problem_118_pre_z input )) (PreH15 : (ascii_range_z input )) (PreH16 : (alpha_codes_z_118 input )) (PreH17 : (no_candidate_after_z_118 input i )) ,
+  TT && emp 
+|--
+  “ ~((closest_vowel_candidate_z_118 input i )) ”
+.
+
+Definition get_closest_vowel_entail_wit_4_2 := 
+(
+forall (word_pre: Z) (input: (@list Z)) (i: Z) (out: Z) (n: Z) (retval: Z) (retval_2: Z) (PreH1 : (retval_2 <> 0)) (PreH2 : (retval_2 = 1)) (PreH3 : (is_vowel_z_118 (Znth (i + 1 ) (c_string (input)) 0) )) (PreH4 : (retval = 1)) (PreH5 : (retval = 1)) (PreH6 : (is_vowel_z_118 (Znth i (c_string (input)) 0) )) (PreH7 : (0 <= ((string_length (input)) + 1 ))) (PreH8 : (i >= 1)) (PreH9 : (n = (string_length (input)))) (PreH10 : (out = 0)) (PreH11 : (3 <= n)) (PreH12 : (n < INT_MAX)) (PreH13 : (0 <= i)) (PreH14 : (i <= (n - 2 ))) (PreH15 : (valid_string input )) (PreH16 : (all_ascii input )) (PreH17 : (problem_118_pre_z input )) (PreH18 : (ascii_range_z input )) (PreH19 : (alpha_codes_z_118 input )) (PreH20 : (no_candidate_after_z_118 input i )) ,
+  (CharArray.full word_pre ((string_length (input)) + 1 ) (c_string (input)) )
+|--
+  “ (n = (string_length (input))) ” 
+  &&  “ (out = 0) ” 
+  &&  “ (3 <= n) ” 
+  &&  “ (n < INT_MAX) ” 
+  &&  “ (1 <= i) ” 
+  &&  “ (i <= (n - 2 )) ” 
+  &&  “ (valid_string input ) ” 
+  &&  “ (all_ascii input ) ” 
+  &&  “ (problem_118_pre_z input ) ” 
+  &&  “ (ascii_range_z input ) ” 
+  &&  “ (alpha_codes_z_118 input ) ” 
+  &&  “ ~((closest_vowel_candidate_z_118 input i )) ” 
+  &&  “ (no_candidate_after_z_118 input i ) ”
+  &&  (store_string word_pre input )
+) \/
+(
+forall (input: (@list Z)) (i: Z) (out: Z) (n: Z) (retval: Z) (retval_2: Z) (PreH1 : (retval_2 <> 0)) (PreH2 : (retval_2 = 1)) (PreH3 : (is_vowel_z_118 (Znth (i + 1 ) (c_string (input)) 0) )) (PreH4 : (retval = 1)) (PreH5 : (retval = 1)) (PreH6 : (is_vowel_z_118 (Znth i (c_string (input)) 0) )) (PreH7 : (0 <= ((string_length (input)) + 1 ))) (PreH8 : (i >= 1)) (PreH9 : (n = (string_length (input)))) (PreH10 : (out = 0)) (PreH11 : (3 <= n)) (PreH12 : (n < INT_MAX)) (PreH13 : (0 <= i)) (PreH14 : (i <= (n - 2 ))) (PreH15 : (valid_string input )) (PreH16 : (all_ascii input )) (PreH17 : (problem_118_pre_z input )) (PreH18 : (ascii_range_z input )) (PreH19 : (alpha_codes_z_118 input )) (PreH20 : (no_candidate_after_z_118 input i )) ,
+  TT && emp 
+|--
+  “ ~((closest_vowel_candidate_z_118 input i )) ”
+  &&  emp
+).
+
+Definition get_closest_vowel_entail_wit_4_2_split_goal_1 := 
+forall (input: (@list Z)) (i: Z) (out: Z) (n: Z) (retval: Z) (retval_2: Z) (PreH1 : (retval_2 <> 0)) (PreH2 : (retval_2 = 1)) (PreH3 : (is_vowel_z_118 (Znth (i + 1 ) (c_string (input)) 0) )) (PreH4 : (retval = 1)) (PreH5 : (retval = 1)) (PreH6 : (is_vowel_z_118 (Znth i (c_string (input)) 0) )) (PreH7 : (0 <= ((string_length (input)) + 1 ))) (PreH8 : (i >= 1)) (PreH9 : (n = (string_length (input)))) (PreH10 : (out = 0)) (PreH11 : (3 <= n)) (PreH12 : (n < INT_MAX)) (PreH13 : (0 <= i)) (PreH14 : (i <= (n - 2 ))) (PreH15 : (valid_string input )) (PreH16 : (all_ascii input )) (PreH17 : (problem_118_pre_z input )) (PreH18 : (ascii_range_z input )) (PreH19 : (alpha_codes_z_118 input )) (PreH20 : (no_candidate_after_z_118 input i )) ,
+  TT && emp 
+|--
+  “ ~((closest_vowel_candidate_z_118 input i )) ”
+.
+
+Definition get_closest_vowel_entail_wit_4_3 := 
+(
+forall (word_pre: Z) (input: (@list Z)) (i: Z) (out: Z) (n: Z) (retval: Z) (retval_2: Z) (retval_3: Z) (PreH1 : (retval_3 <> 0)) (PreH2 : (retval_3 = 1)) (PreH3 : (is_vowel_z_118 (Znth (i - 1 ) (c_string (input)) 0) )) (PreH4 : (retval_2 = 0)) (PreH5 : (retval_2 = 0)) (PreH6 : ~((is_vowel_z_118 (Znth (i + 1 ) (c_string (input)) 0) ))) (PreH7 : (retval = 1)) (PreH8 : (retval = 1)) (PreH9 : (is_vowel_z_118 (Znth i (c_string (input)) 0) )) (PreH10 : (0 <= ((string_length (input)) + 1 ))) (PreH11 : (i >= 1)) (PreH12 : (n = (string_length (input)))) (PreH13 : (out = 0)) (PreH14 : (3 <= n)) (PreH15 : (n < INT_MAX)) (PreH16 : (0 <= i)) (PreH17 : (i <= (n - 2 ))) (PreH18 : (valid_string input )) (PreH19 : (all_ascii input )) (PreH20 : (problem_118_pre_z input )) (PreH21 : (ascii_range_z input )) (PreH22 : (alpha_codes_z_118 input )) (PreH23 : (no_candidate_after_z_118 input i )) ,
+  (CharArray.full word_pre ((string_length (input)) + 1 ) (c_string (input)) )
+|--
+  “ (n = (string_length (input))) ” 
+  &&  “ (out = 0) ” 
+  &&  “ (3 <= n) ” 
+  &&  “ (n < INT_MAX) ” 
+  &&  “ (1 <= i) ” 
+  &&  “ (i <= (n - 2 )) ” 
+  &&  “ (valid_string input ) ” 
+  &&  “ (all_ascii input ) ” 
+  &&  “ (problem_118_pre_z input ) ” 
+  &&  “ (ascii_range_z input ) ” 
+  &&  “ (alpha_codes_z_118 input ) ” 
+  &&  “ ~((closest_vowel_candidate_z_118 input i )) ” 
+  &&  “ (no_candidate_after_z_118 input i ) ”
+  &&  (store_string word_pre input )
+) \/
+(
+forall (input: (@list Z)) (i: Z) (out: Z) (n: Z) (retval: Z) (retval_2: Z) (retval_3: Z) (PreH1 : (retval_3 <> 0)) (PreH2 : (retval_3 = 1)) (PreH3 : (is_vowel_z_118 (Znth (i - 1 ) (c_string (input)) 0) )) (PreH4 : (retval_2 = 0)) (PreH5 : (retval_2 = 0)) (PreH6 : ~((is_vowel_z_118 (Znth (i + 1 ) (c_string (input)) 0) ))) (PreH7 : (retval = 1)) (PreH8 : (retval = 1)) (PreH9 : (is_vowel_z_118 (Znth i (c_string (input)) 0) )) (PreH10 : (0 <= ((string_length (input)) + 1 ))) (PreH11 : (i >= 1)) (PreH12 : (n = (string_length (input)))) (PreH13 : (out = 0)) (PreH14 : (3 <= n)) (PreH15 : (n < INT_MAX)) (PreH16 : (0 <= i)) (PreH17 : (i <= (n - 2 ))) (PreH18 : (valid_string input )) (PreH19 : (all_ascii input )) (PreH20 : (problem_118_pre_z input )) (PreH21 : (ascii_range_z input )) (PreH22 : (alpha_codes_z_118 input )) (PreH23 : (no_candidate_after_z_118 input i )) ,
+  TT && emp 
+|--
+  “ ~((closest_vowel_candidate_z_118 input i )) ”
+  &&  emp
+).
+
+Definition get_closest_vowel_entail_wit_4_3_split_goal_1 := 
+forall (input: (@list Z)) (i: Z) (out: Z) (n: Z) (retval: Z) (retval_2: Z) (retval_3: Z) (PreH1 : (retval_3 <> 0)) (PreH2 : (retval_3 = 1)) (PreH3 : (is_vowel_z_118 (Znth (i - 1 ) (c_string (input)) 0) )) (PreH4 : (retval_2 = 0)) (PreH5 : (retval_2 = 0)) (PreH6 : ~((is_vowel_z_118 (Znth (i + 1 ) (c_string (input)) 0) ))) (PreH7 : (retval = 1)) (PreH8 : (retval = 1)) (PreH9 : (is_vowel_z_118 (Znth i (c_string (input)) 0) )) (PreH10 : (0 <= ((string_length (input)) + 1 ))) (PreH11 : (i >= 1)) (PreH12 : (n = (string_length (input)))) (PreH13 : (out = 0)) (PreH14 : (3 <= n)) (PreH15 : (n < INT_MAX)) (PreH16 : (0 <= i)) (PreH17 : (i <= (n - 2 ))) (PreH18 : (valid_string input )) (PreH19 : (all_ascii input )) (PreH20 : (problem_118_pre_z input )) (PreH21 : (ascii_range_z input )) (PreH22 : (alpha_codes_z_118 input )) (PreH23 : (no_candidate_after_z_118 input i )) ,
+  TT && emp 
+|--
+  “ ~((closest_vowel_candidate_z_118 input i )) ”
+.
+
+Definition get_closest_vowel_entail_wit_5 := 
+(
+forall (word_pre: Z) (input: (@list Z)) (n: Z) (out: Z) (i: Z) (PreH1 : (n = (string_length (input)))) (PreH2 : (out = 0)) (PreH3 : (3 <= n)) (PreH4 : (n < INT_MAX)) (PreH5 : (1 <= i)) (PreH6 : (i <= (n - 2 ))) (PreH7 : (valid_string input )) (PreH8 : (all_ascii input )) (PreH9 : (problem_118_pre_z input )) (PreH10 : (ascii_range_z input )) (PreH11 : (alpha_codes_z_118 input )) (PreH12 : ~((closest_vowel_candidate_z_118 input i ))) (PreH13 : (no_candidate_after_z_118 input i )) ,
+  (store_string word_pre input )
+|--
+  “ (n = (string_length (input))) ” 
+  &&  “ (out = 0) ” 
+  &&  “ (3 <= n) ” 
+  &&  “ (n < INT_MAX) ” 
+  &&  “ (0 <= (i - 1 )) ” 
+  &&  “ ((i - 1 ) <= (n - 2 )) ” 
+  &&  “ (valid_string input ) ” 
+  &&  “ (all_ascii input ) ” 
+  &&  “ (problem_118_pre_z input ) ” 
+  &&  “ (ascii_range_z input ) ” 
+  &&  “ (alpha_codes_z_118 input ) ” 
+  &&  “ (no_candidate_after_z_118 input (i - 1 ) ) ”
+  &&  (store_string word_pre input )
+) \/
+(
+forall (input: (@list Z)) (n: Z) (out: Z) (i: Z) (PreH1 : (0 <= ((string_length (input)) + 1 ))) (PreH2 : (n = (string_length (input)))) (PreH3 : (out = 0)) (PreH4 : (3 <= n)) (PreH5 : (n < INT_MAX)) (PreH6 : (1 <= i)) (PreH7 : (i <= (n - 2 ))) (PreH8 : (valid_string input )) (PreH9 : (all_ascii input )) (PreH10 : (problem_118_pre_z input )) (PreH11 : (ascii_range_z input )) (PreH12 : (alpha_codes_z_118 input )) (PreH13 : ~((closest_vowel_candidate_z_118 input i ))) (PreH14 : (no_candidate_after_z_118 input i )) ,
+  TT && emp 
+|--
+  “ (no_candidate_after_z_118 input (i - 1 ) ) ”
+  &&  emp
+).
+
+Definition get_closest_vowel_entail_wit_5_split_goal_1 := 
+forall (input: (@list Z)) (n: Z) (out: Z) (i: Z) (PreH1 : (0 <= ((string_length (input)) + 1 ))) (PreH2 : (n = (string_length (input)))) (PreH3 : (out = 0)) (PreH4 : (3 <= n)) (PreH5 : (n < INT_MAX)) (PreH6 : (1 <= i)) (PreH7 : (i <= (n - 2 ))) (PreH8 : (valid_string input )) (PreH9 : (all_ascii input )) (PreH10 : (problem_118_pre_z input )) (PreH11 : (ascii_range_z input )) (PreH12 : (alpha_codes_z_118 input )) (PreH13 : ~((closest_vowel_candidate_z_118 input i ))) (PreH14 : (no_candidate_after_z_118 input i )) ,
+  TT && emp 
+|--
+  “ (no_candidate_after_z_118 input (i - 1 ) ) ”
+.
+
+Definition get_closest_vowel_entail_wit_6 := 
+(
+forall (word_pre: Z) (input: (@list Z)) (i: Z) (out: Z) (n: Z) (PreH1 : (i < 1)) (PreH2 : (n = (string_length (input)))) (PreH3 : (out = 0)) (PreH4 : (3 <= n)) (PreH5 : (n < INT_MAX)) (PreH6 : (0 <= i)) (PreH7 : (i <= (n - 2 ))) (PreH8 : (valid_string input )) (PreH9 : (all_ascii input )) (PreH10 : (problem_118_pre_z input )) (PreH11 : (ascii_range_z input )) (PreH12 : (alpha_codes_z_118 input )) (PreH13 : (no_candidate_after_z_118 input i )) ,
+  (store_string word_pre input )
+|--
+  “ (n = (string_length (input))) ” 
+  &&  “ (out = 0) ” 
+  &&  “ (i = 0) ” 
+  &&  “ (valid_string input ) ” 
+  &&  “ (all_ascii input ) ” 
+  &&  “ (problem_118_pre_z input ) ” 
+  &&  “ (ascii_range_z input ) ” 
+  &&  “ (alpha_codes_z_118 input ) ” 
+  &&  “ (no_candidate_after_z_118 input 0 ) ”
+  &&  (store_string word_pre input )
+) \/
+(
+forall (input: (@list Z)) (i: Z) (out: Z) (n: Z) (PreH1 : (0 <= ((string_length (input)) + 1 ))) (PreH2 : (i < 1)) (PreH3 : (n = (string_length (input)))) (PreH4 : (out = 0)) (PreH5 : (3 <= n)) (PreH6 : (n < INT_MAX)) (PreH7 : (0 <= i)) (PreH8 : (i <= (n - 2 ))) (PreH9 : (valid_string input )) (PreH10 : (all_ascii input )) (PreH11 : (problem_118_pre_z input )) (PreH12 : (ascii_range_z input )) (PreH13 : (alpha_codes_z_118 input )) (PreH14 : (no_candidate_after_z_118 input i )) ,
+  TT && emp 
+|--
+  “ (no_candidate_after_z_118 input 0 ) ”
+  &&  emp
+).
+
+Definition get_closest_vowel_entail_wit_6_split_goal_1 := 
+forall (input: (@list Z)) (i: Z) (out: Z) (n: Z) (PreH1 : (0 <= ((string_length (input)) + 1 ))) (PreH2 : (i < 1)) (PreH3 : (n = (string_length (input)))) (PreH4 : (out = 0)) (PreH5 : (3 <= n)) (PreH6 : (n < INT_MAX)) (PreH7 : (0 <= i)) (PreH8 : (i <= (n - 2 ))) (PreH9 : (valid_string input )) (PreH10 : (all_ascii input )) (PreH11 : (problem_118_pre_z input )) (PreH12 : (ascii_range_z input )) (PreH13 : (alpha_codes_z_118 input )) (PreH14 : (no_candidate_after_z_118 input i )) ,
+  TT && emp 
+|--
+  “ (no_candidate_after_z_118 input 0 ) ”
+.
+
+Definition get_closest_vowel_return_wit_1 := 
+(
+forall (word_pre: Z) (input: (@list Z)) (n: Z) (out: Z) (i: Z) (retval: Z) (PreH1 : (retval <> 0)) (PreH2 : (retval <> 0)) (PreH3 : (0 <= ((string_length (input)) + 1 ))) (PreH4 : (n = (string_length (input)))) (PreH5 : (out = 0)) (PreH6 : (i = 0)) (PreH7 : (valid_string input )) (PreH8 : (all_ascii input )) (PreH9 : (problem_118_pre_z input )) (PreH10 : (ascii_range_z input )) (PreH11 : (alpha_codes_z_118 input )) (PreH12 : (no_candidate_after_z_118 input 0 )) ,
+  (CharArray.undef_seg retval (0 + 1 ) 1 )
+  **  (((retval + (0 * sizeof(CHAR) ) )) # Char  |-> 0)
+  **  (CharArray.full word_pre ((string_length (input)) + 1 ) (c_string (input)) )
+|--
+  EX (output: (@list Z)) ,
+  “ (problem_118_spec_z input output ) ”
+  &&  (store_string word_pre input )
+  **  (store_string retval output )
+) \/
+(
+forall (input: (@list Z)) (n: Z) (out: Z) (i: Z) (retval: Z) (PreH1 : (retval <> 0)) (PreH2 : (retval <> 0)) (PreH3 : (0 <= ((string_length (input)) + 1 ))) (PreH4 : (n = (string_length (input)))) (PreH5 : (out = 0)) (PreH6 : (i = 0)) (PreH7 : (valid_string input )) (PreH8 : (all_ascii input )) (PreH9 : (problem_118_pre_z input )) (PreH10 : (ascii_range_z input )) (PreH11 : (alpha_codes_z_118 input )) (PreH12 : (no_candidate_after_z_118 input 0 )) ,
+  (((retval + (0 * sizeof(CHAR) ) )) # Char  |-> 0)
+|--
+  EX (output: (@list Z)) ,
+  “ (problem_118_spec_z input output ) ”
+  &&  (CharArray.full retval ((string_length (output)) + 1 ) (c_string (output)) )
+).
+
+Definition get_closest_vowel_return_wit_2 := 
+(
+forall (word_pre: Z) (input: (@list Z)) (n: Z) (out: Z) (cur: Z) (i: Z) (retval: Z) (PreH1 : (retval <> 0)) (PreH2 : (retval <> 0)) (PreH3 : (0 <= ((string_length (input)) + 1 ))) (PreH4 : (n = (string_length (input)))) (PreH5 : (out = 0)) (PreH6 : (cur = (Znth (i) (input) (0)))) (PreH7 : (3 <= n)) (PreH8 : (n < INT_MAX)) (PreH9 : (1 <= i)) (PreH10 : (i <= (n - 2 ))) (PreH11 : (valid_string input )) (PreH12 : (all_ascii input )) (PreH13 : (problem_118_pre_z input )) (PreH14 : (ascii_range_z input )) (PreH15 : (alpha_codes_z_118 input )) (PreH16 : (closest_vowel_candidate_z_118 input i )) (PreH17 : (no_candidate_after_z_118 input i )) ,
+  (CharArray.undef_seg retval (1 + 1 ) 2 )
+  **  (((retval + (1 * sizeof(CHAR) ) )) # Char  |-> 0)
+  **  (((retval + (0 * sizeof(CHAR) ) )) # Char  |-> (signed_last_nbits (cur) (8)))
+  **  (CharArray.full word_pre ((string_length (input)) + 1 ) (c_string (input)) )
+|--
+  EX (output: (@list Z)) ,
+  “ (problem_118_spec_z input output ) ”
+  &&  (store_string word_pre input )
+  **  (store_string retval output )
+) \/
+(
+forall (input: (@list Z)) (n: Z) (out: Z) (cur: Z) (i: Z) (retval: Z) (PreH1 : (retval <> 0)) (PreH2 : (retval <> 0)) (PreH3 : (0 <= ((string_length (input)) + 1 ))) (PreH4 : (n = (string_length (input)))) (PreH5 : (out = 0)) (PreH6 : (cur = (Znth (i) (input) (0)))) (PreH7 : (3 <= n)) (PreH8 : (n < INT_MAX)) (PreH9 : (1 <= i)) (PreH10 : (i <= (n - 2 ))) (PreH11 : (valid_string input )) (PreH12 : (all_ascii input )) (PreH13 : (problem_118_pre_z input )) (PreH14 : (ascii_range_z input )) (PreH15 : (alpha_codes_z_118 input )) (PreH16 : (closest_vowel_candidate_z_118 input i )) (PreH17 : (no_candidate_after_z_118 input i )) ,
+  (((retval + (1 * sizeof(CHAR) ) )) # Char  |-> 0)
+  **  (((retval + (0 * sizeof(CHAR) ) )) # Char  |-> (signed_last_nbits (cur) (8)))
+|--
+  EX (output: (@list Z)) ,
+  “ (problem_118_spec_z input output ) ”
+  &&  (CharArray.full retval ((string_length (output)) + 1 ) (c_string (output)) )
+).
+
+Definition get_closest_vowel_return_wit_3 := 
+(
+forall (word_pre: Z) (input: (@list Z)) (n: Z) (out: Z) (retval: Z) (PreH1 : (retval <> 0)) (PreH2 : (retval <> 0)) (PreH3 : (0 <= ((string_length (input)) + 1 ))) (PreH4 : (n < 3)) (PreH5 : (n = (string_length (input)))) (PreH6 : (out = 0)) (PreH7 : (valid_string input )) (PreH8 : (all_ascii input )) (PreH9 : (problem_118_pre_z input )) (PreH10 : (ascii_range_z input )) (PreH11 : (alpha_codes_z_118 input )) (PreH12 : ((string_length (input)) < INT_MAX)) ,
+  (CharArray.undef_seg retval (0 + 1 ) 1 )
+  **  (((retval + (0 * sizeof(CHAR) ) )) # Char  |-> 0)
+  **  (CharArray.full word_pre ((string_length (input)) + 1 ) (c_string (input)) )
+|--
+  EX (output: (@list Z)) ,
+  “ (problem_118_spec_z input output ) ”
+  &&  (store_string word_pre input )
+  **  (store_string retval output )
+) \/
+(
+forall (input: (@list Z)) (n: Z) (out: Z) (retval: Z) (PreH1 : (retval <> 0)) (PreH2 : (retval <> 0)) (PreH3 : (0 <= ((string_length (input)) + 1 ))) (PreH4 : (n < 3)) (PreH5 : (n = (string_length (input)))) (PreH6 : (out = 0)) (PreH7 : (valid_string input )) (PreH8 : (all_ascii input )) (PreH9 : (problem_118_pre_z input )) (PreH10 : (ascii_range_z input )) (PreH11 : (alpha_codes_z_118 input )) (PreH12 : ((string_length (input)) < INT_MAX)) ,
+  (((retval + (0 * sizeof(CHAR) ) )) # Char  |-> 0)
+|--
+  EX (output: (@list Z)) ,
+  “ (problem_118_spec_z input output ) ”
+  &&  (CharArray.full retval ((string_length (output)) + 1 ) (c_string (output)) )
+).
+
+Definition get_closest_vowel_partial_solve_wit_1_pure := 
+forall (word_pre: Z) (input: (@list Z)) (PreH1 : (valid_string input )) (PreH2 : (all_ascii input )) (PreH3 : (problem_118_pre_z input )) (PreH4 : (ascii_range_z input )) (PreH5 : ((string_length (input)) < INT_MAX)) ,
+  ((( &( "n" ) )) # Int  |->_)
+  **  ((( &( "word" ) )) # Ptr  |-> word_pre)
+  **  (store_string word_pre input )
+|--
+  “ (valid_string input ) ” 
+  &&  “ ((string_length (input)) < INT_MAX) ”
+.
+
+Definition get_closest_vowel_partial_solve_wit_1_aux := 
+forall (word_pre: Z) (input: (@list Z)) (PreH1 : (valid_string input )) (PreH2 : (all_ascii input )) (PreH3 : (problem_118_pre_z input )) (PreH4 : (ascii_range_z input )) (PreH5 : ((string_length (input)) < INT_MAX)) ,
+  (store_string word_pre input )
+|--
+  “ (valid_string input ) ” 
+  &&  “ ((string_length (input)) < INT_MAX) ” 
+  &&  “ (0 <= ((string_length (input)) + 1 )) ” 
+  &&  “ (valid_string input ) ” 
+  &&  “ (all_ascii input ) ” 
+  &&  “ (problem_118_pre_z input ) ” 
+  &&  “ (ascii_range_z input ) ” 
+  &&  “ ((string_length (input)) < INT_MAX) ”
+  &&  (store_string word_pre input )
+.
+
+Definition get_closest_vowel_partial_solve_wit_1 := get_closest_vowel_partial_solve_wit_1_pure -> get_closest_vowel_partial_solve_wit_1_aux.
+
+Definition get_closest_vowel_partial_solve_wit_2_pure := 
+forall (word_pre: Z) (input: (@list Z)) (n: Z) (out: Z) (PreH1 : (n < 3)) (PreH2 : (n = (string_length (input)))) (PreH3 : (out = 0)) (PreH4 : (valid_string input )) (PreH5 : (all_ascii input )) (PreH6 : (problem_118_pre_z input )) (PreH7 : (ascii_range_z input )) (PreH8 : (alpha_codes_z_118 input )) (PreH9 : ((string_length (input)) < INT_MAX)) ,
+  ((( &( "word" ) )) # Ptr  |-> word_pre)
+  **  ((( &( "n" ) )) # Int  |-> n)
+  **  ((( &( "out" ) )) # Ptr  |-> out)
+  **  (store_string word_pre input )
+|--
+  “ (1 > 0) ” 
+  &&  “ (1 < INT_MAX) ”
+.
+
+Definition get_closest_vowel_partial_solve_wit_2_aux := 
+forall (word_pre: Z) (input: (@list Z)) (n: Z) (out: Z) (PreH1 : (n < 3)) (PreH2 : (n = (string_length (input)))) (PreH3 : (out = 0)) (PreH4 : (valid_string input )) (PreH5 : (all_ascii input )) (PreH6 : (problem_118_pre_z input )) (PreH7 : (ascii_range_z input )) (PreH8 : (alpha_codes_z_118 input )) (PreH9 : ((string_length (input)) < INT_MAX)) ,
+  (store_string word_pre input )
+|--
+  “ (1 > 0) ” 
+  &&  “ (1 < INT_MAX) ” 
+  &&  “ (0 <= ((string_length (input)) + 1 )) ” 
+  &&  “ (n < 3) ” 
+  &&  “ (n = (string_length (input))) ” 
+  &&  “ (out = 0) ” 
+  &&  “ (valid_string input ) ” 
+  &&  “ (all_ascii input ) ” 
+  &&  “ (problem_118_pre_z input ) ” 
+  &&  “ (ascii_range_z input ) ” 
+  &&  “ (alpha_codes_z_118 input ) ” 
+  &&  “ ((string_length (input)) < INT_MAX) ”
+  &&  (CharArray.full word_pre ((string_length (input)) + 1 ) (c_string (input)) )
+.
+
+Definition get_closest_vowel_partial_solve_wit_2 := get_closest_vowel_partial_solve_wit_2_pure -> get_closest_vowel_partial_solve_wit_2_aux.
+
+Definition get_closest_vowel_partial_solve_wit_3 := 
+forall (word_pre: Z) (input: (@list Z)) (n: Z) (out: Z) (retval: Z) (PreH1 : (retval <> 0)) (PreH2 : (retval <> 0)) (PreH3 : (0 <= ((string_length (input)) + 1 ))) (PreH4 : (n < 3)) (PreH5 : (n = (string_length (input)))) (PreH6 : (out = 0)) (PreH7 : (valid_string input )) (PreH8 : (all_ascii input )) (PreH9 : (problem_118_pre_z input )) (PreH10 : (ascii_range_z input )) (PreH11 : (alpha_codes_z_118 input )) (PreH12 : ((string_length (input)) < INT_MAX)) ,
+  (CharArray.undef_full retval 1 )
+  **  (CharArray.full word_pre ((string_length (input)) + 1 ) (c_string (input)) )
+|--
+  “ (retval <> 0) ” 
+  &&  “ (retval <> 0) ” 
+  &&  “ (0 <= ((string_length (input)) + 1 )) ” 
+  &&  “ (n < 3) ” 
+  &&  “ (n = (string_length (input))) ” 
+  &&  “ (out = 0) ” 
+  &&  “ (valid_string input ) ” 
+  &&  “ (all_ascii input ) ” 
+  &&  “ (problem_118_pre_z input ) ” 
+  &&  “ (ascii_range_z input ) ” 
+  &&  “ (alpha_codes_z_118 input ) ” 
+  &&  “ ((string_length (input)) < INT_MAX) ”
+  &&  (((retval + (0 * sizeof(CHAR) ) )) # Char  |->_)
+  **  (CharArray.undef_missing_i retval 0 0 1 )
+  **  (CharArray.full word_pre ((string_length (input)) + 1 ) (c_string (input)) )
+.
+
+Definition get_closest_vowel_partial_solve_wit_4_pure := 
+(
+forall (word_pre: Z) (input: (@list Z)) (i: Z) (left_vowel: Z) (right_vowel: Z) (cur_vowel: Z) (out: Z) (n: Z) (PreH1 : (i >= 1)) (PreH2 : (n = (string_length (input)))) (PreH3 : (out = 0)) (PreH4 : (3 <= n)) (PreH5 : (n < INT_MAX)) (PreH6 : (0 <= i)) (PreH7 : (i <= (n - 2 ))) (PreH8 : (valid_string input )) (PreH9 : (all_ascii input )) (PreH10 : (problem_118_pre_z input )) (PreH11 : (ascii_range_z input )) (PreH12 : (alpha_codes_z_118 input )) (PreH13 : (no_candidate_after_z_118 input i )) ,
+  ((( &( "word" ) )) # Ptr  |-> word_pre)
+  **  ((( &( "n" ) )) # Int  |-> n)
+  **  ((( &( "out" ) )) # Ptr  |-> out)
+  **  ((( &( "cur" ) )) # Int  |-> (Znth i (c_string (input)) 0))
+  **  ((( &( "right" ) )) # Int  |-> (Znth (i + 1 ) (c_string (input)) 0))
+  **  ((( &( "left" ) )) # Int  |-> (Znth (i - 1 ) (c_string (input)) 0))
+  **  ((( &( "cur_vowel" ) )) # Int  |-> cur_vowel)
+  **  ((( &( "right_vowel" ) )) # Int  |-> right_vowel)
+  **  ((( &( "left_vowel" ) )) # Int  |-> left_vowel)
+  **  ((( &( "i" ) )) # Int  |-> i)
+  **  (store_string word_pre input )
+|--
+  “ ((Znth i (c_string (input)) 0) <= 127) ” 
+  &&  “ (0 <= (Znth i (c_string (input)) 0)) ”
+) \/
+(
+forall (word_pre: Z) (input: (@list Z)) (i: Z) (left_vowel: Z) (right_vowel: Z) (cur_vowel: Z) (out: Z) (n: Z) (PreH1 : (i <= INT_MAX)) (PreH2 : (left_vowel <= INT_MAX)) (PreH3 : (right_vowel <= INT_MAX)) (PreH4 : (cur_vowel <= INT_MAX)) (PreH5 : ((Znth (i - 1 ) (c_string (input)) 0) <= INT_MAX)) (PreH6 : ((Znth (i + 1 ) (c_string (input)) 0) <= INT_MAX)) (PreH7 : ((Znth i (c_string (input)) 0) <= INT_MAX)) (PreH8 : (n <= INT_MAX)) (PreH9 : (i >= INT_MIN)) (PreH10 : (left_vowel >= INT_MIN)) (PreH11 : (right_vowel >= INT_MIN)) (PreH12 : (cur_vowel >= INT_MIN)) (PreH13 : ((Znth (i - 1 ) (c_string (input)) 0) >= INT_MIN)) (PreH14 : ((Znth (i + 1 ) (c_string (input)) 0) >= INT_MIN)) (PreH15 : ((Znth i (c_string (input)) 0) >= INT_MIN)) (PreH16 : (n >= INT_MIN)) (PreH17 : (0 <= ((string_length (input)) + 1 ))) (PreH18 : (i >= 1)) (PreH19 : (n = (string_length (input)))) (PreH20 : (out = 0)) (PreH21 : (3 <= n)) (PreH22 : (n < INT_MAX)) (PreH23 : (0 <= i)) (PreH24 : (i <= (n - 2 ))) (PreH25 : (valid_string input )) (PreH26 : (all_ascii input )) (PreH27 : (problem_118_pre_z input )) (PreH28 : (ascii_range_z input )) (PreH29 : (alpha_codes_z_118 input )) (PreH30 : (no_candidate_after_z_118 input i )) ,
+  (CharArray.full word_pre ((string_length (input)) + 1 ) (c_string (input)) )
+  **  ((( &( "word" ) )) # Ptr  |-> word_pre)
+  **  ((( &( "n" ) )) # Int  |-> n)
+  **  ((( &( "out" ) )) # Ptr  |-> out)
+  **  ((( &( "cur" ) )) # Int  |-> (Znth i (c_string (input)) 0))
+  **  ((( &( "right" ) )) # Int  |-> (Znth (i + 1 ) (c_string (input)) 0))
+  **  ((( &( "left" ) )) # Int  |-> (Znth (i - 1 ) (c_string (input)) 0))
+  **  ((( &( "cur_vowel" ) )) # Int  |-> cur_vowel)
+  **  ((( &( "right_vowel" ) )) # Int  |-> right_vowel)
+  **  ((( &( "left_vowel" ) )) # Int  |-> left_vowel)
+  **  ((( &( "i" ) )) # Int  |-> i)
+|--
+  “ (0 <= (Znth i (c_string (input)) 0)) ” 
+  &&  “ ((Znth i (c_string (input)) 0) <= 127) ”
+).
+
+Definition get_closest_vowel_partial_solve_wit_4_pure_split_goal_1 := 
+forall (word_pre: Z) (input: (@list Z)) (i: Z) (left_vowel: Z) (right_vowel: Z) (cur_vowel: Z) (out: Z) (n: Z) (PreH1 : (i <= INT_MAX)) (PreH2 : (left_vowel <= INT_MAX)) (PreH3 : (right_vowel <= INT_MAX)) (PreH4 : (cur_vowel <= INT_MAX)) (PreH5 : ((Znth (i - 1 ) (c_string (input)) 0) <= INT_MAX)) (PreH6 : ((Znth (i + 1 ) (c_string (input)) 0) <= INT_MAX)) (PreH7 : ((Znth i (c_string (input)) 0) <= INT_MAX)) (PreH8 : (n <= INT_MAX)) (PreH9 : (i >= INT_MIN)) (PreH10 : (left_vowel >= INT_MIN)) (PreH11 : (right_vowel >= INT_MIN)) (PreH12 : (cur_vowel >= INT_MIN)) (PreH13 : ((Znth (i - 1 ) (c_string (input)) 0) >= INT_MIN)) (PreH14 : ((Znth (i + 1 ) (c_string (input)) 0) >= INT_MIN)) (PreH15 : ((Znth i (c_string (input)) 0) >= INT_MIN)) (PreH16 : (n >= INT_MIN)) (PreH17 : (0 <= ((string_length (input)) + 1 ))) (PreH18 : (i >= 1)) (PreH19 : (n = (string_length (input)))) (PreH20 : (out = 0)) (PreH21 : (3 <= n)) (PreH22 : (n < INT_MAX)) (PreH23 : (0 <= i)) (PreH24 : (i <= (n - 2 ))) (PreH25 : (valid_string input )) (PreH26 : (all_ascii input )) (PreH27 : (problem_118_pre_z input )) (PreH28 : (ascii_range_z input )) (PreH29 : (alpha_codes_z_118 input )) (PreH30 : (no_candidate_after_z_118 input i )) ,
+  (CharArray.full word_pre ((string_length (input)) + 1 ) (c_string (input)) )
+  **  ((( &( "word" ) )) # Ptr  |-> word_pre)
+  **  ((( &( "n" ) )) # Int  |-> n)
+  **  ((( &( "out" ) )) # Ptr  |-> out)
+  **  ((( &( "cur" ) )) # Int  |-> (Znth i (c_string (input)) 0))
+  **  ((( &( "right" ) )) # Int  |-> (Znth (i + 1 ) (c_string (input)) 0))
+  **  ((( &( "left" ) )) # Int  |-> (Znth (i - 1 ) (c_string (input)) 0))
+  **  ((( &( "cur_vowel" ) )) # Int  |-> cur_vowel)
+  **  ((( &( "right_vowel" ) )) # Int  |-> right_vowel)
+  **  ((( &( "left_vowel" ) )) # Int  |-> left_vowel)
+  **  ((( &( "i" ) )) # Int  |-> i)
+|--
+  “ (0 <= (Znth i (c_string (input)) 0)) ”
+.
+
+Definition get_closest_vowel_partial_solve_wit_4_pure_split_goal_2 := 
+forall (word_pre: Z) (input: (@list Z)) (i: Z) (left_vowel: Z) (right_vowel: Z) (cur_vowel: Z) (out: Z) (n: Z) (PreH1 : (i <= INT_MAX)) (PreH2 : (left_vowel <= INT_MAX)) (PreH3 : (right_vowel <= INT_MAX)) (PreH4 : (cur_vowel <= INT_MAX)) (PreH5 : ((Znth (i - 1 ) (c_string (input)) 0) <= INT_MAX)) (PreH6 : ((Znth (i + 1 ) (c_string (input)) 0) <= INT_MAX)) (PreH7 : ((Znth i (c_string (input)) 0) <= INT_MAX)) (PreH8 : (n <= INT_MAX)) (PreH9 : (i >= INT_MIN)) (PreH10 : (left_vowel >= INT_MIN)) (PreH11 : (right_vowel >= INT_MIN)) (PreH12 : (cur_vowel >= INT_MIN)) (PreH13 : ((Znth (i - 1 ) (c_string (input)) 0) >= INT_MIN)) (PreH14 : ((Znth (i + 1 ) (c_string (input)) 0) >= INT_MIN)) (PreH15 : ((Znth i (c_string (input)) 0) >= INT_MIN)) (PreH16 : (n >= INT_MIN)) (PreH17 : (0 <= ((string_length (input)) + 1 ))) (PreH18 : (i >= 1)) (PreH19 : (n = (string_length (input)))) (PreH20 : (out = 0)) (PreH21 : (3 <= n)) (PreH22 : (n < INT_MAX)) (PreH23 : (0 <= i)) (PreH24 : (i <= (n - 2 ))) (PreH25 : (valid_string input )) (PreH26 : (all_ascii input )) (PreH27 : (problem_118_pre_z input )) (PreH28 : (ascii_range_z input )) (PreH29 : (alpha_codes_z_118 input )) (PreH30 : (no_candidate_after_z_118 input i )) ,
+  (CharArray.full word_pre ((string_length (input)) + 1 ) (c_string (input)) )
+  **  ((( &( "word" ) )) # Ptr  |-> word_pre)
+  **  ((( &( "n" ) )) # Int  |-> n)
+  **  ((( &( "out" ) )) # Ptr  |-> out)
+  **  ((( &( "cur" ) )) # Int  |-> (Znth i (c_string (input)) 0))
+  **  ((( &( "right" ) )) # Int  |-> (Znth (i + 1 ) (c_string (input)) 0))
+  **  ((( &( "left" ) )) # Int  |-> (Znth (i - 1 ) (c_string (input)) 0))
+  **  ((( &( "cur_vowel" ) )) # Int  |-> cur_vowel)
+  **  ((( &( "right_vowel" ) )) # Int  |-> right_vowel)
+  **  ((( &( "left_vowel" ) )) # Int  |-> left_vowel)
+  **  ((( &( "i" ) )) # Int  |-> i)
+|--
+  “ ((Znth i (c_string (input)) 0) <= 127) ”
+.
+
+Definition get_closest_vowel_partial_solve_wit_4_aux := 
+forall (word_pre: Z) (input: (@list Z)) (i: Z) (out: Z) (n: Z) (PreH1 : (i >= 1)) (PreH2 : (n = (string_length (input)))) (PreH3 : (out = 0)) (PreH4 : (3 <= n)) (PreH5 : (n < INT_MAX)) (PreH6 : (0 <= i)) (PreH7 : (i <= (n - 2 ))) (PreH8 : (valid_string input )) (PreH9 : (all_ascii input )) (PreH10 : (problem_118_pre_z input )) (PreH11 : (ascii_range_z input )) (PreH12 : (alpha_codes_z_118 input )) (PreH13 : (no_candidate_after_z_118 input i )) ,
+  (store_string word_pre input )
+|--
+  “ ((Znth i (c_string (input)) 0) <= 127) ” 
+  &&  “ (0 <= (Znth i (c_string (input)) 0)) ” 
+  &&  “ (0 <= ((string_length (input)) + 1 )) ” 
+  &&  “ (i >= 1) ” 
+  &&  “ (n = (string_length (input))) ” 
+  &&  “ (out = 0) ” 
+  &&  “ (3 <= n) ” 
+  &&  “ (n < INT_MAX) ” 
+  &&  “ (0 <= i) ” 
+  &&  “ (i <= (n - 2 )) ” 
+  &&  “ (valid_string input ) ” 
+  &&  “ (all_ascii input ) ” 
+  &&  “ (problem_118_pre_z input ) ” 
+  &&  “ (ascii_range_z input ) ” 
+  &&  “ (alpha_codes_z_118 input ) ” 
+  &&  “ (no_candidate_after_z_118 input i ) ”
+  &&  (CharArray.full word_pre ((string_length (input)) + 1 ) (c_string (input)) )
+.
+
+Definition get_closest_vowel_partial_solve_wit_4 := get_closest_vowel_partial_solve_wit_4_pure -> get_closest_vowel_partial_solve_wit_4_aux.
+
+Definition get_closest_vowel_partial_solve_wit_5_pure := 
+(
+forall (word_pre: Z) (input: (@list Z)) (i: Z) (left_vowel: Z) (right_vowel: Z) (out: Z) (n: Z) (retval: Z) (PreH1 : (retval = 1)) (PreH2 : (retval = 1)) (PreH3 : (is_vowel_z_118 (Znth i (c_string (input)) 0) )) (PreH4 : (0 <= ((string_length (input)) + 1 ))) (PreH5 : (i >= 1)) (PreH6 : (n = (string_length (input)))) (PreH7 : (out = 0)) (PreH8 : (3 <= n)) (PreH9 : (n < INT_MAX)) (PreH10 : (0 <= i)) (PreH11 : (i <= (n - 2 ))) (PreH12 : (valid_string input )) (PreH13 : (all_ascii input )) (PreH14 : (problem_118_pre_z input )) (PreH15 : (ascii_range_z input )) (PreH16 : (alpha_codes_z_118 input )) (PreH17 : (no_candidate_after_z_118 input i )) ,
+  (CharArray.full word_pre ((string_length (input)) + 1 ) (c_string (input)) )
+  **  ((( &( "word" ) )) # Ptr  |-> word_pre)
+  **  ((( &( "n" ) )) # Int  |-> n)
+  **  ((( &( "out" ) )) # Ptr  |-> out)
+  **  ((( &( "cur" ) )) # Int  |-> (Znth i (c_string (input)) 0))
+  **  ((( &( "right" ) )) # Int  |-> (Znth (i + 1 ) (c_string (input)) 0))
+  **  ((( &( "left" ) )) # Int  |-> (Znth (i - 1 ) (c_string (input)) 0))
+  **  ((( &( "cur_vowel" ) )) # Int  |-> retval)
+  **  ((( &( "right_vowel" ) )) # Int  |-> right_vowel)
+  **  ((( &( "left_vowel" ) )) # Int  |-> left_vowel)
+  **  ((( &( "i" ) )) # Int  |-> i)
+|--
+  “ ((Znth (i + 1 ) (c_string (input)) 0) <= 127) ” 
+  &&  “ (0 <= (Znth (i + 1 ) (c_string (input)) 0)) ”
+) \/
+(
+forall (word_pre: Z) (input: (@list Z)) (i: Z) (left_vowel: Z) (right_vowel: Z) (out: Z) (n: Z) (retval: Z) (PreH1 : (i <= INT_MAX)) (PreH2 : (left_vowel <= INT_MAX)) (PreH3 : (right_vowel <= INT_MAX)) (PreH4 : (retval <= INT_MAX)) (PreH5 : ((Znth (i - 1 ) (c_string (input)) 0) <= INT_MAX)) (PreH6 : ((Znth (i + 1 ) (c_string (input)) 0) <= INT_MAX)) (PreH7 : ((Znth i (c_string (input)) 0) <= INT_MAX)) (PreH8 : (n <= INT_MAX)) (PreH9 : (i >= INT_MIN)) (PreH10 : (left_vowel >= INT_MIN)) (PreH11 : (right_vowel >= INT_MIN)) (PreH12 : (retval >= INT_MIN)) (PreH13 : ((Znth (i - 1 ) (c_string (input)) 0) >= INT_MIN)) (PreH14 : ((Znth (i + 1 ) (c_string (input)) 0) >= INT_MIN)) (PreH15 : ((Znth i (c_string (input)) 0) >= INT_MIN)) (PreH16 : (n >= INT_MIN)) (PreH17 : (retval = 1)) (PreH18 : (retval = 1)) (PreH19 : (is_vowel_z_118 (Znth i (c_string (input)) 0) )) (PreH20 : (0 <= ((string_length (input)) + 1 ))) (PreH21 : (i >= 1)) (PreH22 : (n = (string_length (input)))) (PreH23 : (out = 0)) (PreH24 : (3 <= n)) (PreH25 : (n < INT_MAX)) (PreH26 : (0 <= i)) (PreH27 : (i <= (n - 2 ))) (PreH28 : (valid_string input )) (PreH29 : (all_ascii input )) (PreH30 : (problem_118_pre_z input )) (PreH31 : (ascii_range_z input )) (PreH32 : (alpha_codes_z_118 input )) (PreH33 : (no_candidate_after_z_118 input i )) ,
+  (CharArray.full word_pre ((string_length (input)) + 1 ) (c_string (input)) )
+  **  ((( &( "word" ) )) # Ptr  |-> word_pre)
+  **  ((( &( "n" ) )) # Int  |-> n)
+  **  ((( &( "out" ) )) # Ptr  |-> out)
+  **  ((( &( "cur" ) )) # Int  |-> (Znth i (c_string (input)) 0))
+  **  ((( &( "right" ) )) # Int  |-> (Znth (i + 1 ) (c_string (input)) 0))
+  **  ((( &( "left" ) )) # Int  |-> (Znth (i - 1 ) (c_string (input)) 0))
+  **  ((( &( "cur_vowel" ) )) # Int  |-> retval)
+  **  ((( &( "right_vowel" ) )) # Int  |-> right_vowel)
+  **  ((( &( "left_vowel" ) )) # Int  |-> left_vowel)
+  **  ((( &( "i" ) )) # Int  |-> i)
+|--
+  “ (0 <= (Znth (i + 1 ) (c_string (input)) 0)) ” 
+  &&  “ ((Znth (i + 1 ) (c_string (input)) 0) <= 127) ”
+).
+
+Definition get_closest_vowel_partial_solve_wit_5_pure_split_goal_1 := 
+forall (word_pre: Z) (input: (@list Z)) (i: Z) (left_vowel: Z) (right_vowel: Z) (out: Z) (n: Z) (retval: Z) (PreH1 : (i <= INT_MAX)) (PreH2 : (left_vowel <= INT_MAX)) (PreH3 : (right_vowel <= INT_MAX)) (PreH4 : (retval <= INT_MAX)) (PreH5 : ((Znth (i - 1 ) (c_string (input)) 0) <= INT_MAX)) (PreH6 : ((Znth (i + 1 ) (c_string (input)) 0) <= INT_MAX)) (PreH7 : ((Znth i (c_string (input)) 0) <= INT_MAX)) (PreH8 : (n <= INT_MAX)) (PreH9 : (i >= INT_MIN)) (PreH10 : (left_vowel >= INT_MIN)) (PreH11 : (right_vowel >= INT_MIN)) (PreH12 : (retval >= INT_MIN)) (PreH13 : ((Znth (i - 1 ) (c_string (input)) 0) >= INT_MIN)) (PreH14 : ((Znth (i + 1 ) (c_string (input)) 0) >= INT_MIN)) (PreH15 : ((Znth i (c_string (input)) 0) >= INT_MIN)) (PreH16 : (n >= INT_MIN)) (PreH17 : (retval = 1)) (PreH18 : (retval = 1)) (PreH19 : (is_vowel_z_118 (Znth i (c_string (input)) 0) )) (PreH20 : (0 <= ((string_length (input)) + 1 ))) (PreH21 : (i >= 1)) (PreH22 : (n = (string_length (input)))) (PreH23 : (out = 0)) (PreH24 : (3 <= n)) (PreH25 : (n < INT_MAX)) (PreH26 : (0 <= i)) (PreH27 : (i <= (n - 2 ))) (PreH28 : (valid_string input )) (PreH29 : (all_ascii input )) (PreH30 : (problem_118_pre_z input )) (PreH31 : (ascii_range_z input )) (PreH32 : (alpha_codes_z_118 input )) (PreH33 : (no_candidate_after_z_118 input i )) ,
+  (CharArray.full word_pre ((string_length (input)) + 1 ) (c_string (input)) )
+  **  ((( &( "word" ) )) # Ptr  |-> word_pre)
+  **  ((( &( "n" ) )) # Int  |-> n)
+  **  ((( &( "out" ) )) # Ptr  |-> out)
+  **  ((( &( "cur" ) )) # Int  |-> (Znth i (c_string (input)) 0))
+  **  ((( &( "right" ) )) # Int  |-> (Znth (i + 1 ) (c_string (input)) 0))
+  **  ((( &( "left" ) )) # Int  |-> (Znth (i - 1 ) (c_string (input)) 0))
+  **  ((( &( "cur_vowel" ) )) # Int  |-> retval)
+  **  ((( &( "right_vowel" ) )) # Int  |-> right_vowel)
+  **  ((( &( "left_vowel" ) )) # Int  |-> left_vowel)
+  **  ((( &( "i" ) )) # Int  |-> i)
+|--
+  “ (0 <= (Znth (i + 1 ) (c_string (input)) 0)) ”
+.
+
+Definition get_closest_vowel_partial_solve_wit_5_pure_split_goal_2 := 
+forall (word_pre: Z) (input: (@list Z)) (i: Z) (left_vowel: Z) (right_vowel: Z) (out: Z) (n: Z) (retval: Z) (PreH1 : (i <= INT_MAX)) (PreH2 : (left_vowel <= INT_MAX)) (PreH3 : (right_vowel <= INT_MAX)) (PreH4 : (retval <= INT_MAX)) (PreH5 : ((Znth (i - 1 ) (c_string (input)) 0) <= INT_MAX)) (PreH6 : ((Znth (i + 1 ) (c_string (input)) 0) <= INT_MAX)) (PreH7 : ((Znth i (c_string (input)) 0) <= INT_MAX)) (PreH8 : (n <= INT_MAX)) (PreH9 : (i >= INT_MIN)) (PreH10 : (left_vowel >= INT_MIN)) (PreH11 : (right_vowel >= INT_MIN)) (PreH12 : (retval >= INT_MIN)) (PreH13 : ((Znth (i - 1 ) (c_string (input)) 0) >= INT_MIN)) (PreH14 : ((Znth (i + 1 ) (c_string (input)) 0) >= INT_MIN)) (PreH15 : ((Znth i (c_string (input)) 0) >= INT_MIN)) (PreH16 : (n >= INT_MIN)) (PreH17 : (retval = 1)) (PreH18 : (retval = 1)) (PreH19 : (is_vowel_z_118 (Znth i (c_string (input)) 0) )) (PreH20 : (0 <= ((string_length (input)) + 1 ))) (PreH21 : (i >= 1)) (PreH22 : (n = (string_length (input)))) (PreH23 : (out = 0)) (PreH24 : (3 <= n)) (PreH25 : (n < INT_MAX)) (PreH26 : (0 <= i)) (PreH27 : (i <= (n - 2 ))) (PreH28 : (valid_string input )) (PreH29 : (all_ascii input )) (PreH30 : (problem_118_pre_z input )) (PreH31 : (ascii_range_z input )) (PreH32 : (alpha_codes_z_118 input )) (PreH33 : (no_candidate_after_z_118 input i )) ,
+  (CharArray.full word_pre ((string_length (input)) + 1 ) (c_string (input)) )
+  **  ((( &( "word" ) )) # Ptr  |-> word_pre)
+  **  ((( &( "n" ) )) # Int  |-> n)
+  **  ((( &( "out" ) )) # Ptr  |-> out)
+  **  ((( &( "cur" ) )) # Int  |-> (Znth i (c_string (input)) 0))
+  **  ((( &( "right" ) )) # Int  |-> (Znth (i + 1 ) (c_string (input)) 0))
+  **  ((( &( "left" ) )) # Int  |-> (Znth (i - 1 ) (c_string (input)) 0))
+  **  ((( &( "cur_vowel" ) )) # Int  |-> retval)
+  **  ((( &( "right_vowel" ) )) # Int  |-> right_vowel)
+  **  ((( &( "left_vowel" ) )) # Int  |-> left_vowel)
+  **  ((( &( "i" ) )) # Int  |-> i)
+|--
+  “ ((Znth (i + 1 ) (c_string (input)) 0) <= 127) ”
+.
+
+Definition get_closest_vowel_partial_solve_wit_5_aux := 
+forall (word_pre: Z) (input: (@list Z)) (i: Z) (out: Z) (n: Z) (retval: Z) (PreH1 : (retval = 1)) (PreH2 : (retval = 1)) (PreH3 : (is_vowel_z_118 (Znth i (c_string (input)) 0) )) (PreH4 : (0 <= ((string_length (input)) + 1 ))) (PreH5 : (i >= 1)) (PreH6 : (n = (string_length (input)))) (PreH7 : (out = 0)) (PreH8 : (3 <= n)) (PreH9 : (n < INT_MAX)) (PreH10 : (0 <= i)) (PreH11 : (i <= (n - 2 ))) (PreH12 : (valid_string input )) (PreH13 : (all_ascii input )) (PreH14 : (problem_118_pre_z input )) (PreH15 : (ascii_range_z input )) (PreH16 : (alpha_codes_z_118 input )) (PreH17 : (no_candidate_after_z_118 input i )) ,
+  (CharArray.full word_pre ((string_length (input)) + 1 ) (c_string (input)) )
+|--
+  “ ((Znth (i + 1 ) (c_string (input)) 0) <= 127) ” 
+  &&  “ (0 <= (Znth (i + 1 ) (c_string (input)) 0)) ” 
+  &&  “ (retval = 1) ” 
+  &&  “ (retval = 1) ” 
+  &&  “ (is_vowel_z_118 (Znth i (c_string (input)) 0) ) ” 
+  &&  “ (0 <= ((string_length (input)) + 1 )) ” 
+  &&  “ (i >= 1) ” 
+  &&  “ (n = (string_length (input))) ” 
+  &&  “ (out = 0) ” 
+  &&  “ (3 <= n) ” 
+  &&  “ (n < INT_MAX) ” 
+  &&  “ (0 <= i) ” 
+  &&  “ (i <= (n - 2 )) ” 
+  &&  “ (valid_string input ) ” 
+  &&  “ (all_ascii input ) ” 
+  &&  “ (problem_118_pre_z input ) ” 
+  &&  “ (ascii_range_z input ) ” 
+  &&  “ (alpha_codes_z_118 input ) ” 
+  &&  “ (no_candidate_after_z_118 input i ) ”
+  &&  (CharArray.full word_pre ((string_length (input)) + 1 ) (c_string (input)) )
+.
+
+Definition get_closest_vowel_partial_solve_wit_5 := get_closest_vowel_partial_solve_wit_5_pure -> get_closest_vowel_partial_solve_wit_5_aux.
+
+Definition get_closest_vowel_partial_solve_wit_6_pure := 
+(
+forall (word_pre: Z) (input: (@list Z)) (i: Z) (left_vowel: Z) (out: Z) (n: Z) (retval: Z) (retval_2: Z) (PreH1 : (retval_2 = 0)) (PreH2 : (retval_2 = 0)) (PreH3 : ~((is_vowel_z_118 (Znth (i + 1 ) (c_string (input)) 0) ))) (PreH4 : (retval = 1)) (PreH5 : (retval = 1)) (PreH6 : (is_vowel_z_118 (Znth i (c_string (input)) 0) )) (PreH7 : (0 <= ((string_length (input)) + 1 ))) (PreH8 : (i >= 1)) (PreH9 : (n = (string_length (input)))) (PreH10 : (out = 0)) (PreH11 : (3 <= n)) (PreH12 : (n < INT_MAX)) (PreH13 : (0 <= i)) (PreH14 : (i <= (n - 2 ))) (PreH15 : (valid_string input )) (PreH16 : (all_ascii input )) (PreH17 : (problem_118_pre_z input )) (PreH18 : (ascii_range_z input )) (PreH19 : (alpha_codes_z_118 input )) (PreH20 : (no_candidate_after_z_118 input i )) ,
+  (CharArray.full word_pre ((string_length (input)) + 1 ) (c_string (input)) )
+  **  ((( &( "word" ) )) # Ptr  |-> word_pre)
+  **  ((( &( "n" ) )) # Int  |-> n)
+  **  ((( &( "out" ) )) # Ptr  |-> out)
+  **  ((( &( "cur" ) )) # Int  |-> (Znth i (c_string (input)) 0))
+  **  ((( &( "right" ) )) # Int  |-> (Znth (i + 1 ) (c_string (input)) 0))
+  **  ((( &( "left" ) )) # Int  |-> (Znth (i - 1 ) (c_string (input)) 0))
+  **  ((( &( "cur_vowel" ) )) # Int  |-> retval)
+  **  ((( &( "right_vowel" ) )) # Int  |-> retval_2)
+  **  ((( &( "left_vowel" ) )) # Int  |-> left_vowel)
+  **  ((( &( "i" ) )) # Int  |-> i)
+|--
+  “ ((Znth (i - 1 ) (c_string (input)) 0) <= 127) ” 
+  &&  “ (0 <= (Znth (i - 1 ) (c_string (input)) 0)) ”
+) \/
+(
+forall (word_pre: Z) (input: (@list Z)) (i: Z) (left_vowel: Z) (out: Z) (n: Z) (retval: Z) (retval_2: Z) (PreH1 : (i <= INT_MAX)) (PreH2 : (left_vowel <= INT_MAX)) (PreH3 : (retval_2 <= INT_MAX)) (PreH4 : (retval <= INT_MAX)) (PreH5 : ((Znth (i - 1 ) (c_string (input)) 0) <= INT_MAX)) (PreH6 : ((Znth (i + 1 ) (c_string (input)) 0) <= INT_MAX)) (PreH7 : ((Znth i (c_string (input)) 0) <= INT_MAX)) (PreH8 : (n <= INT_MAX)) (PreH9 : (i >= INT_MIN)) (PreH10 : (left_vowel >= INT_MIN)) (PreH11 : (retval_2 >= INT_MIN)) (PreH12 : (retval >= INT_MIN)) (PreH13 : ((Znth (i - 1 ) (c_string (input)) 0) >= INT_MIN)) (PreH14 : ((Znth (i + 1 ) (c_string (input)) 0) >= INT_MIN)) (PreH15 : ((Znth i (c_string (input)) 0) >= INT_MIN)) (PreH16 : (n >= INT_MIN)) (PreH17 : (retval_2 = 0)) (PreH18 : (retval_2 = 0)) (PreH19 : ~((is_vowel_z_118 (Znth (i + 1 ) (c_string (input)) 0) ))) (PreH20 : (retval = 1)) (PreH21 : (retval = 1)) (PreH22 : (is_vowel_z_118 (Znth i (c_string (input)) 0) )) (PreH23 : (0 <= ((string_length (input)) + 1 ))) (PreH24 : (i >= 1)) (PreH25 : (n = (string_length (input)))) (PreH26 : (out = 0)) (PreH27 : (3 <= n)) (PreH28 : (n < INT_MAX)) (PreH29 : (0 <= i)) (PreH30 : (i <= (n - 2 ))) (PreH31 : (valid_string input )) (PreH32 : (all_ascii input )) (PreH33 : (problem_118_pre_z input )) (PreH34 : (ascii_range_z input )) (PreH35 : (alpha_codes_z_118 input )) (PreH36 : (no_candidate_after_z_118 input i )) ,
+  (CharArray.full word_pre ((string_length (input)) + 1 ) (c_string (input)) )
+  **  ((( &( "word" ) )) # Ptr  |-> word_pre)
+  **  ((( &( "n" ) )) # Int  |-> n)
+  **  ((( &( "out" ) )) # Ptr  |-> out)
+  **  ((( &( "cur" ) )) # Int  |-> (Znth i (c_string (input)) 0))
+  **  ((( &( "right" ) )) # Int  |-> (Znth (i + 1 ) (c_string (input)) 0))
+  **  ((( &( "left" ) )) # Int  |-> (Znth (i - 1 ) (c_string (input)) 0))
+  **  ((( &( "cur_vowel" ) )) # Int  |-> retval)
+  **  ((( &( "right_vowel" ) )) # Int  |-> retval_2)
+  **  ((( &( "left_vowel" ) )) # Int  |-> left_vowel)
+  **  ((( &( "i" ) )) # Int  |-> i)
+|--
+  “ (0 <= (Znth (i - 1 ) (c_string (input)) 0)) ” 
+  &&  “ ((Znth (i - 1 ) (c_string (input)) 0) <= 127) ”
+).
+
+Definition get_closest_vowel_partial_solve_wit_6_pure_split_goal_1 := 
+forall (word_pre: Z) (input: (@list Z)) (i: Z) (left_vowel: Z) (out: Z) (n: Z) (retval: Z) (retval_2: Z) (PreH1 : (i <= INT_MAX)) (PreH2 : (left_vowel <= INT_MAX)) (PreH3 : (retval_2 <= INT_MAX)) (PreH4 : (retval <= INT_MAX)) (PreH5 : ((Znth (i - 1 ) (c_string (input)) 0) <= INT_MAX)) (PreH6 : ((Znth (i + 1 ) (c_string (input)) 0) <= INT_MAX)) (PreH7 : ((Znth i (c_string (input)) 0) <= INT_MAX)) (PreH8 : (n <= INT_MAX)) (PreH9 : (i >= INT_MIN)) (PreH10 : (left_vowel >= INT_MIN)) (PreH11 : (retval_2 >= INT_MIN)) (PreH12 : (retval >= INT_MIN)) (PreH13 : ((Znth (i - 1 ) (c_string (input)) 0) >= INT_MIN)) (PreH14 : ((Znth (i + 1 ) (c_string (input)) 0) >= INT_MIN)) (PreH15 : ((Znth i (c_string (input)) 0) >= INT_MIN)) (PreH16 : (n >= INT_MIN)) (PreH17 : (retval_2 = 0)) (PreH18 : (retval_2 = 0)) (PreH19 : ~((is_vowel_z_118 (Znth (i + 1 ) (c_string (input)) 0) ))) (PreH20 : (retval = 1)) (PreH21 : (retval = 1)) (PreH22 : (is_vowel_z_118 (Znth i (c_string (input)) 0) )) (PreH23 : (0 <= ((string_length (input)) + 1 ))) (PreH24 : (i >= 1)) (PreH25 : (n = (string_length (input)))) (PreH26 : (out = 0)) (PreH27 : (3 <= n)) (PreH28 : (n < INT_MAX)) (PreH29 : (0 <= i)) (PreH30 : (i <= (n - 2 ))) (PreH31 : (valid_string input )) (PreH32 : (all_ascii input )) (PreH33 : (problem_118_pre_z input )) (PreH34 : (ascii_range_z input )) (PreH35 : (alpha_codes_z_118 input )) (PreH36 : (no_candidate_after_z_118 input i )) ,
+  (CharArray.full word_pre ((string_length (input)) + 1 ) (c_string (input)) )
+  **  ((( &( "word" ) )) # Ptr  |-> word_pre)
+  **  ((( &( "n" ) )) # Int  |-> n)
+  **  ((( &( "out" ) )) # Ptr  |-> out)
+  **  ((( &( "cur" ) )) # Int  |-> (Znth i (c_string (input)) 0))
+  **  ((( &( "right" ) )) # Int  |-> (Znth (i + 1 ) (c_string (input)) 0))
+  **  ((( &( "left" ) )) # Int  |-> (Znth (i - 1 ) (c_string (input)) 0))
+  **  ((( &( "cur_vowel" ) )) # Int  |-> retval)
+  **  ((( &( "right_vowel" ) )) # Int  |-> retval_2)
+  **  ((( &( "left_vowel" ) )) # Int  |-> left_vowel)
+  **  ((( &( "i" ) )) # Int  |-> i)
+|--
+  “ (0 <= (Znth (i - 1 ) (c_string (input)) 0)) ”
+.
+
+Definition get_closest_vowel_partial_solve_wit_6_pure_split_goal_2 := 
+forall (word_pre: Z) (input: (@list Z)) (i: Z) (left_vowel: Z) (out: Z) (n: Z) (retval: Z) (retval_2: Z) (PreH1 : (i <= INT_MAX)) (PreH2 : (left_vowel <= INT_MAX)) (PreH3 : (retval_2 <= INT_MAX)) (PreH4 : (retval <= INT_MAX)) (PreH5 : ((Znth (i - 1 ) (c_string (input)) 0) <= INT_MAX)) (PreH6 : ((Znth (i + 1 ) (c_string (input)) 0) <= INT_MAX)) (PreH7 : ((Znth i (c_string (input)) 0) <= INT_MAX)) (PreH8 : (n <= INT_MAX)) (PreH9 : (i >= INT_MIN)) (PreH10 : (left_vowel >= INT_MIN)) (PreH11 : (retval_2 >= INT_MIN)) (PreH12 : (retval >= INT_MIN)) (PreH13 : ((Znth (i - 1 ) (c_string (input)) 0) >= INT_MIN)) (PreH14 : ((Znth (i + 1 ) (c_string (input)) 0) >= INT_MIN)) (PreH15 : ((Znth i (c_string (input)) 0) >= INT_MIN)) (PreH16 : (n >= INT_MIN)) (PreH17 : (retval_2 = 0)) (PreH18 : (retval_2 = 0)) (PreH19 : ~((is_vowel_z_118 (Znth (i + 1 ) (c_string (input)) 0) ))) (PreH20 : (retval = 1)) (PreH21 : (retval = 1)) (PreH22 : (is_vowel_z_118 (Znth i (c_string (input)) 0) )) (PreH23 : (0 <= ((string_length (input)) + 1 ))) (PreH24 : (i >= 1)) (PreH25 : (n = (string_length (input)))) (PreH26 : (out = 0)) (PreH27 : (3 <= n)) (PreH28 : (n < INT_MAX)) (PreH29 : (0 <= i)) (PreH30 : (i <= (n - 2 ))) (PreH31 : (valid_string input )) (PreH32 : (all_ascii input )) (PreH33 : (problem_118_pre_z input )) (PreH34 : (ascii_range_z input )) (PreH35 : (alpha_codes_z_118 input )) (PreH36 : (no_candidate_after_z_118 input i )) ,
+  (CharArray.full word_pre ((string_length (input)) + 1 ) (c_string (input)) )
+  **  ((( &( "word" ) )) # Ptr  |-> word_pre)
+  **  ((( &( "n" ) )) # Int  |-> n)
+  **  ((( &( "out" ) )) # Ptr  |-> out)
+  **  ((( &( "cur" ) )) # Int  |-> (Znth i (c_string (input)) 0))
+  **  ((( &( "right" ) )) # Int  |-> (Znth (i + 1 ) (c_string (input)) 0))
+  **  ((( &( "left" ) )) # Int  |-> (Znth (i - 1 ) (c_string (input)) 0))
+  **  ((( &( "cur_vowel" ) )) # Int  |-> retval)
+  **  ((( &( "right_vowel" ) )) # Int  |-> retval_2)
+  **  ((( &( "left_vowel" ) )) # Int  |-> left_vowel)
+  **  ((( &( "i" ) )) # Int  |-> i)
+|--
+  “ ((Znth (i - 1 ) (c_string (input)) 0) <= 127) ”
+.
+
+Definition get_closest_vowel_partial_solve_wit_6_aux := 
+forall (word_pre: Z) (input: (@list Z)) (i: Z) (out: Z) (n: Z) (retval: Z) (retval_2: Z) (PreH1 : (retval_2 = 0)) (PreH2 : (retval_2 = 0)) (PreH3 : ~((is_vowel_z_118 (Znth (i + 1 ) (c_string (input)) 0) ))) (PreH4 : (retval = 1)) (PreH5 : (retval = 1)) (PreH6 : (is_vowel_z_118 (Znth i (c_string (input)) 0) )) (PreH7 : (0 <= ((string_length (input)) + 1 ))) (PreH8 : (i >= 1)) (PreH9 : (n = (string_length (input)))) (PreH10 : (out = 0)) (PreH11 : (3 <= n)) (PreH12 : (n < INT_MAX)) (PreH13 : (0 <= i)) (PreH14 : (i <= (n - 2 ))) (PreH15 : (valid_string input )) (PreH16 : (all_ascii input )) (PreH17 : (problem_118_pre_z input )) (PreH18 : (ascii_range_z input )) (PreH19 : (alpha_codes_z_118 input )) (PreH20 : (no_candidate_after_z_118 input i )) ,
+  (CharArray.full word_pre ((string_length (input)) + 1 ) (c_string (input)) )
+|--
+  “ ((Znth (i - 1 ) (c_string (input)) 0) <= 127) ” 
+  &&  “ (0 <= (Znth (i - 1 ) (c_string (input)) 0)) ” 
+  &&  “ (retval_2 = 0) ” 
+  &&  “ (retval_2 = 0) ” 
+  &&  “ ~((is_vowel_z_118 (Znth (i + 1 ) (c_string (input)) 0) )) ” 
+  &&  “ (retval = 1) ” 
+  &&  “ (retval = 1) ” 
+  &&  “ (is_vowel_z_118 (Znth i (c_string (input)) 0) ) ” 
+  &&  “ (0 <= ((string_length (input)) + 1 )) ” 
+  &&  “ (i >= 1) ” 
+  &&  “ (n = (string_length (input))) ” 
+  &&  “ (out = 0) ” 
+  &&  “ (3 <= n) ” 
+  &&  “ (n < INT_MAX) ” 
+  &&  “ (0 <= i) ” 
+  &&  “ (i <= (n - 2 )) ” 
+  &&  “ (valid_string input ) ” 
+  &&  “ (all_ascii input ) ” 
+  &&  “ (problem_118_pre_z input ) ” 
+  &&  “ (ascii_range_z input ) ” 
+  &&  “ (alpha_codes_z_118 input ) ” 
+  &&  “ (no_candidate_after_z_118 input i ) ”
+  &&  (CharArray.full word_pre ((string_length (input)) + 1 ) (c_string (input)) )
+.
+
+Definition get_closest_vowel_partial_solve_wit_6 := get_closest_vowel_partial_solve_wit_6_pure -> get_closest_vowel_partial_solve_wit_6_aux.
+
+Definition get_closest_vowel_partial_solve_wit_7_pure := 
+forall (word_pre: Z) (input: (@list Z)) (n: Z) (out: Z) (cur: Z) (i: Z) (right: Z) (left: Z) (cur_vowel: Z) (right_vowel: Z) (left_vowel: Z) (PreH1 : (n = (string_length (input)))) (PreH2 : (out = 0)) (PreH3 : (cur = (Znth (i) (input) (0)))) (PreH4 : (3 <= n)) (PreH5 : (n < INT_MAX)) (PreH6 : (1 <= i)) (PreH7 : (i <= (n - 2 ))) (PreH8 : (valid_string input )) (PreH9 : (all_ascii input )) (PreH10 : (problem_118_pre_z input )) (PreH11 : (ascii_range_z input )) (PreH12 : (alpha_codes_z_118 input )) (PreH13 : (closest_vowel_candidate_z_118 input i )) (PreH14 : (no_candidate_after_z_118 input i )) ,
+  ((( &( "word" ) )) # Ptr  |-> word_pre)
+  **  ((( &( "n" ) )) # Int  |-> n)
+  **  ((( &( "out" ) )) # Ptr  |-> out)
+  **  ((( &( "cur" ) )) # Int  |-> cur)
+  **  ((( &( "i" ) )) # Int  |-> i)
+  **  ((( &( "right" ) )) # Int  |-> right)
+  **  ((( &( "left" ) )) # Int  |-> left)
+  **  ((( &( "cur_vowel" ) )) # Int  |-> cur_vowel)
+  **  ((( &( "right_vowel" ) )) # Int  |-> right_vowel)
+  **  ((( &( "left_vowel" ) )) # Int  |-> left_vowel)
+  **  (store_string word_pre input )
+|--
+  “ (2 > 0) ” 
+  &&  “ (2 < INT_MAX) ”
+.
+
+Definition get_closest_vowel_partial_solve_wit_7_aux := 
+forall (word_pre: Z) (input: (@list Z)) (n: Z) (out: Z) (cur: Z) (i: Z) (PreH1 : (n = (string_length (input)))) (PreH2 : (out = 0)) (PreH3 : (cur = (Znth (i) (input) (0)))) (PreH4 : (3 <= n)) (PreH5 : (n < INT_MAX)) (PreH6 : (1 <= i)) (PreH7 : (i <= (n - 2 ))) (PreH8 : (valid_string input )) (PreH9 : (all_ascii input )) (PreH10 : (problem_118_pre_z input )) (PreH11 : (ascii_range_z input )) (PreH12 : (alpha_codes_z_118 input )) (PreH13 : (closest_vowel_candidate_z_118 input i )) (PreH14 : (no_candidate_after_z_118 input i )) ,
+  (store_string word_pre input )
+|--
+  “ (2 > 0) ” 
+  &&  “ (2 < INT_MAX) ” 
+  &&  “ (0 <= ((string_length (input)) + 1 )) ” 
+  &&  “ (n = (string_length (input))) ” 
+  &&  “ (out = 0) ” 
+  &&  “ (cur = (Znth (i) (input) (0))) ” 
+  &&  “ (3 <= n) ” 
+  &&  “ (n < INT_MAX) ” 
+  &&  “ (1 <= i) ” 
+  &&  “ (i <= (n - 2 )) ” 
+  &&  “ (valid_string input ) ” 
+  &&  “ (all_ascii input ) ” 
+  &&  “ (problem_118_pre_z input ) ” 
+  &&  “ (ascii_range_z input ) ” 
+  &&  “ (alpha_codes_z_118 input ) ” 
+  &&  “ (closest_vowel_candidate_z_118 input i ) ” 
+  &&  “ (no_candidate_after_z_118 input i ) ”
+  &&  (CharArray.full word_pre ((string_length (input)) + 1 ) (c_string (input)) )
+.
+
+Definition get_closest_vowel_partial_solve_wit_7 := get_closest_vowel_partial_solve_wit_7_pure -> get_closest_vowel_partial_solve_wit_7_aux.
+
+Definition get_closest_vowel_partial_solve_wit_8 := 
+forall (word_pre: Z) (input: (@list Z)) (n: Z) (out: Z) (cur: Z) (i: Z) (retval: Z) (PreH1 : (retval <> 0)) (PreH2 : (retval <> 0)) (PreH3 : (0 <= ((string_length (input)) + 1 ))) (PreH4 : (n = (string_length (input)))) (PreH5 : (out = 0)) (PreH6 : (cur = (Znth (i) (input) (0)))) (PreH7 : (3 <= n)) (PreH8 : (n < INT_MAX)) (PreH9 : (1 <= i)) (PreH10 : (i <= (n - 2 ))) (PreH11 : (valid_string input )) (PreH12 : (all_ascii input )) (PreH13 : (problem_118_pre_z input )) (PreH14 : (ascii_range_z input )) (PreH15 : (alpha_codes_z_118 input )) (PreH16 : (closest_vowel_candidate_z_118 input i )) (PreH17 : (no_candidate_after_z_118 input i )) ,
+  (CharArray.undef_full retval 2 )
+  **  (CharArray.full word_pre ((string_length (input)) + 1 ) (c_string (input)) )
+|--
+  “ (retval <> 0) ” 
+  &&  “ (retval <> 0) ” 
+  &&  “ (0 <= ((string_length (input)) + 1 )) ” 
+  &&  “ (n = (string_length (input))) ” 
+  &&  “ (out = 0) ” 
+  &&  “ (cur = (Znth (i) (input) (0))) ” 
+  &&  “ (3 <= n) ” 
+  &&  “ (n < INT_MAX) ” 
+  &&  “ (1 <= i) ” 
+  &&  “ (i <= (n - 2 )) ” 
+  &&  “ (valid_string input ) ” 
+  &&  “ (all_ascii input ) ” 
+  &&  “ (problem_118_pre_z input ) ” 
+  &&  “ (ascii_range_z input ) ” 
+  &&  “ (alpha_codes_z_118 input ) ” 
+  &&  “ (closest_vowel_candidate_z_118 input i ) ” 
+  &&  “ (no_candidate_after_z_118 input i ) ”
+  &&  (((retval + (0 * sizeof(CHAR) ) )) # Char  |->_)
+  **  (CharArray.undef_missing_i retval 0 0 2 )
+  **  (CharArray.full word_pre ((string_length (input)) + 1 ) (c_string (input)) )
+.
+
+Definition get_closest_vowel_partial_solve_wit_9 := 
+forall (word_pre: Z) (input: (@list Z)) (n: Z) (out: Z) (cur: Z) (i: Z) (retval: Z) (PreH1 : (retval <> 0)) (PreH2 : (retval <> 0)) (PreH3 : (0 <= ((string_length (input)) + 1 ))) (PreH4 : (n = (string_length (input)))) (PreH5 : (out = 0)) (PreH6 : (cur = (Znth (i) (input) (0)))) (PreH7 : (3 <= n)) (PreH8 : (n < INT_MAX)) (PreH9 : (1 <= i)) (PreH10 : (i <= (n - 2 ))) (PreH11 : (valid_string input )) (PreH12 : (all_ascii input )) (PreH13 : (problem_118_pre_z input )) (PreH14 : (ascii_range_z input )) (PreH15 : (alpha_codes_z_118 input )) (PreH16 : (closest_vowel_candidate_z_118 input i )) (PreH17 : (no_candidate_after_z_118 input i )) ,
+  (CharArray.undef_seg retval (0 + 1 ) 2 )
+  **  (((retval + (0 * sizeof(CHAR) ) )) # Char  |-> (signed_last_nbits (cur) (8)))
+  **  (CharArray.full word_pre ((string_length (input)) + 1 ) (c_string (input)) )
+|--
+  “ (retval <> 0) ” 
+  &&  “ (retval <> 0) ” 
+  &&  “ (0 <= ((string_length (input)) + 1 )) ” 
+  &&  “ (n = (string_length (input))) ” 
+  &&  “ (out = 0) ” 
+  &&  “ (cur = (Znth (i) (input) (0))) ” 
+  &&  “ (3 <= n) ” 
+  &&  “ (n < INT_MAX) ” 
+  &&  “ (1 <= i) ” 
+  &&  “ (i <= (n - 2 )) ” 
+  &&  “ (valid_string input ) ” 
+  &&  “ (all_ascii input ) ” 
+  &&  “ (problem_118_pre_z input ) ” 
+  &&  “ (ascii_range_z input ) ” 
+  &&  “ (alpha_codes_z_118 input ) ” 
+  &&  “ (closest_vowel_candidate_z_118 input i ) ” 
+  &&  “ (no_candidate_after_z_118 input i ) ”
+  &&  (((retval + (1 * sizeof(CHAR) ) )) # Char  |->_)
+  **  (CharArray.undef_missing_i retval 1 (0 + 1 ) 2 )
+  **  (((retval + (0 * sizeof(CHAR) ) )) # Char  |-> (signed_last_nbits (cur) (8)))
+  **  (CharArray.full word_pre ((string_length (input)) + 1 ) (c_string (input)) )
+.
+
+Definition get_closest_vowel_partial_solve_wit_10_pure := 
+forall (word_pre: Z) (input: (@list Z)) (n: Z) (out: Z) (cur: Z) (right: Z) (left: Z) (cur_vowel: Z) (right_vowel: Z) (left_vowel: Z) (i: Z) (PreH1 : (n = (string_length (input)))) (PreH2 : (out = 0)) (PreH3 : (i = 0)) (PreH4 : (valid_string input )) (PreH5 : (all_ascii input )) (PreH6 : (problem_118_pre_z input )) (PreH7 : (ascii_range_z input )) (PreH8 : (alpha_codes_z_118 input )) (PreH9 : (no_candidate_after_z_118 input 0 )) ,
+  ((( &( "word" ) )) # Ptr  |-> word_pre)
+  **  ((( &( "n" ) )) # Int  |-> n)
+  **  ((( &( "out" ) )) # Ptr  |-> out)
+  **  ((( &( "cur" ) )) # Int  |-> cur)
+  **  ((( &( "right" ) )) # Int  |-> right)
+  **  ((( &( "left" ) )) # Int  |-> left)
+  **  ((( &( "cur_vowel" ) )) # Int  |-> cur_vowel)
+  **  ((( &( "right_vowel" ) )) # Int  |-> right_vowel)
+  **  ((( &( "left_vowel" ) )) # Int  |-> left_vowel)
+  **  ((( &( "i" ) )) # Int  |-> i)
+  **  (store_string word_pre input )
+|--
+  “ (1 > 0) ” 
+  &&  “ (1 < INT_MAX) ”
+.
+
+Definition get_closest_vowel_partial_solve_wit_10_aux := 
+forall (word_pre: Z) (input: (@list Z)) (n: Z) (out: Z) (i: Z) (PreH1 : (n = (string_length (input)))) (PreH2 : (out = 0)) (PreH3 : (i = 0)) (PreH4 : (valid_string input )) (PreH5 : (all_ascii input )) (PreH6 : (problem_118_pre_z input )) (PreH7 : (ascii_range_z input )) (PreH8 : (alpha_codes_z_118 input )) (PreH9 : (no_candidate_after_z_118 input 0 )) ,
+  (store_string word_pre input )
+|--
+  “ (1 > 0) ” 
+  &&  “ (1 < INT_MAX) ” 
+  &&  “ (0 <= ((string_length (input)) + 1 )) ” 
+  &&  “ (n = (string_length (input))) ” 
+  &&  “ (out = 0) ” 
+  &&  “ (i = 0) ” 
+  &&  “ (valid_string input ) ” 
+  &&  “ (all_ascii input ) ” 
+  &&  “ (problem_118_pre_z input ) ” 
+  &&  “ (ascii_range_z input ) ” 
+  &&  “ (alpha_codes_z_118 input ) ” 
+  &&  “ (no_candidate_after_z_118 input 0 ) ”
+  &&  (CharArray.full word_pre ((string_length (input)) + 1 ) (c_string (input)) )
+.
+
+Definition get_closest_vowel_partial_solve_wit_10 := get_closest_vowel_partial_solve_wit_10_pure -> get_closest_vowel_partial_solve_wit_10_aux.
+
+Definition get_closest_vowel_partial_solve_wit_11 := 
+forall (word_pre: Z) (input: (@list Z)) (n: Z) (out: Z) (i: Z) (retval: Z) (PreH1 : (retval <> 0)) (PreH2 : (retval <> 0)) (PreH3 : (0 <= ((string_length (input)) + 1 ))) (PreH4 : (n = (string_length (input)))) (PreH5 : (out = 0)) (PreH6 : (i = 0)) (PreH7 : (valid_string input )) (PreH8 : (all_ascii input )) (PreH9 : (problem_118_pre_z input )) (PreH10 : (ascii_range_z input )) (PreH11 : (alpha_codes_z_118 input )) (PreH12 : (no_candidate_after_z_118 input 0 )) ,
+  (CharArray.undef_full retval 1 )
+  **  (CharArray.full word_pre ((string_length (input)) + 1 ) (c_string (input)) )
+|--
+  “ (retval <> 0) ” 
+  &&  “ (retval <> 0) ” 
+  &&  “ (0 <= ((string_length (input)) + 1 )) ” 
+  &&  “ (n = (string_length (input))) ” 
+  &&  “ (out = 0) ” 
+  &&  “ (i = 0) ” 
+  &&  “ (valid_string input ) ” 
+  &&  “ (all_ascii input ) ” 
+  &&  “ (problem_118_pre_z input ) ” 
+  &&  “ (ascii_range_z input ) ” 
+  &&  “ (alpha_codes_z_118 input ) ” 
+  &&  “ (no_candidate_after_z_118 input 0 ) ”
+  &&  (((retval + (0 * sizeof(CHAR) ) )) # Char  |->_)
+  **  (CharArray.undef_missing_i retval 0 0 1 )
+  **  (CharArray.full word_pre ((string_length (input)) + 1 ) (c_string (input)) )
+.
+
+Module Type VC_Correct.
+
+Include char_array_Strategy_Correct.
+Include string_Strategy_Correct.
+
+Axiom proof_of_is_vowel_code_118_safety_wit_1 : is_vowel_code_118_safety_wit_1.
+Axiom proof_of_is_vowel_code_118_safety_wit_2 : is_vowel_code_118_safety_wit_2.
+Axiom proof_of_is_vowel_code_118_safety_wit_3 : is_vowel_code_118_safety_wit_3.
+Axiom proof_of_is_vowel_code_118_safety_wit_4 : is_vowel_code_118_safety_wit_4.
+Axiom proof_of_is_vowel_code_118_safety_wit_5 : is_vowel_code_118_safety_wit_5.
+Axiom proof_of_is_vowel_code_118_safety_wit_6 : is_vowel_code_118_safety_wit_6.
+Axiom proof_of_is_vowel_code_118_safety_wit_7 : is_vowel_code_118_safety_wit_7.
+Axiom proof_of_is_vowel_code_118_safety_wit_8 : is_vowel_code_118_safety_wit_8.
+Axiom proof_of_is_vowel_code_118_safety_wit_9 : is_vowel_code_118_safety_wit_9.
+Axiom proof_of_is_vowel_code_118_safety_wit_10 : is_vowel_code_118_safety_wit_10.
+Axiom proof_of_is_vowel_code_118_safety_wit_11 : is_vowel_code_118_safety_wit_11.
+Axiom proof_of_is_vowel_code_118_safety_wit_12 : is_vowel_code_118_safety_wit_12.
+Axiom proof_of_is_vowel_code_118_safety_wit_13 : is_vowel_code_118_safety_wit_13.
+Axiom proof_of_is_vowel_code_118_safety_wit_14 : is_vowel_code_118_safety_wit_14.
+Axiom proof_of_is_vowel_code_118_safety_wit_15 : is_vowel_code_118_safety_wit_15.
+Axiom proof_of_is_vowel_code_118_safety_wit_16 : is_vowel_code_118_safety_wit_16.
+Axiom proof_of_is_vowel_code_118_safety_wit_17 : is_vowel_code_118_safety_wit_17.
+Axiom proof_of_is_vowel_code_118_safety_wit_18 : is_vowel_code_118_safety_wit_18.
+Axiom proof_of_is_vowel_code_118_safety_wit_19 : is_vowel_code_118_safety_wit_19.
+Axiom proof_of_is_vowel_code_118_safety_wit_20 : is_vowel_code_118_safety_wit_20.
+Axiom proof_of_is_vowel_code_118_safety_wit_21 : is_vowel_code_118_safety_wit_21.
+Axiom proof_of_is_vowel_code_118_return_wit_1 : is_vowel_code_118_return_wit_1.
+Axiom proof_of_is_vowel_code_118_return_wit_2 : is_vowel_code_118_return_wit_2.
+Axiom proof_of_is_vowel_code_118_return_wit_3 : is_vowel_code_118_return_wit_3.
+Axiom proof_of_is_vowel_code_118_return_wit_4 : is_vowel_code_118_return_wit_4.
+Axiom proof_of_is_vowel_code_118_return_wit_5 : is_vowel_code_118_return_wit_5.
+Axiom proof_of_is_vowel_code_118_return_wit_6 : is_vowel_code_118_return_wit_6.
+Axiom proof_of_is_vowel_code_118_return_wit_7 : is_vowel_code_118_return_wit_7.
+Axiom proof_of_is_vowel_code_118_return_wit_8 : is_vowel_code_118_return_wit_8.
+Axiom proof_of_is_vowel_code_118_return_wit_9 : is_vowel_code_118_return_wit_9.
+Axiom proof_of_is_vowel_code_118_return_wit_10 : is_vowel_code_118_return_wit_10.
+Axiom proof_of_is_vowel_code_118_return_wit_11 : is_vowel_code_118_return_wit_11.
+Axiom proof_of_get_closest_vowel_safety_wit_1 : get_closest_vowel_safety_wit_1.
+Axiom proof_of_get_closest_vowel_safety_wit_2 : get_closest_vowel_safety_wit_2.
+Axiom proof_of_get_closest_vowel_safety_wit_3 : get_closest_vowel_safety_wit_3.
+Axiom proof_of_get_closest_vowel_safety_wit_4 : get_closest_vowel_safety_wit_4.
+Axiom proof_of_get_closest_vowel_safety_wit_5 : get_closest_vowel_safety_wit_5.
+Axiom proof_of_get_closest_vowel_safety_wit_6 : get_closest_vowel_safety_wit_6.
+Axiom proof_of_get_closest_vowel_safety_wit_7 : get_closest_vowel_safety_wit_7.
+Axiom proof_of_get_closest_vowel_safety_wit_8 : get_closest_vowel_safety_wit_8.
+Axiom proof_of_get_closest_vowel_safety_wit_9 : get_closest_vowel_safety_wit_9.
+Axiom proof_of_get_closest_vowel_safety_wit_10 : get_closest_vowel_safety_wit_10.
+Axiom proof_of_get_closest_vowel_safety_wit_11 : get_closest_vowel_safety_wit_11.
+Axiom proof_of_get_closest_vowel_safety_wit_12 : get_closest_vowel_safety_wit_12.
+Axiom proof_of_get_closest_vowel_safety_wit_13 : get_closest_vowel_safety_wit_13.
+Axiom proof_of_get_closest_vowel_safety_wit_14 : get_closest_vowel_safety_wit_14.
+Axiom proof_of_get_closest_vowel_safety_wit_15 : get_closest_vowel_safety_wit_15.
+Axiom proof_of_get_closest_vowel_safety_wit_16 : get_closest_vowel_safety_wit_16.
+Axiom proof_of_get_closest_vowel_safety_wit_17 : get_closest_vowel_safety_wit_17.
+Axiom proof_of_get_closest_vowel_safety_wit_18 : get_closest_vowel_safety_wit_18.
+Axiom proof_of_get_closest_vowel_safety_wit_19 : get_closest_vowel_safety_wit_19.
+Axiom proof_of_get_closest_vowel_safety_wit_20 : get_closest_vowel_safety_wit_20.
+Axiom proof_of_get_closest_vowel_safety_wit_21 : get_closest_vowel_safety_wit_21.
+Axiom proof_of_get_closest_vowel_safety_wit_22 : get_closest_vowel_safety_wit_22.
+Axiom proof_of_get_closest_vowel_safety_wit_23 : get_closest_vowel_safety_wit_23.
+Axiom proof_of_get_closest_vowel_safety_wit_24 : get_closest_vowel_safety_wit_24.
+Axiom proof_of_get_closest_vowel_safety_wit_25 : get_closest_vowel_safety_wit_25.
+Axiom proof_of_get_closest_vowel_safety_wit_26 : get_closest_vowel_safety_wit_26.
+Axiom proof_of_get_closest_vowel_safety_wit_27 : get_closest_vowel_safety_wit_27.
+Axiom proof_of_get_closest_vowel_safety_wit_28 : get_closest_vowel_safety_wit_28.
+Axiom proof_of_get_closest_vowel_safety_wit_29 : get_closest_vowel_safety_wit_29.
+Axiom proof_of_get_closest_vowel_safety_wit_30 : get_closest_vowel_safety_wit_30.
+Axiom proof_of_get_closest_vowel_safety_wit_31 : get_closest_vowel_safety_wit_31.
+Axiom proof_of_get_closest_vowel_safety_wit_32 : get_closest_vowel_safety_wit_32.
+Axiom proof_of_get_closest_vowel_safety_wit_33 : get_closest_vowel_safety_wit_33.
+Axiom proof_of_get_closest_vowel_safety_wit_34 : get_closest_vowel_safety_wit_34.
+Axiom proof_of_get_closest_vowel_safety_wit_35 : get_closest_vowel_safety_wit_35.
+Axiom proof_of_get_closest_vowel_safety_wit_36 : get_closest_vowel_safety_wit_36.
+Axiom proof_of_get_closest_vowel_safety_wit_37 : get_closest_vowel_safety_wit_37.
+Axiom proof_of_get_closest_vowel_safety_wit_38 : get_closest_vowel_safety_wit_38.
+Axiom proof_of_get_closest_vowel_safety_wit_39 : get_closest_vowel_safety_wit_39.
+Axiom proof_of_get_closest_vowel_safety_wit_40 : get_closest_vowel_safety_wit_40.
+Axiom proof_of_get_closest_vowel_safety_wit_41 : get_closest_vowel_safety_wit_41.
+Axiom proof_of_get_closest_vowel_safety_wit_42 : get_closest_vowel_safety_wit_42.
+Axiom proof_of_get_closest_vowel_safety_wit_43 : get_closest_vowel_safety_wit_43.
+Axiom proof_of_get_closest_vowel_safety_wit_44 : get_closest_vowel_safety_wit_44.
+Axiom proof_of_get_closest_vowel_safety_wit_45 : get_closest_vowel_safety_wit_45.
+Axiom proof_of_get_closest_vowel_entail_wit_1 : get_closest_vowel_entail_wit_1.
+Axiom proof_of_get_closest_vowel_entail_wit_2 : get_closest_vowel_entail_wit_2.
+Axiom proof_of_get_closest_vowel_entail_wit_3 : get_closest_vowel_entail_wit_3.
+Axiom proof_of_get_closest_vowel_entail_wit_4_1 : get_closest_vowel_entail_wit_4_1.
+Axiom proof_of_get_closest_vowel_entail_wit_4_2 : get_closest_vowel_entail_wit_4_2.
+Axiom proof_of_get_closest_vowel_entail_wit_4_3 : get_closest_vowel_entail_wit_4_3.
+Axiom proof_of_get_closest_vowel_entail_wit_5 : get_closest_vowel_entail_wit_5.
+Axiom proof_of_get_closest_vowel_entail_wit_6 : get_closest_vowel_entail_wit_6.
+Axiom proof_of_get_closest_vowel_return_wit_1 : get_closest_vowel_return_wit_1.
+Axiom proof_of_get_closest_vowel_return_wit_2 : get_closest_vowel_return_wit_2.
+Axiom proof_of_get_closest_vowel_return_wit_3 : get_closest_vowel_return_wit_3.
+Axiom proof_of_get_closest_vowel_partial_solve_wit_1_pure : get_closest_vowel_partial_solve_wit_1_pure.
+Axiom proof_of_get_closest_vowel_partial_solve_wit_1 : get_closest_vowel_partial_solve_wit_1.
+Axiom proof_of_get_closest_vowel_partial_solve_wit_2_pure : get_closest_vowel_partial_solve_wit_2_pure.
+Axiom proof_of_get_closest_vowel_partial_solve_wit_2 : get_closest_vowel_partial_solve_wit_2.
+Axiom proof_of_get_closest_vowel_partial_solve_wit_3 : get_closest_vowel_partial_solve_wit_3.
+Axiom proof_of_get_closest_vowel_partial_solve_wit_4_pure : get_closest_vowel_partial_solve_wit_4_pure.
+Axiom proof_of_get_closest_vowel_partial_solve_wit_4 : get_closest_vowel_partial_solve_wit_4.
+Axiom proof_of_get_closest_vowel_partial_solve_wit_5_pure : get_closest_vowel_partial_solve_wit_5_pure.
+Axiom proof_of_get_closest_vowel_partial_solve_wit_5 : get_closest_vowel_partial_solve_wit_5.
+Axiom proof_of_get_closest_vowel_partial_solve_wit_6_pure : get_closest_vowel_partial_solve_wit_6_pure.
+Axiom proof_of_get_closest_vowel_partial_solve_wit_6 : get_closest_vowel_partial_solve_wit_6.
+Axiom proof_of_get_closest_vowel_partial_solve_wit_7_pure : get_closest_vowel_partial_solve_wit_7_pure.
+Axiom proof_of_get_closest_vowel_partial_solve_wit_7 : get_closest_vowel_partial_solve_wit_7.
+Axiom proof_of_get_closest_vowel_partial_solve_wit_8 : get_closest_vowel_partial_solve_wit_8.
+Axiom proof_of_get_closest_vowel_partial_solve_wit_9 : get_closest_vowel_partial_solve_wit_9.
+Axiom proof_of_get_closest_vowel_partial_solve_wit_10_pure : get_closest_vowel_partial_solve_wit_10_pure.
+Axiom proof_of_get_closest_vowel_partial_solve_wit_10 : get_closest_vowel_partial_solve_wit_10.
+Axiom proof_of_get_closest_vowel_partial_solve_wit_11 : get_closest_vowel_partial_solve_wit_11.
+
+End VC_Correct.
