QCP_examples/humaneval/spec_logic_rewrite_c_files/C_118_proof_manual.v
@@ -1,0 +1,211 @@
+Require Import Coq.ZArith.ZArith.
+Require Import Coq.Bool.Bool.
+Require Import Coq.Strings.String.
+Require Import Coq.Strings.Ascii.
+Require Import Coq.Lists.List.
+Require Import Coq.Classes.RelationClasses.
+Require Import Coq.Classes.Morphisms.
+Require Import Coq.micromega.Psatz.
+Require Import Coq.Sorting.Permutation.
+From AUXLib Require Import int_auto Axioms Feq Idents ListLib VMap.
+Require Import SetsClass.SetsClass. Import SetsNotation.
+From SimpleC.SL Require Import Mem SeparationLogic.
+From SimpleC.EE Require Import C_118_goal.
+From SimpleC.EE Require Import C_118_proof_auto.
+Require Import Logic.LogicGenerator.demo932.Interface.
+Local Open Scope Z_scope.
+Local Open Scope sets.
+Local Open Scope string_scope.
+Local Open Scope list.
+Import naive_C_Rules.
+Require Import SimpleC.StdLib.string_lib.
+Require Import coins_118.
+Local Open Scope sac.
+
+Lemma proof_of_is_vowel_code_118_return_wit_1 : is_vowel_code_118_return_wit_1.
+Proof. left; intros; unfold is_vowel_z_118; entailer!; firstorder. Qed.
+
+Lemma proof_of_is_vowel_code_118_return_wit_2 : is_vowel_code_118_return_wit_2.
+Proof. right; intros; unfold is_vowel_z_118; entailer!; firstorder. Qed.
+
+Lemma proof_of_is_vowel_code_118_return_wit_3 : is_vowel_code_118_return_wit_3.
+Proof. right; intros; unfold is_vowel_z_118; entailer!; firstorder. Qed.
+
+Lemma proof_of_is_vowel_code_118_return_wit_4 : is_vowel_code_118_return_wit_4.
+Proof. right; intros; unfold is_vowel_z_118; entailer!; firstorder. Qed.
+
+Lemma proof_of_is_vowel_code_118_return_wit_5 : is_vowel_code_118_return_wit_5.
+Proof. right; intros; unfold is_vowel_z_118; entailer!; firstorder. Qed.
+
+Lemma proof_of_is_vowel_code_118_return_wit_6 : is_vowel_code_118_return_wit_6.
+Proof. right; intros; unfold is_vowel_z_118; entailer!; firstorder. Qed.
+
+Lemma proof_of_is_vowel_code_118_return_wit_7 : is_vowel_code_118_return_wit_7.
+Proof. right; intros; unfold is_vowel_z_118; entailer!; firstorder. Qed.
+
+Lemma proof_of_is_vowel_code_118_return_wit_8 : is_vowel_code_118_return_wit_8.
+Proof. right; intros; unfold is_vowel_z_118; entailer!; firstorder. Qed.
+
+Lemma proof_of_is_vowel_code_118_return_wit_9 : is_vowel_code_118_return_wit_9.
+Proof. right; intros; unfold is_vowel_z_118; entailer!; firstorder. Qed.
+
+Lemma proof_of_is_vowel_code_118_return_wit_10 : is_vowel_code_118_return_wit_10.
+Proof. right; intros; unfold is_vowel_z_118; entailer!; firstorder. Qed.
+
+Lemma proof_of_is_vowel_code_118_return_wit_11 : is_vowel_code_118_return_wit_11.
+Proof. right; intros; unfold is_vowel_z_118; entailer!; firstorder. Qed.
+
+Lemma proof_of_get_closest_vowel_entail_wit_1 : get_closest_vowel_entail_wit_1.
+Proof.
+  right; intros.
+  pose proof (problem_118_pre_z_alpha_codes input PreH5 PreH6).
+  entailer!.
+Qed.
+
+Lemma proof_of_get_closest_vowel_entail_wit_2 : get_closest_vowel_entail_wit_2.
+Proof.
+  right; intros.
+  subst n.
+  pose proof (no_candidate_after_z_118_start input).
+  unfold string_length in *.
+  entailer!.
+Qed.
+
+Lemma proof_of_get_closest_vowel_entail_wit_3 : get_closest_vowel_entail_wit_3.
+Proof.
+  right; intros.
+  assert (Hi : 1 <= i < Zlength input - 1) by
+    (unfold string_length in *; lia).
+  pose proof (candidate_z_118_from_c_string input i PreH22 Hi
+    PreH3 PreH9 PreH6) as Hcandidate.
+  pose proof (c_string_inside_eq_118 input i ltac:(lia)) as Heq.
+  entailer!.
+Qed.
+
+Lemma proof_of_get_closest_vowel_entail_wit_4_1 : get_closest_vowel_entail_wit_4_1.
+Proof.
+  right; intros.
+  entailer!.
+  apply candidate_z_118_not_cur.
+  - unfold string_length in *; lia.
+  - exact PreH3.
+Qed.
+
+Lemma proof_of_get_closest_vowel_entail_wit_4_2 : get_closest_vowel_entail_wit_4_2.
+Proof.
+  right; intros.
+  entailer!.
+  apply candidate_z_118_not_right.
+  - unfold string_length in *; lia.
+  - exact PreH3.
+Qed.
+
+Lemma proof_of_get_closest_vowel_entail_wit_4_3 : get_closest_vowel_entail_wit_4_3.
+Proof.
+  right; intros.
+  entailer!.
+  apply candidate_z_118_not_left.
+  - unfold string_length in *; lia.
+  - exact PreH3.
+Qed.
+
+Lemma proof_of_get_closest_vowel_entail_wit_5 : get_closest_vowel_entail_wit_5.
+Proof.
+  right; intros.
+  pose proof (no_candidate_after_z_118_step input i PreH13 PreH14).
+  entailer!.
+Qed.
+
+Lemma proof_of_get_closest_vowel_entail_wit_6 : get_closest_vowel_entail_wit_6.
+Proof.
+  right; intros.
+  assert (i = 0) by lia; subst i.
+  entailer!.
+Qed.
+
+Lemma proof_of_get_closest_vowel_return_wit_1 : get_closest_vowel_return_wit_1.
+Proof.
+  left; intros.
+  Exists (@nil Z).
+  pose proof (problem_118_spec_z_not_found input PreH10 PreH12).
+  unfold store_string, string_length, c_string.
+  simpl.
+  entailer!.
+  rewrite (CharArray.undef_seg_empty retval 1).
+  sep_apply_l_atomic (CharArray.seg_single retval 0 0).
+  sep_apply_l_atomic (CharArray.seg_to_full retval 0 1 (0 :: nil)).
+  replace (retval + 0 * sizeof(CHAR)) with retval by lia.
+  replace (1 - 0) with 1 by lia.
+  entailer!.
+Qed.
+
+Lemma proof_of_get_closest_vowel_return_wit_2 : get_closest_vowel_return_wit_2.
+Proof.
+  left; intros; subst cur.
+  Exists (Znth i input 0 :: nil).
+  pose proof (problem_118_spec_z_found input i PreH14 PreH16 PreH17).
+  assert (Hrange : 0 <= Znth i input 0 <= 127).
+  { apply alpha_codes_z_118_range with (input := input); [exact PreH15 |].
+    unfold string_length in *; lia. }
+  rewrite (signed_last_nbits_eq (Znth i input 0) 8) by lia.
+  unfold store_string, string_length, c_string.
+  simpl.
+  entailer!.
+  rewrite (CharArray.undef_seg_empty retval 2).
+  sep_apply_l_atomic (CharArray.seg_single retval 1 0).
+  sep_apply_l_atomic (CharArray.seg_single retval 0 (Znth i input 0)).
+  replace (1 + 1) with 2 by lia.
+  replace (0 + 1) with 1 by lia.
+  rewrite derivable1_sepcon_comm.
+  sep_apply_l_atomic (CharArray.seg_merge_to_seg
+    retval 0 1 2 (Znth i input 0 :: nil) (0 :: nil)).
+  - entailer!.
+  - simpl.
+    sep_apply_l_atomic (CharArray.seg_to_full retval 0 2
+      (Znth i input 0 :: 0 :: nil)).
+    replace (retval + 0 * sizeof(CHAR)) with retval by lia.
+    replace (2 - 0) with 2 by lia.
+    entailer!.
+Qed.
+
+Lemma proof_of_get_closest_vowel_return_wit_3 : get_closest_vowel_return_wit_3.
+Proof.
+  left; intros.
+  Exists (@nil Z).
+  pose proof (problem_118_spec_z_short input PreH10 ltac:(unfold string_length in *; lia)).
+  unfold store_string, string_length, c_string.
+  simpl.
+  entailer!.
+  rewrite (CharArray.undef_seg_empty retval 1).
+  sep_apply_l_atomic (CharArray.seg_single retval 0 0).
+  sep_apply_l_atomic (CharArray.seg_to_full retval 0 1 (0 :: nil)).
+  replace (retval + 0 * sizeof(CHAR)) with retval by lia.
+  replace (1 - 0) with 1 by lia.
+  entailer!.
+Qed.
+
+Lemma proof_of_get_closest_vowel_partial_solve_wit_4_pure :
+  get_closest_vowel_partial_solve_wit_4_pure.
+Proof.
+  left; intros.
+  pose proof (alpha_codes_c_string_range_118 input i PreH12 ltac:(unfold string_length in *; lia)).
+  entailer!.
+Qed.
+
+Lemma proof_of_get_closest_vowel_partial_solve_wit_5_pure :
+  get_closest_vowel_partial_solve_wit_5_pure.
+Proof.
+  left; intros.
+  pose proof (alpha_codes_c_string_range_118 input (i + 1) PreH16
+    ltac:(unfold string_length in *; lia)).
+  entailer!.
+Qed.
+
+Lemma proof_of_get_closest_vowel_partial_solve_wit_6_pure :
+  get_closest_vowel_partial_solve_wit_6_pure.
+Proof.
+  left; intros.
+  pose proof (alpha_codes_c_string_range_118 input (i - 1) PreH19
+    ltac:(unfold string_length in *; lia)).
+  entailer!.
+Qed.
