QCP_examples/humaneval/spec_logic_rewrite_c_files/coins_118.v
@@ -1,0 +1,397 @@
+Load "../spec/118".
+
+Require Import Coq.ZArith.ZArith.
+Require Import Coq.Lists.List.
+Require Import Coq.Strings.String.
+Require Import Coq.Strings.Ascii.
+Require Import Lia.
+From AUXLib Require Import ListLib.
+From SimpleC.SL Require Import IntLib.
+Require Import SimpleC.StdLib.string_lib.
+Load "../StringClaude/string_bridge".
+Import ListNotations.
+
+Local Open Scope Z_scope.
+Local Open Scope string_scope.
+
+Definition problem_118_pre_z (input : list Z) : Prop :=
+  problem_118_pre (string_of_list_z input).
+
+Definition problem_118_spec_z (input output : list Z) : Prop :=
+  problem_118_spec (string_of_list_z input) (string_of_list_z output).
+
+Definition is_vowel_z_118 (c : Z) : Prop :=
+  c = 65 \/ c = 69 \/ c = 73 \/ c = 79 \/ c = 85 \/
+  c = 97 \/ c = 101 \/ c = 105 \/ c = 111 \/ c = 117.
+
+Definition is_alpha_z_118 (c : Z) : Prop :=
+  65 <= c <= 90 \/ 97 <= c <= 122.
+
+Definition is_consonant_z_118 (c : Z) : Prop :=
+  is_alpha_z_118 c /\ ~ is_vowel_z_118 c.
+
+Definition alpha_codes_z_118 (input : list Z) : Prop :=
+  forall i, 0 <= i < Zlength input ->
+    is_alpha_z_118 (Znth i input 0).
+
+Definition closest_vowel_candidate_z_118
+    (input : list Z) (i : Z) : Prop :=
+  1 <= i < Zlength input - 1 /\
+  is_consonant_z_118 (Znth (i - 1) input 0) /\
+  is_vowel_z_118 (Znth i input 0) /\
+  is_consonant_z_118 (Znth (i + 1) input 0).
+
+Definition no_candidate_after_z_118
+    (input : list Z) (i : Z) : Prop :=
+  forall j, i < j < Zlength input - 1 ->
+    ~ closest_vowel_candidate_z_118 input j.
+
+Lemma problem_118_pre_z_alpha_codes : forall input,
+  problem_118_pre_z input ->
+  ascii_range_z input ->
+  alpha_codes_z_118 input.
+Proof.
+  intros input Hpre Hrange i Hi.
+  unfold problem_118_pre_z, problem_118_pre in Hpre.
+  rewrite list_ascii_of_string_string_of_list_z in Hpre.
+  apply Forall_forall with (x := ascii_of_z (Znth i input 0)) in Hpre.
+  - unfold is_alpha in Hpre.
+    rewrite nat_of_ascii_ascii_of_z in Hpre by (apply Hrange; lia).
+    unfold is_alpha_z_118.
+    lia.
+  - apply in_map.
+    unfold Znth.
+    apply nth_In.
+    rewrite <- z_to_nat_Zlength.
+    lia.
+Qed.
+
+Lemma is_vowel_z_118_range : forall c,
+  is_vowel_z_118 c -> 0 <= c <= 127.
+Proof.
+  intros c H.
+  unfold is_vowel_z_118 in H.
+  lia.
+Qed.
+
+Lemma alpha_codes_z_118_range : forall input i,
+  alpha_codes_z_118 input ->
+  0 <= i < Zlength input ->
+  0 <= Znth i input 0 <= 127.
+Proof.
+  intros input i Halpha Hi.
+  specialize (Halpha i Hi).
+  unfold is_alpha_z_118 in Halpha.
+  lia.
+Qed.
+
+Lemma no_candidate_after_z_118_start : forall input,
+  no_candidate_after_z_118 input (Zlength input - 2).
+Proof.
+  unfold no_candidate_after_z_118.
+  intros input j Hj.
+  lia.
+Qed.
+
+Lemma no_candidate_after_z_118_step : forall input i,
+  ~ closest_vowel_candidate_z_118 input i ->
+  no_candidate_after_z_118 input i ->
+  no_candidate_after_z_118 input (i - 1).
+Proof.
+  unfold no_candidate_after_z_118.
+  intros input i Hnot Hafter j Hj.
+  destruct (Z.eq_dec j i) as [-> | Hne].
+  - exact Hnot.
+  - apply Hafter.
+    lia.
+Qed.
+
+Lemma c_string_inside_eq_118 : forall input i,
+  0 <= i < Zlength input ->
+  Znth i (c_string input) 0 = Znth i input 0.
+Proof.
+  intros input i Hi.
+  apply c_string_Znth_inside.
+  exact Hi.
+Qed.
+
+Lemma alpha_codes_c_string_range_118 : forall input i,
+  alpha_codes_z_118 input ->
+  0 <= i < Zlength input ->
+  0 <= Znth i (c_string input) 0 <= 127.
+Proof.
+  intros input i Halpha Hi.
+  rewrite c_string_inside_eq_118 by exact Hi.
+  apply alpha_codes_z_118_range; assumption.
+Qed.
+
+Lemma candidate_z_118_from_c_string : forall input i,
+  alpha_codes_z_118 input ->
+  1 <= i < Zlength input - 1 ->
+  ~ is_vowel_z_118 (Znth (i - 1) (c_string input) 0) ->
+  is_vowel_z_118 (Znth i (c_string input) 0) ->
+  ~ is_vowel_z_118 (Znth (i + 1) (c_string input) 0) ->
+  closest_vowel_candidate_z_118 input i.
+Proof.
+  intros input i Halpha Hi Hleft Hcur Hright.
+  unfold closest_vowel_candidate_z_118, is_consonant_z_118.
+  split; [exact Hi |].
+  rewrite !c_string_inside_eq_118 in * by lia.
+  repeat split; try assumption.
+  - apply Halpha. lia.
+  - apply Halpha. lia.
+Qed.
+
+Lemma candidate_z_118_not_cur : forall input i,
+  1 <= i < Zlength input - 1 ->
+  ~ is_vowel_z_118 (Znth i (c_string input) 0) ->
+  ~ closest_vowel_candidate_z_118 input i.
+Proof.
+  intros input i Hi Hnot Hcandidate.
+  destruct Hcandidate as [_ [_ [Hcur _]]].
+  rewrite c_string_inside_eq_118 in Hnot by lia.
+  contradiction.
+Qed.
+
+Lemma candidate_z_118_not_right : forall input i,
+  1 <= i < Zlength input - 1 ->
+  is_vowel_z_118 (Znth (i + 1) (c_string input) 0) ->
+  ~ closest_vowel_candidate_z_118 input i.
+Proof.
+  intros input i Hi Hvowel Hcandidate.
+  destruct Hcandidate as [_ [_ [_ [_ Hnot]]]].
+  rewrite c_string_inside_eq_118 in Hvowel by lia.
+  contradiction.
+Qed.
+
+Lemma candidate_z_118_not_left : forall input i,
+  1 <= i < Zlength input - 1 ->
+  is_vowel_z_118 (Znth (i - 1) (c_string input) 0) ->
+  ~ closest_vowel_candidate_z_118 input i.
+Proof.
+  intros input i Hi Hvowel Hcandidate.
+  destruct Hcandidate as [_ [[_ Hnot] _]].
+  rewrite c_string_inside_eq_118 in Hvowel by lia.
+  contradiction.
+Qed.
+
+Lemma is_vowel_z_118_to_spec : forall c,
+  is_vowel_z_118 c -> is_vowel (ascii_of_z c).
+Proof.
+  intros c H.
+  unfold is_vowel_z_118 in H.
+  repeat (destruct H as [-> | H]; [simpl; exact I |]).
+  subst; simpl; exact I.
+Qed.
+
+Lemma spec_vowel_to_is_vowel_z_118 : forall c,
+  0 <= c < 256 ->
+  is_vowel (ascii_of_z c) ->
+  is_vowel_z_118 c.
+Proof.
+  intros c Hrange Hvowel.
+  unfold ascii_of_z in Hvowel.
+  remember (ascii_of_nat (Z.to_nat c)) as a eqn:Ha.
+  destruct a as [b0 b1 b2 b3 b4 b5 b6 b7].
+  destruct b0, b1, b2, b3, b4, b5, b6, b7;
+    simpl in Hvowel; try contradiction;
+    apply (f_equal nat_of_ascii) in Ha;
+    rewrite nat_ascii_embedding in Ha by lia;
+    cbn in Ha;
+    unfold is_vowel_z_118; lia.
+Qed.
+
+Lemma is_alpha_z_118_to_spec : forall c,
+  0 <= c < 256 ->
+  is_alpha_z_118 c ->
+  is_alpha (ascii_of_z c).
+Proof.
+  intros c Hrange Halpha.
+  unfold is_alpha.
+  rewrite nat_of_ascii_ascii_of_z by exact Hrange.
+  unfold is_alpha_z_118 in Halpha.
+  lia.
+Qed.
+
+Lemma spec_alpha_to_is_alpha_z_118 : forall c,
+  0 <= c < 256 ->
+  is_alpha (ascii_of_z c) ->
+  is_alpha_z_118 c.
+Proof.
+  intros c Hrange Halpha.
+  unfold is_alpha in Halpha.
+  rewrite nat_of_ascii_ascii_of_z in Halpha by exact Hrange.
+  unfold is_alpha_z_118.
+  lia.
+Qed.
+
+Lemma is_consonant_z_118_to_spec : forall c,
+  0 <= c < 256 ->
+  is_consonant_z_118 c ->
+  is_consonant (ascii_of_z c).
+Proof.
+  intros c Hrange [Halpha Hnot].
+  split.
+  - apply is_alpha_z_118_to_spec; assumption.
+  - intro Hvowel.
+    apply Hnot.
+    apply spec_vowel_to_is_vowel_z_118; assumption.
+Qed.
+
+Lemma spec_consonant_to_is_consonant_z_118 : forall c,
+  0 <= c < 256 ->
+  is_consonant (ascii_of_z c) ->
+  is_consonant_z_118 c.
+Proof.
+  intros c Hrange [Halpha Hnot].
+  split.
+  - apply spec_alpha_to_is_alpha_z_118; assumption.
+  - intro Hvowel.
+    apply Hnot.
+    apply is_vowel_z_118_to_spec.
+    exact Hvowel.
+Qed.
+
+Lemma candidate_z_118_to_spec : forall input i,
+  ascii_range_z input ->
+  closest_vowel_candidate_z_118 input i ->
+  vowel_between_consonants
+    (string_of_list_z input) (Z.to_nat i)
+    (ascii_of_z (Znth i input 0)).
+Proof.
+  intros input i Hrange [Hi [Hleft [Hcur Hright]]].
+  unfold vowel_between_consonants.
+  split.
+  - rewrite string_of_list_z_length.
+    rewrite <- z_to_nat_Zlength.
+    lia.
+  - exists (ascii_of_z (Znth (i - 1) input 0)).
+    exists (ascii_of_z (Znth (i + 1) input 0)).
+    split.
+    + replace (Z.to_nat i - 1)%nat with (Z.to_nat (i - 1)) by lia.
+      apply string_get_string_of_list_z_z.
+      lia.
+    + split.
+      * apply string_get_string_of_list_z_z.
+        lia.
+      * split.
+        -- replace (Z.to_nat i + 1)%nat with (Z.to_nat (i + 1)) by lia.
+           apply string_get_string_of_list_z_z.
+           lia.
+        -- split.
+           ++ apply is_consonant_z_118_to_spec.
+              ** apply Hrange. lia.
+              ** exact Hleft.
+           ++ split.
+              ** apply is_vowel_z_118_to_spec.
+                 exact Hcur.
+              ** apply is_consonant_z_118_to_spec.
+                 --- apply Hrange. lia.
+                 --- exact Hright.
+Qed.
+
+Lemma spec_candidate_to_candidate_z_118 : forall input i vowel,
+  ascii_range_z input ->
+  vowel_between_consonants (string_of_list_z input) i vowel ->
+  closest_vowel_candidate_z_118 input (Z.of_nat i).
+Proof.
+  intros input i vowel Hrange [Hi [left [right Hcandidate]]].
+  destruct Hcandidate as [Hleft_get [Hvowel_get [Hright_get Hprops]]].
+  destruct Hprops as [Hleft [Hvowel Hright]].
+  unfold closest_vowel_candidate_z_118.
+  split.
+  - rewrite string_of_list_z_length in Hi.
+    rewrite <- z_to_nat_Zlength in Hi.
+    lia.
+  - assert (Hzi : 1 <= Z.of_nat i < Zlength input - 1).
+    { rewrite string_of_list_z_length in Hi.
+      rewrite <- z_to_nat_Zlength in Hi.
+      lia. }
+    assert (Hget_left :
+      String.get (i - 1)%nat (string_of_list_z input) =
+      Some (ascii_of_z (Znth (Z.of_nat i - 1) input 0))).
+    { replace (i - 1)%nat with (Z.to_nat (Z.of_nat i - 1)) by lia.
+      apply string_get_string_of_list_z_z. lia. }
+    pose proof
+      (string_get_string_of_list_z_z input (Z.of_nat i) ltac:(lia))
+      as Hget_cur.
+    rewrite Nat2Z.id in Hget_cur.
+    assert (Hget_right :
+      String.get (i + 1)%nat (string_of_list_z input) =
+      Some (ascii_of_z (Znth (Z.of_nat i + 1) input 0))).
+    { replace (i + 1)%nat with (Z.to_nat (Z.of_nat i + 1)) by lia.
+      apply string_get_string_of_list_z_z. lia. }
+    rewrite Hleft_get in Hget_left.
+    rewrite Hvowel_get in Hget_cur.
+    rewrite Hright_get in Hget_right.
+    inversion Hget_left; inversion Hget_cur; inversion Hget_right; subst.
+    split.
+    + apply spec_consonant_to_is_consonant_z_118.
+      * apply Hrange. lia.
+      * exact Hleft.
+    + split.
+      * apply spec_vowel_to_is_vowel_z_118.
+        -- apply Hrange. lia.
+        -- exact Hvowel.
+      * apply spec_consonant_to_is_consonant_z_118.
+        -- apply Hrange. lia.
+        -- exact Hright.
+Qed.
+
+Lemma problem_118_spec_z_found : forall input i,
+  ascii_range_z input ->
+  closest_vowel_candidate_z_118 input i ->
+  no_candidate_after_z_118 input i ->
+  problem_118_spec_z input [Znth i input 0].
+Proof.
+  intros input i Hrange Hcandidate Hafter.
+  unfold problem_118_spec_z, problem_118_spec.
+  left.
+  exists (Z.to_nat i), (ascii_of_z (Znth i input 0)).
+  split.
+  - apply candidate_z_118_to_spec; assumption.
+  - split.
+    + intros j other Hij Hbad.
+      apply (Hafter (Z.of_nat j)).
+      * destruct Hbad as [Hj _].
+        rewrite string_of_list_z_length in Hj.
+        rewrite <- z_to_nat_Zlength in Hj.
+        destruct Hcandidate as [Hi _].
+        lia.
+      * apply spec_candidate_to_candidate_z_118 with (vowel := other);
+          assumption.
+    + reflexivity.
+Qed.
+
+Lemma problem_118_spec_z_not_found : forall input,
+  ascii_range_z input ->
+  no_candidate_after_z_118 input 0 ->
+  problem_118_spec_z input [].
+Proof.
+  intros input Hrange Hnone.
+  unfold problem_118_spec_z, problem_118_spec.
+  right.
+  split.
+  - intros i vowel Hbad.
+    apply (Hnone (Z.of_nat i)).
+    + destruct Hbad as [Hi _].
+      rewrite string_of_list_z_length in Hi.
+      rewrite <- z_to_nat_Zlength in Hi.
+      lia.
+    + apply spec_candidate_to_candidate_z_118 with (vowel := vowel);
+        assumption.
+  - reflexivity.
+Qed.
+
+Lemma problem_118_spec_z_short : forall input,
+  ascii_range_z input ->
+  Zlength input < 3 ->
+  problem_118_spec_z input [].
+Proof.
+  intros input Hrange Hshort.
+  apply problem_118_spec_z_not_found; [exact Hrange |].
+  unfold no_candidate_after_z_118.
+  intros j Hj Hcandidate.
+  destruct Hcandidate as [Hbounds _].
+  lia.
+Qed.
